<?xml version="1.0" encoding="UTF-8"?>
<rdf:RDF xmlns:rdf="http://www.w3.org/1999/02/22-rdf-syntax-ns#" xmlns:rdfs="http://www.w3.org/2000/01/rdf-schema#" xmlns:skos="http://www.w3.org/2004/02/skos/core#" xmlns:dc="http://purl.org/dc/elements/1.1/" xmlns:dct="http://purl.org/dc/terms/" xml:lang="en">

	<!--

	# This file includes the CaLAThe concept scheme part of the 6th version of CaLAThe, which is available online at cadastralvocabulary.org/CaLAThe.rdf
	The present CaLAThe concept scheme part and the corresponding CaLATheCodeList concept scheme part are provided in separate files. #

	<skos:Collection rdf:about="http://www.cadastralvocabulary.org/CaLATheSet">
	<skos:member>rdf:about="http://www.cadastralvocabulary.org/CaLAThe"</skos:member>
	<skos:member>rdf:about="http://www.cadastralvocabulary.org/CaLATheCodeList"</skos:member>
	</skos:Collection>

	-->

	<skos:ConceptScheme rdf:about="http://www.cadastralvocabulary.org/CaLAThe">
		<skos:prefLabel>CaLAThe 6.0</skos:prefLabel>
		<dc:title>CaLAThe - Cadastre and Land Administration Thesaurus, version 6.0</dc:title>
		<skos:description>The Thesaurus for the domain of Cadastre and Land Administration, CaLAThe, regards the surveying and mapping of land, more specifically the boundaries of land parcels and individually owned buildings and building parts (condominiums), as performed by the profession of surveyors. From a public point of view, the domain provides the administrative and technical base for taxation of land and buildings, and for land use planning; from a private point of view, the domain supports security in ownership and other land-related rights. CaLAThe lies partly within the technical domains of civil engineering and computer science, partly within social science domains, including law and public administration</skos:description>
		<dc:description>The Cadastre and Land Administration Thesaurus, CaLAThe, is a controlled vocabulary, recorded at http://www.cadastralvocabulary.org. The initial 2011 version of CaLAThe was prepared based on terms and term relationships derived from DIS version of the ISO 19152:2012 Land Administration Domain Model (LADM). Moreover, it referred to existing thesauri, primarily the GEMET thesaurus, the AGROVOC thesaurus, and the STW Thesaurus for Economics. Terms rendering dynamic or temporal aspects of the domain were added in version 2, while version 3 was supplemented with terms from the OGC Land and Infrastructure Conceptual Model Standard (LandInfra). Version 4 added code lists names and values from both standards, specified within its own skos:ConceptScheme. The code list values refer to CaLAThe thesaurus terms when possible in a meaningful way. Version 5 started a multi-lingual itinerary by adding terms (skos:prefLabel) in Danish and Turkish, the native language of the authors. Version 6 presents new and revised definitions for CaLAThe concepts. Intensional definition (also known as the genus-differentia definition) method recommended by ISO 704:2009 ‘Terminology work - Principles and methods’ is applied in the preparation of definitions. This new version also improves multilingualism of CaLAThe by adding Malay terms. The corresponding code list part, version 2, includes code lists specified in Land and Survey parts of OGC LandInfra. Also, a skos:Collection statement was added to specify relations between the two skos:ConceptSchemes. - The content of the present file may be queried by means of the SKOS Play facility at http://labs.sparna.fr/skos-play/. SKOS Play offers presentation of each of the two concept schemes, as well as each of the three languages. Validated through http://demo.seco.tkk.fi/skosify/skosify</dc:description>
		<dc:creator>Erik Stubkjær</dc:creator>
		<dc:creator> Volkan Çağdaş</dc:creator>
		<dc:date>2023-10-01</dc:date>
		<dct:issued>2023-10-01</dct:issued>
		<skos:hasTopConcept rdf:resource="http://www.cadastralvocabulary.org/CaLAThe/Party"/>
		<skos:hasTopConcept rdf:resource="http://www.cadastralvocabulary.org/CaLAThe/Law"/>
		<skos:hasTopConcept rdf:resource="http://www.cadastralvocabulary.org/CaLAThe/Information"/>
		<skos:hasTopConcept rdf:resource="http://www.cadastralvocabulary.org/CaLAThe/Land"/>
		<skos:hasTopConcept rdf:resource="http://www.cadastralvocabulary.org/CaLAThe/Activity"/>
		<skos:hasTopConcept rdf:resource="http://www.cadastralvocabulary.org/CaLAThe/Survey"/>
	</skos:ConceptScheme>

	<skos:Concept rdf:about="http://www.cadastralvocabulary.org/CaLAThe/2D">
		<skos:prefLabel xml:lang="en">2D</skos:prefLabel>
		<skos:prefLabel xml:lang="da">2D</skos:prefLabel>
		<skos:prefLabel xml:lang="tr">2B</skos:prefLabel>
		<skos:prefLabel xml:lang="ms">2D</skos:prefLabel>
		<skos:scopeNote>OGC LandInfra / InfraGML term</skos:scopeNote>
		<skos:definition>Dimension type, cf. OGC LandInfra 7.10.6 SpatialUnit</skos:definition>
		<skos:changeNote>Established with version 4</skos:changeNote>
		<skos:inScheme rdf:resource="http://www.cadastralvocabulary.org/CaLAThe"/>
		<skos:broader rdf:resource="http://www.cadastralvocabulary.org/CaLAThe/DimensionType"/>
	</skos:Concept>

	<skos:Concept rdf:about="http://www.cadastralvocabulary.org/CaLAThe/3D">
		<skos:prefLabel xml:lang="en">3D</skos:prefLabel>
		<skos:prefLabel xml:lang="da">3D</skos:prefLabel>
		<skos:prefLabel xml:lang="tr">3B</skos:prefLabel>
		<skos:prefLabel xml:lang="ms">3D</skos:prefLabel>
		<skos:scopeNote>OGC LandInfra / InfraGML term</skos:scopeNote>
		<skos:definition>Dimension type, cf. OGC LandInfra 7.10.6 SpatialUnit</skos:definition>
		<skos:changeNote>Established with version 4</skos:changeNote>
		<skos:inScheme rdf:resource="http://www.cadastralvocabulary.org/CaLAThe"/>
		<skos:broader rdf:resource="http://www.cadastralvocabulary.org/CaLAThe/DimensionType"/>
	</skos:Concept>

	<skos:Concept rdf:about="http://www.cadastralvocabulary.org/CaLAThe/Activity">
		<skos:prefLabel xml:lang="en">Activity</skos:prefLabel>
		<skos:prefLabel xml:lang="da">Aktivitet</skos:prefLabel>
		<skos:prefLabel xml:lang="tr">Aktivite</skos:prefLabel>
		<skos:prefLabel xml:lang="ms">Aktiviti</skos:prefLabel>
		<skos:altLabel>Transaction</skos:altLabel>
		<skos:altLabel>Registration</skos:altLabel>	<skos:scopeNote>EULIS / ELRA glossary term</skos:scopeNote>
		<skos:definition>Activity which through document investigations, field research and surveys clarifies and documents the location of an existing parcel boundary. National ruling may request boundary disputes be addressed through this activity before civil lawsuit is filed.</skos:definition>
		<skos:changeNote>Established with version 2. Narrower ParcelEstablishment added with version 3. Survey with version 4.</skos:changeNote>
		<skos:inScheme rdf:resource="http://www.cadastralvocabulary.org/CaLAThe"/>
		<skos:narrower rdf:resource="http://www.cadastralvocabulary.org/CaLAThe/Exchange"/>
		<skos:narrower rdf:resource="http://www.cadastralvocabulary.org/CaLAThe/PropertyFormation"/>
		<skos:narrower rdf:resource="http://www.cadastralvocabulary.org/CaLAThe/Transfer"/>
	</skos:Concept>

	<skos:Concept rdf:about="http://www.cadastralvocabulary.org/CaLAThe/AdministrativeUnit">
		<skos:prefLabel xml:lang="en">Administrative unit</skos:prefLabel>
		<skos:prefLabel xml:lang="da">Administrativ inddeling</skos:prefLabel>
		<skos:prefLabel xml:lang="tr">İdari birim</skos:prefLabel>
		<skos:prefLabel xml:lang="ms">Unit pentadbiran</skos:prefLabel>
		<skos:altLabel>Jurisdiction</skos:altLabel>
		<skos:altLabel>LA_SpatialUnitGroup</skos:altLabel>
		<skos:altLabel>Administrative division</skos:altLabel>
		<skos:scopeNote>GEMET term</skos:scopeNote>
		<skos:definition>Unit of administration where a Member State has and/or exercises jurisdictional rights, for local, regional and national governance (Source: INSPIRE feature concept dictionary).</skos:definition>
		<skos:changeNote>Established with version 1. Edited with version 3 and 4. Definition is revised in version 5.</skos:changeNote>
		<skos:exactMatch rdf:resource="http://inspire.ec.europa.eu/featureconcept/AdministrativeUnit"/>
		<skos:exactMatch rdf:resource="http://eurovoc.europa.eu/362"/>
		<skos:inScheme rdf:resource="http://www.cadastralvocabulary.org/CaLAThe"/>
		<skos:broader rdf:resource="http://www.cadastralvocabulary.org/CaLAThe/LandDivision"/>
		<skos:narrower rdf:resource="http://www.cadastralvocabulary.org/CaLAThe/NUTSRegion"/>
		<skos:narrower rdf:resource="http://www.cadastralvocabulary.org/CaLAThe/ProtectedSite"/>
		<skos:narrower rdf:resource="http://www.cadastralvocabulary.org/CaLAThe/Site"/>
	</skos:Concept>

	<skos:Concept rdf:about="http://www.cadastralvocabulary.org/CaLAThe/AdversePossession">
		<skos:prefLabel xml:lang="en">Adverse possession</skos:prefLabel>
		<skos:prefLabel xml:lang="da">Ejendomshævd</skos:prefLabel>
		<skos:prefLabel xml:lang="tr">Kazandırıcı zamanaşımı</skos:prefLabel>
		<skos:prefLabel xml:lang="ms">Pendudukan bertentangan</skos:prefLabel>
		<skos:altLabel>Prescriptive acquisition</skos:altLabel>
		<skos:changeNote>Established with version 2.</skos:changeNote>
		<skos:inScheme rdf:resource="http://www.cadastralvocabulary.org/CaLAThe"/>
		<skos:broader rdf:resource="http://www.cadastralvocabulary.org/CaLAThe/Ownership"/>
	</skos:Concept>

	<skos:Concept rdf:about="http://www.cadastralvocabulary.org/CaLAThe/AerialPhotograph">
		<skos:prefLabel xml:lang="en">Aerial photograph</skos:prefLabel>
		<skos:prefLabel xml:lang="da">Luftfoto</skos:prefLabel>
		<skos:prefLabel xml:lang="tr">Hava fotoğrafı</skos:prefLabel>
		<skos:prefLabel xml:lang="ms">Foto udara</skos:prefLabel>
		<skos:scopeNote>GEMET term</skos:scopeNote>
		<skos:definition>An image of the ground surface made on a light-sensitive material and taken at a high altitude from an aircraft, spacecraft or rocket (Source: GEMET).</skos:definition>
		<skos:changeNote>Established with version 1.</skos:changeNote>
		<skos:exactMatch rdf:resource="http://aims.fao.org/aos/agrovoc/c_be37a91c"/>
		<skos:inScheme rdf:resource="http://www.cadastralvocabulary.org/CaLAThe"/>
		<skos:broader rdf:resource="http://www.cadastralvocabulary.org/CaLAThe/DigitalImagery"/>
	</skos:Concept>

	<skos:Concept rdf:about="http://www.cadastralvocabulary.org/CaLAThe/Amalgamation">
		<skos:prefLabel xml:lang="en">Amalgamation</skos:prefLabel>
		<skos:prefLabel xml:lang="da">Sammenlægning</skos:prefLabel>
		<skos:prefLabel xml:lang="tr">Birleştirme</skos:prefLabel>
		<skos:prefLabel xml:lang="ms">Cantuman</skos:prefLabel>
		<skos:definition>Activity that combines two or more neighbouring Cadastral parcels.</skos:definition>
		<skos:changeNote>Established with version 2.</skos:changeNote>
		<skos:inScheme rdf:resource="http://www.cadastralvocabulary.org/CaLAThe"/>
		<skos:broader rdf:resource="http://www.cadastralvocabulary.org/CaLAThe/PropertyFormation"/>
	</skos:Concept>

	<skos:Concept rdf:about="http://www.cadastralvocabulary.org/CaLAThe/AngelObservation">
		<skos:prefLabel xml:lang="en">Angle observation</skos:prefLabel>
		<skos:prefLabel xml:lang="da">Vinkelobservation</skos:prefLabel>
		<skos:prefLabel xml:lang="tr">Açı gözlemi</skos:prefLabel>
		<skos:prefLabel xml:lang="ms">Sudut pemerhatian</skos:prefLabel>
		<skos:changeNote>Established with version 4</skos:changeNote>
		<skos:inScheme rdf:resource="http://www.cadastralvocabulary.org/CaLAThe"/>
		<skos:broader rdf:resource="http://www.cadastralvocabulary.org/CaLAThe/Observation"/>
		<skos:broader rdf:resource="http://www.cadastralvocabulary.org/CaLAThe/Theodolite"/>
	</skos:Concept>

	<skos:Concept rdf:about="http://www.cadastralvocabulary.org/CaLAThe/Association">
		<skos:prefLabel xml:lang="en">Association</skos:prefLabel>
		<skos:prefLabel xml:lang="da">Forening</skos:prefLabel>
		<skos:prefLabel xml:lang="tr">Birlik</skos:prefLabel>
		<skos:prefLabel xml:lang="ms">Persatuan</skos:prefLabel>
		<skos:scopeNote>GEMET term</skos:scopeNote>
		<skos:definition>A body of persons associated for the regulation of a common economic activity by means of a special organization (Source: GEMET).</skos:definition>
		<skos:changeNote>Established with version 1.</skos:changeNote>
		<skos:exactMatch rdf:resource="http://www.eionet.europa.eu/gemet/concept/607"/>
		<skos:exactMatch rdf:resource="http://eurovoc.europa.eu/2944"/>
		<skos:inScheme rdf:resource="http://www.cadastralvocabulary.org/CaLAThe"/>
		<skos:broader rdf:resource="http://www.cadastralvocabulary.org/CaLAThe/Organisation"/>
		<skos:narrower rdf:resource="http://www.cadastralvocabulary.org/CaLAThe/ProfessionalSociety"/>
	</skos:Concept>

	<skos:Concept rdf:about="http://www.cadastralvocabulary.org/CaLAThe/Bank">
		<skos:prefLabel xml:lang="en">Bank</skos:prefLabel>
		<skos:prefLabel xml:lang="da">Bank</skos:prefLabel>
		<skos:prefLabel xml:lang="tr">Banka</skos:prefLabel>
		<skos:prefLabel xml:lang="ms">Bank</skos:prefLabel>
		<skos:scopeNote>ISO LADM term</skos:scopeNote>
		<skos:changeNote>Established with version 1.</skos:changeNote>
		<skos:exactMatch rdf:resource="http://zbw.eu/stw/descriptor/13283-4"/>
		<skos:exactMatch rdf:resource="http://aims.fao.org/aos/agrovoc/c_812"/>
		<skos:exactMatch rdf:resource="http://eurovoc.europa.eu/4738"/>
		<skos:inScheme rdf:resource="http://www.cadastralvocabulary.org/CaLAThe"/>
		<skos:broader rdf:resource="http://www.cadastralvocabulary.org/CaLAThe/Corporation"/>
	</skos:Concept>

	<skos:Concept rdf:about="http://www.cadastralvocabulary.org/CaLAThe/BEString">
		<skos:prefLabel xml:lang="en">BEString</skos:prefLabel>
		<skos:scopeNote>OGC LandInfra / InfraGML term</skos:scopeNote>
		<skos:definition>A one-dimensional geometric string representation, limited to curves of type LineString; CircularString; CompoundCurve constructed from LineStrings, CircularStrings, and/or other CompoundCurves; or MultiCurve of any of the previously specified types. (LandInfra 7.10.7)</skos:definition>
		<skos:changeNote>Established with version 4</skos:changeNote>
		<skos:inScheme rdf:resource="http://www.cadastralvocabulary.org/CaLAThe"/>
		<skos:broader rdf:resource="http://www.cadastralvocabulary.org/CaLAThe/BoundingElement"/>
		<skos:narrower rdf:resource="http://www.cadastralvocabulary.org/CaLAThe/StringType"/>
		<skos:narrower rdf:resource="http://www.cadastralvocabulary.org/CaLAThe/LineString"/>
	</skos:Concept>

	<skos:Concept rdf:about="http://www.cadastralvocabulary.org/CaLAThe/Boundary">
		<skos:prefLabel xml:lang="en">Boundary</skos:prefLabel>
		<skos:prefLabel xml:lang="da">Grænse, Matrikelskel</skos:prefLabel>
		<skos:prefLabel xml:lang="tr">Sınır</skos:prefLabel>
		<skos:prefLabel xml:lang="ms">Sempadan</skos:prefLabel>
		<skos:altLabel>LA_Boundary</skos:altLabel>
		<skos:scopeNote>ISO LADM and OGC LandInfra / InfraGML term</skos:scopeNote>
		<skos:definition>Set that represents the limit of an entity. Note 1 to entry: Boundary is most commonly used in the context of geometry, where the set is a collection of points or a collection of objects that represent those points. In other arenas, the term is used metaphorically to describe the transition between an entity and the rest of its domain of discourse (Source: OGC LandInfra 4.8.3, referring to ISO 19107:2003, 4.4; ISO 19152:2012 4.1.3).</skos:definition>
		<skos:changeNote>Established with version 2. Definition added with version 3.</skos:changeNote>
		<skos:inScheme rdf:resource="http://www.cadastralvocabulary.org/CaLAThe"/>
		<skos:broader rdf:resource="http://www.cadastralvocabulary.org/CaLAThe/LandDivision"/>
		<skos:narrower rdf:resource="http://www.cadastralvocabulary.org/CaLAThe/BoundaryMark"/>
	</skos:Concept>

	<skos:Concept rdf:about="http://www.cadastralvocabulary.org/CaLAThe/BoundaryMark">
		<skos:prefLabel xml:lang="en">Boundary mark</skos:prefLabel>
		<skos:prefLabel xml:lang="da">Skelmærke, Grænsesten</skos:prefLabel>
		<skos:prefLabel xml:lang="tr">Sınır işareti</skos:prefLabel>
		<skos:prefLabel xml:lang="ms">Tanda sempadan</skos:prefLabel>
		<skos:altLabel>Boundary monument</skos:altLabel>
		<skos:definition>Physical object which by its form defines a point on the surface of the Earth, which is stably located, and which is recorded in a statement. It may carry a symbol of authority, which communicates its purpose, e.g. marking of the legal boundary between two Land parcels according to jurisdiction-specific provisions (Source: OGC LandInfra, 4.8.16; 7.10.5.1).</skos:definition>
		<skos:changeNote>Established with version 1. Definition with version 3.</skos:changeNote>
		<skos:inScheme rdf:resource="http://www.cadastralvocabulary.org/CaLAThe"/>
		<skos:broader rdf:resource="http://www.cadastralvocabulary.org/CaLAThe/Boundary"/>
		<skos:broader rdf:resource="http://www.cadastralvocabulary.org/CaLAThe/SurveyMark"/>
		<skos:related rdf:resource="http://www.cadastralvocabulary.org/CaLAThe/CadastralParcel"/>
	</skos:Concept>

	<skos:Concept rdf:about="http://www.cadastralvocabulary.org/CaLAThe/BoundaryRe-measurement">
		<skos:prefLabel xml:lang="en">Boundary re-measurement</skos:prefLabel>
		<skos:prefLabel xml:lang="da">Teknisk ændring</skos:prefLabel>
		<skos:prefLabel xml:lang="tr">Tescile tabi teknik işlemler</skos:prefLabel>
		<skos:prefLabel xml:lang="ms">Pengukuran semula sempadan</skos:prefLabel>
		<skos:definition>Activity which re-establish existing Boundary according to documented location. - Boundary re-measurement presupposes that the location of boundaries concerned is well documented. </skos:definition>
		<skos:changeNote>Established with version 2.</skos:changeNote>
		<skos:inScheme rdf:resource="http://www.cadastralvocabulary.org/CaLAThe"/>
		<skos:broader rdf:resource="http://www.cadastralvocabulary.org/CaLAThe/BoundarySurveyAndMarking"/>
	</skos:Concept>

	<skos:Concept rdf:about="http://www.cadastralvocabulary.org/CaLAThe/BoundaryRectification">
		<skos:prefLabel xml:lang="en">Boundary rectification</skos:prefLabel>
		<skos:prefLabel xml:lang="da">Ejendomsberigtigelse</skos:prefLabel>
		<skos:prefLabel xml:lang="tr">Sınır düzeltmesi</skos:prefLabel>
		<skos:prefLabel xml:lang="ms">Pembetulan sempadan</skos:prefLabel>
		<skos:definition>A Boundary survey and marking conducted for correcting errors in the determined positions of Boundaries.  </skos:definition>
		<skos:changeNote>Established with version 2.</skos:changeNote>
		<skos:inScheme rdf:resource="http://www.cadastralvocabulary.org/CaLAThe"/>
		<skos:broader rdf:resource="http://www.cadastralvocabulary.org/CaLAThe/BoundarySurveyAndMarking"/>
	</skos:Concept>

	<skos:Concept rdf:about="http://www.cadastralvocabulary.org/CaLAThe/BoundarySurveyAndMarking">
		<skos:prefLabel xml:lang="en">Boundary survey and marking</skos:prefLabel>
		<skos:prefLabel xml:lang="da">Afmærkning og indmåling af ske</skos:prefLabel>
		<skos:prefLabel xml:lang="tr">Sınırlandırma ve ölçme</skos:prefLabel>
		<skos:prefLabel xml:lang="ms">Penandaan dan pengukuran sempa</skos:prefLabel>
		<skos:definition>An Activity of placing and surveying Boundary marks representing the location of a Boundary of a Cadastral parcel, and documenting the Activity.</skos:definition>
		<skos:changeNote>Established with version 2.0. Narrower added in version 3. </skos:changeNote>
		<skos:inScheme rdf:resource="http://www.cadastralvocabulary.org/CaLAThe"/>
		<skos:broader rdf:resource="http://www.cadastralvocabulary.org/CaLAThe/Subdivision"/>
		<skos:narrower rdf:resource="http://www.cadastralvocabulary.org/CaLAThe/BoundaryRectification"/>
		<skos:narrower rdf:resource="http://www.cadastralvocabulary.org/CaLAThe/LegalBoundaryDetermination"/>
		<skos:narrower rdf:resource="http://www.cadastralvocabulary.org/CaLAThe/BoundaryRe-measurement"/>
		<skos:narrower rdf:resource="http://www.cadastralvocabulary.org/CaLAThe/SurveyMonumentEstablishment"/>
	</skos:Concept>

	<skos:Concept rdf:about="http://www.cadastralvocabulary.org/CaLAThe/BoundingElement">
		<skos:prefLabel xml:lang="en">Bounding element</skos:prefLabel>
		<skos:prefLabel xml:lang="da">Begrænsende element</skos:prefLabel>
		<skos:prefLabel xml:lang="tr">Sınırlandırıcı eleman</skos:prefLabel>
		<skos:prefLabel xml:lang="ms">Unsur pembatasan</skos:prefLabel>
		<skos:scopeNote>OGC LandInfra / InfraGML term</skos:scopeNote>
		<skos:definition>A Bounding element describe or define all or part of the geometry and location of the a Spatial unit (OGC LandInfra, 7.10.7).</skos:definition>
		<skos:changeNote>Established with version 3.</skos:changeNote>
		<skos:inScheme rdf:resource="http://www.cadastralvocabulary.org/CaLAThe"/>
		<skos:broader rdf:resource="http://www.cadastralvocabulary.org/CaLAThe/SpatialUnit"/>
		<skos:narrower rdf:resource="http://www.cadastralvocabulary.org/CaLAThe/BEString"/>
		<skos:narrower rdf:resource="http://www.cadastralvocabulary.org/CaLAThe/LA_BoundaryFaceString"/>
	</skos:Concept>

	<skos:Concept rdf:about="http://www.cadastralvocabulary.org/CaLAThe/BuildingUsePart">
		<skos:prefLabel xml:lang="en">Building use part</skos:prefLabel>
		<skos:prefLabel xml:lang="da">Ejerlejlighedslod</skos:prefLabel>
		<skos:prefLabel xml:lang="tr">Bina kullanım bölümü</skos:prefLabel>
		<skos:prefLabel xml:lang="ms">Bahagian guna bangunan</skos:prefLabel>
		<skos:altLabel>Building part</skos:altLabel>
		<skos:scopeNote>OGC LandInfra / InfraGML term</skos:scopeNote>
		<skos:definition>Part of a floor of a multi-storage building, subdivided according to management and use by a lawful process (Source: OGC LandInfra, 4.8.2; Compares to ISO 19152:2012 4.1.6 building unit, and to Ifc 5.4.3.51 SpatialZone).</skos:definition>
		<skos:changeNote>Established with version 1. Definition added with version 3.</skos:changeNote>
		<skos:inScheme rdf:resource="http://www.cadastralvocabulary.org/CaLAThe"/>
		<skos:broader rdf:resource="http://www.cadastralvocabulary.org/CaLAThe/Condominium"/>
		<skos:broader rdf:resource="http://www.cadastralvocabulary.org/CaLAThe/CondominiumBuilding"/>
	</skos:Concept>

	<skos:Concept rdf:about="http://www.cadastralvocabulary.org/CaLAThe/Buyer">
		<skos:prefLabel xml:lang="en">Buyer</skos:prefLabel>
		<skos:prefLabel xml:lang="da">Køber</skos:prefLabel>
		<skos:prefLabel xml:lang="tr">Alıcı</skos:prefLabel>
		<skos:prefLabel xml:lang="ms">Pembeli</skos:prefLabel>
		<skos:scopeNote>OGC LandInfra / InfraGML term</skos:scopeNote>
		<skos:changeNote>Established with version 4</skos:changeNote>
		<skos:inScheme rdf:resource="http://www.cadastralvocabulary.org/CaLAThe"/>
		<skos:broader rdf:resource="http://www.cadastralvocabulary.org/CaLAThe/Signatory"/>
	</skos:Concept>

	<skos:Concept rdf:about="http://www.cadastralvocabulary.org/CaLAThe/CadastralAccount">
		<skos:prefLabel xml:lang="en">Cadastral account</skos:prefLabel>
		<skos:prefLabel xml:lang="da">Skematisk redegørelse</skos:prefLabel>
		<skos:prefLabel xml:lang="tr">Tescil bildirimi</skos:prefLabel>
		<skos:prefLabel xml:lang="ms">Akaun kadaster</skos:prefLabel>
		<skos:scopeNote>OGC LandInfra / InfraGML term</skos:scopeNote>
		<skos:definition>Land surveyors account of parcel and boundary changes, with references to pertinent legislation, intended for recording body (land administration agency, cadastral authority) (Source: OGC LandInfra, 7.10.4.1).</skos:definition>
		<skos:changeNote>Established with version 3.</skos:changeNote>
		<skos:inScheme rdf:resource="http://www.cadastralvocabulary.org/CaLAThe"/>
		<skos:broader rdf:resource="http://www.cadastralvocabulary.org/CaLAThe/Document"/>
	</skos:Concept>

	<skos:Concept rdf:about="http://www.cadastralvocabulary.org/CaLAThe/CadastralMap">
		<skos:prefLabel xml:lang="en">Cadastral map</skos:prefLabel>
		<skos:prefLabel xml:lang="da">Matrikelkort</skos:prefLabel>
		<skos:prefLabel xml:lang="tr">Kadastral harita</skos:prefLabel>
		<skos:prefLabel xml:lang="ms">Peta kadaster</skos:prefLabel>
		<skos:scopeNote>UNECE WPLA Guidelines</skos:scopeNote>
		<skos:definition>A map showing land (cadastral) parcel boundaries. Cadastral maps may also show buildings. (Source: UNECE, 2004).</skos:definition>
		<skos:changeNote>Established with version 1. Definition and matches edited with verson 6.</skos:changeNote>
		<skos:inScheme rdf:resource="http://www.cadastralvocabulary.org/CaLAThe"/>
		<skos:closeMatch rdf:resource="http://inspire.ec.europa.eu/featureconcept/CadastralParcel"/>
		<skos:broadMatch rdf:resource="https://agrovoc.fao.org/browse/agrovoc/en/page/c_fdee7675"/>
		<skos:broader rdf:resource="http://www.cadastralvocabulary.org/CaLAThe/Map"/>
		<skos:broader rdf:resource="http://www.cadastralvocabulary.org/CaLAThe/Cadastre"/>
	</skos:Concept>

	<skos:Concept rdf:about="http://www.cadastralvocabulary.org/CaLAThe/CadastralParcel">
		<skos:prefLabel xml:lang="en">Cadastral parcel</skos:prefLabel>
		<skos:prefLabel xml:lang="da">Jordstykke, lod</skos:prefLabel>
		<skos:prefLabel xml:lang="tr">Kadastral parsel</skos:prefLabel>
		<skos:prefLabel xml:lang="ms">Petak kadaster</skos:prefLabel>
		<skos:altLabel>Land parcel</skos:altLabel>
		<skos:altLabel>Parcel</skos:altLabel><skos:scopeNote>INSPIRE theme</skos:scopeNote>
		<skos:definition>Contiguous part of the surface of the Earth, as specified through lawful process (Source: OGC LandInfra / InfraGML, 4.8.11).</skos:definition>
		<skos:changeNote>Established with version 1. Definition and Land parcel alternative term with version 3.</skos:changeNote>
		<skos:exactMatch rdf:resource="http://inspire.ec.europa.eu/featureconcept/CadastralParcel"/>
		<skos:inScheme rdf:resource="http://www.cadastralvocabulary.org/CaLAThe"/>
		<skos:broader rdf:resource="http://www.cadastralvocabulary.org/CaLAThe/RealProperty"/>
		<skos:narrower rdf:resource="http://www.cadastralvocabulary.org/CaLAThe/CarrierParcel"/>
		<skos:narrower rdf:resource="http://www.cadastralvocabulary.org/CaLAThe/MainParcel"/>
		<skos:related rdf:resource="http://www.cadastralvocabulary.org/CaLAThe/BoundaryMark"/>
	</skos:Concept>

	<skos:Concept rdf:about="http://www.cadastralvocabulary.org/CaLAThe/CadastralSurveyDocument">
		<skos:prefLabel xml:lang="en">Cadastral survey document</skos:prefLabel>
		<skos:prefLabel xml:lang="da">Måleblad</skos:prefLabel>
		<skos:prefLabel xml:lang="tr">Ölçü krokisi</skos:prefLabel>
		<skos:prefLabel xml:lang="ms">Dokumen ukur kadaster</skos:prefLabel>
		<skos:definition>Land surveyors account of changes, with references to pertinent legislation, intended for recording body (land administration agency, cadastral authority) (Motivated by OGC LandInfra / InfraGML 7.10.4.1).</skos:definition>
		<skos:changeNote>Established with version 1. Definition added in version 3.</skos:changeNote>
		<skos:inScheme rdf:resource="http://www.cadastralvocabulary.org/CaLAThe"/>
		<skos:broader rdf:resource="http://www.cadastralvocabulary.org/CaLAThe/Document"/>
		<skos:related rdf:resource="http://www.cadastralvocabulary.org/CaLAThe/Registrar"/>
		<skos:related rdf:resource="http://www.cadastralvocabulary.org/CaLAThe/Cadastre"/>
	</skos:Concept>

	<skos:Concept rdf:about="http://www.cadastralvocabulary.org/CaLAThe/CadastralSystem">
		<skos:prefLabel xml:lang="en">Cadastral system</skos:prefLabel>
		<skos:prefLabel xml:lang="da">Matrikel-og tinglysningssystem</skos:prefLabel>
		<skos:prefLabel xml:lang="tr">Kadastral sistem</skos:prefLabel>
		<skos:prefLabel xml:lang="ms">Sistem kadaster</skos:prefLabel>
		<skos:definition>Combination of land register and cadastre (Source: Adopted from https://doi.org/10.1016/S0198-9715(00)00051-X)</skos:definition>
		<skos:changeNote>Established with version 1. With version 6 broader ‘Governmental organisation’ replaced with broader ‘Geographical information system’</skos:changeNote>
		<skos:inScheme rdf:resource="http://www.cadastralvocabulary.org/CaLAThe"/>
		<skos:broader rdf:resource="http://www.cadastralvocabulary.org/CaLAThe/GeographicInformationSystem"/>
		<skos:narrower rdf:resource="http://www.cadastralvocabulary.org/CaLAThe/Cadastre"/>
		<skos:narrower rdf:resource="http://www.cadastralvocabulary.org/CaLAThe/LandRegistry"/>
	</skos:Concept>

	<skos:Concept rdf:about="http://www.cadastralvocabulary.org/CaLAThe/Cadastre">
		<skos:prefLabel xml:lang="en">Cadastre</skos:prefLabel>
		<skos:prefLabel xml:lang="da">Matrikel, Matrikelregister</skos:prefLabel>
		<skos:prefLabel xml:lang="tr">Kadastro</skos:prefLabel>
		<skos:prefLabel xml:lang="ms">Kadaster</skos:prefLabel>
		<skos:altLabel xml:lang="en">National survey and cadastre</skos:altLabel>
		<skos:scopeNote>UNECE, WPLA: Guidelines, 2004. AGROVOC Multilingual Thesaurus term</skos:scopeNote>
		<skos:definition>A geographic information system that records land parcels. The term includes (i) Juridical cadastre: a register of ownership of parcels of land; (ii) Fiscal cadastre: a register of properties recording their value; (iii) Land-use cadastre: a register of land use; (iv) Multi-purpose cadastre: a register including many attributes of land parcels.(Source: UNECE, WPLA: Guidelines, 2004)</skos:definition>
		<skos:changeNote>Established with version 1. Definition and matches were edited with version 6.</skos:changeNote>
		<skos:closeMatch rdf:resource="https://agrovoc.fao.org/browse/agrovoc/en/page/c_1177"/>
		<skos:inScheme rdf:resource="http://www.cadastralvocabulary.org/CaLAThe"/>
		<skos:broader rdf:resource="http://www.cadastralvocabulary.org/CaLAThe/CadastralSystem"/>
		<skos:broader rdf:resource="http://www.cadastralvocabulary.org/CaLAThe/Registry"/>
		<skos:narrower rdf:resource="http://www.cadastralvocabulary.org/CaLAThe/CadastralMap"/>
	</skos:Concept>

	<skos:Concept rdf:about="http://www.cadastralvocabulary.org/CaLAThe/Camera">
		<skos:prefLabel xml:lang="en">Camera</skos:prefLabel>
		<skos:prefLabel xml:lang="da">Kamera</skos:prefLabel>
		<skos:prefLabel xml:lang="tr">Kamera</skos:prefLabel>
		<skos:prefLabel xml:lang="ms">Kamera</skos:prefLabel>
		<skos:changeNote>Established with version 4</skos:changeNote>
		<skos:inScheme rdf:resource="http://www.cadastralvocabulary.org/CaLAThe"/>
		<skos:broader rdf:resource="http://www.cadastralvocabulary.org/CaLAThe/SurveyingInstrument"/>
		<skos:narrower rdf:resource="http://www.cadastralvocabulary.org/CaLAThe/Image"/>
	</skos:Concept>

	<skos:Concept rdf:about="http://www.cadastralvocabulary.org/CaLAThe/CarrierParcel">
		<skos:prefLabel xml:lang="en">Carrier parcel</skos:prefLabel>
		<skos:prefLabel xml:lang="da">Reference-parcel</skos:prefLabel>
		<skos:prefLabel xml:lang="tr">Yüklü parsel</skos:prefLabel>
		<skos:prefLabel xml:lang="ms">Petak pembawa</skos:prefLabel>
		<skos:scopeNote>OGC LandInfra / InfraGML term</skos:scopeNote>
		<skos:definition>Land parcel on which a condominium building is located or which carries a superficies, that is a building or construction, established and owned by a person on land leased from another person (Source: OGC LandInfra, 7.10.2.4).</skos:definition>
		<skos:changeNote>Established with version 3.</skos:changeNote>
		<skos:inScheme rdf:resource="http://www.cadastralvocabulary.org/CaLAThe"/>
		<skos:broader rdf:resource="http://www.cadastralvocabulary.org/CaLAThe/CadastralParcel"/>
		<skos:related rdf:resource="http://www.cadastralvocabulary.org/CaLAThe/CondominiumBuilding"/>
		<skos:related rdf:resource="http://www.cadastralvocabulary.org/CaLAThe/SuperficieObject"/>
	</skos:Concept>

	<skos:Concept rdf:about="http://www.cadastralvocabulary.org/CaLAThe/Certificate">
		<skos:prefLabel xml:lang="en">Certificate</skos:prefLabel>
		<skos:prefLabel xml:lang="da">Certifikat</skos:prefLabel>
		<skos:prefLabel xml:lang="tr">Sertifika</skos:prefLabel>
		<skos:prefLabel xml:lang="ms">Sijil</skos:prefLabel>
		<skos:changeNote>Established with version 1.</skos:changeNote>
		<skos:inScheme rdf:resource="http://www.cadastralvocabulary.org/CaLAThe"/>
		<skos:broader rdf:resource="http://www.cadastralvocabulary.org/CaLAThe/Document"/>
		<skos:narrower rdf:resource="http://www.cadastralvocabulary.org/CaLAThe/PropertyEnquiryCertificate"/>
	</skos:Concept>

	<skos:Concept rdf:about="http://www.cadastralvocabulary.org/CaLAThe/ChangeOfPropertyUnitType">
		<skos:prefLabel xml:lang="en">Change of property unit type</skos:prefLabel>
		<skos:prefLabel xml:lang="da">Ændring af ejendomstype</skos:prefLabel>
		<skos:prefLabel xml:lang="tr">Cins değişikliği</skos:prefLabel>
		<skos:prefLabel xml:lang="ms">Perubahan jenis unit harta</skos:prefLabel>
		<skos:definition>An Activity leading to a change in the registered type of Real property.</skos:definition>
		<skos:changeNote>Established with version 2.</skos:changeNote>
		<skos:inScheme rdf:resource="http://www.cadastralvocabulary.org/CaLAThe"/>
		<skos:broader rdf:resource="http://www.cadastralvocabulary.org/CaLAThe/PropertyFormation"/>
		<skos:narrower rdf:resource="http://www.cadastralvocabulary.org/CaLAThe/CondominiumSubdivision"/>
	</skos:Concept>

	<skos:Concept rdf:about="http://www.cadastralvocabulary.org/CaLAThe/Chief">
		<skos:prefLabel xml:lang="en">Chief</skos:prefLabel>
		<skos:prefLabel xml:lang="da">Høvding</skos:prefLabel>
		<skos:prefLabel xml:lang="tr">Şef</skos:prefLabel>
		<skos:prefLabel xml:lang="ms">Ketua</skos:prefLabel>
		<skos:scopeNote>ISO LADM term</skos:scopeNote>
		<skos:definition>A Natural person who is the leader of a Social group, such as Tribe. </skos:definition>
		<skos:changeNote>Established with version 1. Definition is added with version 6.</skos:changeNote>
		<skos:inScheme rdf:resource="http://www.cadastralvocabulary.org/CaLAThe"/>
		<skos:broader rdf:resource="http://www.cadastralvocabulary.org/CaLAThe/SocietalRole"/>
	</skos:Concept>

	<skos:Concept rdf:about="http://www.cadastralvocabulary.org/CaLAThe/CoOwnership">
		<skos:prefLabel xml:lang="en">Co-ownership</skos:prefLabel>
		<skos:prefLabel xml:lang="da">Sameje</skos:prefLabel>
		<skos:prefLabel xml:lang="tr">Paylı mülkiyet</skos:prefLabel>
		<skos:prefLabel xml:lang="ms">Pemilikan bersama</skos:prefLabel>
		<skos:altLabel>Shared ownership</skos:altLabel>
		<skos:definition>Divided or undivided concurrent ownership exercised towards a property (Source: Legal Dictionary of Property in Canada - Dualjuridik). Where two or more people own the same property (Source: EULIS / ELRA glossary).</skos:definition>
		<skos:changeNote>Replaced to Shared ownership in version 3.</skos:changeNote>
		<skos:inScheme rdf:resource="http://www.cadastralvocabulary.org/CaLAThe"/>
		<skos:broader rdf:resource="http://www.cadastralvocabulary.org/CaLAThe/Ownership"/>
		<skos:narrower rdf:resource="http://www.cadastralvocabulary.org/CaLAThe/CondominiumRight"/>
		<skos:narrower rdf:resource="http://www.cadastralvocabulary.org/CaLAThe/TimeshareRight"/>
		<skos:narrower rdf:resource="http://www.cadastralvocabulary.org/CaLAThe/CoOwnershipShare"/>
		<skos:narrower rdf:resource="http://www.cadastralvocabulary.org/CaLAThe/RightOfSuperficie"/>
	</skos:Concept>

	<skos:Concept rdf:about="http://www.cadastralvocabulary.org/CaLAThe/CoOwnershipShare">
		<skos:prefLabel xml:lang="en">Co-ownership share</skos:prefLabel>
		<skos:prefLabel xml:lang="da">Andel i fælleseje</skos:prefLabel>
		<skos:prefLabel xml:lang="tr">Mülkiyet payı</skos:prefLabel>
		<skos:prefLabel xml:lang="ms">Syer pemilikan bersama</skos:prefLabel>
		<skos:changeNote>Established with version 3.</skos:changeNote>
		<skos:inScheme rdf:resource="http://www.cadastralvocabulary.org/CaLAThe"/>
		<skos:broader rdf:resource="http://www.cadastralvocabulary.org/CaLAThe/CoOwnership"/>
		<skos:narrower rdf:resource="http://www.cadastralvocabulary.org/CaLAThe/PartyShare"/>
		<skos:narrower rdf:resource="http://www.cadastralvocabulary.org/CaLAThe/CondominiumShare"/>
	</skos:Concept>

	<skos:Concept rdf:about="http://www.cadastralvocabulary.org/CaLAThe/CodeList">
		<skos:prefLabel xml:lang="en">Code list</skos:prefLabel>
		<skos:prefLabel xml:lang="da">Kodeliste</skos:prefLabel>
		<skos:prefLabel xml:lang="tr">Kod listesi</skos:prefLabel>
		<skos:prefLabel xml:lang="ms">Senarai kod</skos:prefLabel>
		<skos:scopeNote>ISO 19136</skos:scopeNote>
		<skos:definition>(1) Value domain including a code for each permissible value (Geolexica; ISO 19136-1:2020, (E), 3.1.7) (2) Complete set of data element values of a coded simple data element (ADMS Controlled Vocabularies ISO 9735-1:2002, 4.14) - A code list is identified by a name and comprises a set of values</skos:definition>
		<skos:changeNote>Added with version 5. Updated ISO reference and added exact match with version 6</skos:changeNote>
		<skos:exactMatch rdf:resource="https://isotc211.geolexica.org/concepts/50/"/>
		<skos:inScheme rdf:resource="http://www.cadastralvocabulary.org/CaLAThe"/>
		<skos:broader rdf:resource="http://www.cadastralvocabulary.org/CaLAThe/Information"/>
		<skos:narrower rdf:resource="http://www.cadastralvocabulary.org/CaLAThe/UserDefinedValue"/>
	</skos:Concept>

	<skos:Concept rdf:about="http://www.cadastralvocabulary.org/CaLAThe/CollectiveOwnership">
		<skos:prefLabel xml:lang="en">Collective ownership</skos:prefLabel>
		<skos:prefLabel xml:lang="da">Ejendomsfællesskab</skos:prefLabel>
		<skos:prefLabel xml:lang="tr">Birlikte mülkiyet</skos:prefLabel>
		<skos:prefLabel xml:lang="ms">Pemilikan kolektif</skos:prefLabel>
		<skos:changeNote>Established with version 3.</skos:changeNote>
		<skos:exactMatch rdf:resource="http://aims.fao.org/aos/agrovoc/c_29157"/>
		<skos:inScheme rdf:resource="http://www.cadastralvocabulary.org/CaLAThe"/>
		<skos:broader rdf:resource="http://www.cadastralvocabulary.org/CaLAThe/CustomaryLaw"/>
	</skos:Concept>

	<skos:Concept rdf:about="http://www.cadastralvocabulary.org/CaLAThe/Compass">
		<skos:prefLabel xml:lang="en">Compass</skos:prefLabel>
		<skos:prefLabel xml:lang="da">Kompas</skos:prefLabel>
		<skos:prefLabel xml:lang="tr">Pusula</skos:prefLabel>
		<skos:prefLabel xml:lang="ms">Kompas</skos:prefLabel>
		<skos:scopeNote>OGC LandInfra / InfraGML term</skos:scopeNote>
		<skos:changeNote>Established with version 4</skos:changeNote>
		<skos:inScheme rdf:resource="http://www.cadastralvocabulary.org/CaLAThe"/>
		<skos:broader rdf:resource="http://www.cadastralvocabulary.org/CaLAThe/SurveyingInstrument"/>
	</skos:Concept>

	<skos:Concept rdf:about="http://www.cadastralvocabulary.org/CaLAThe/Condominium">
		<skos:prefLabel xml:lang="en">Condominium</skos:prefLabel>
		<skos:prefLabel xml:lang="da">Ejerlejlighed, ej.hedskompleks</skos:prefLabel>
		<skos:prefLabel xml:lang="tr">Bağımsız bölüm</skos:prefLabel>
		<skos:prefLabel xml:lang="ms">Kondominium</skos:prefLabel>
		<skos:altLabel>Condominium unit</skos:altLabel>
		<skos:scopeNote>OGC LandInfra / InfraGML term</skos:scopeNote>
		<skos:definition>Concurrent ownership of real property that has been divided into private and common portions (Legal Dictionary of Property in Canada - Dualjuridik). Note 1 to entry: Condominium unit owners must be members of a mandatory owners  association and engage in the maintenance of joint facilities according to a specified share (Source: OGC LandInfra, 4.8.4).</skos:definition>
		<skos:changeNote>Established with version 3.</skos:changeNote>
		<skos:inScheme rdf:resource="http://www.cadastralvocabulary.org/CaLAThe"/>
		<skos:broader rdf:resource="http://www.cadastralvocabulary.org/CaLAThe/RealProperty"/>
		<skos:narrower rdf:resource="http://www.cadastralvocabulary.org/CaLAThe/BuildingUsePart"/>
		<skos:related rdf:resource="http://www.cadastralvocabulary.org/CaLAThe/CondominiumRight"/>
		<skos:related rdf:resource="http://www.cadastralvocabulary.org/CaLAThe/CondominiumScheme"/>
	</skos:Concept>

	<skos:Concept rdf:about="http://www.cadastralvocabulary.org/CaLAThe/CondominiumAcquisition">
		<skos:prefLabel xml:lang="en">Condominium acquisition</skos:prefLabel>
		<skos:prefLabel xml:lang="da">Erhvervelse af ejerlejlighed</skos:prefLabel>
		<skos:prefLabel xml:lang="tr">Bağımsız bölüm edinimi</skos:prefLabel>
		<skos:prefLabel xml:lang="ms">Pengambilan kondominium</skos:prefLabel>
		<skos:scopeNote>OGC LandInfra / InfraGML term</skos:scopeNote>
		<skos:definition>Conveyance of a Condominium unit, where seller is either the Owner of the original Real property or the owner of a Condominium unit (Source: OGC LandInfra, 7.10.4.1).</skos:definition>
		<skos:changeNote>Established with version 3.</skos:changeNote>
		<skos:inScheme rdf:resource="http://www.cadastralvocabulary.org/CaLAThe"/>
		<skos:broader rdf:resource="http://www.cadastralvocabulary.org/CaLAThe/Conveyance"/>
	</skos:Concept>

	<skos:Concept rdf:about="http://www.cadastralvocabulary.org/CaLAThe/CondominiumBuilding">
		<skos:prefLabel xml:lang="en">Condominium building</skos:prefLabel>
		<skos:prefLabel xml:lang="da">Bygning, opdelt i ejerlejlighe</skos:prefLabel>
		<skos:prefLabel xml:lang="tr">Kat mülkiyetine konu bina</skos:prefLabel>
		<skos:prefLabel xml:lang="ms">Bangunan kondominium</skos:prefLabel>
		<skos:scopeNote>OGC LandInfra / InfraGML term</skos:scopeNote>
		<skos:definition>A Building containing Condominium units subject to a single CondominiumScheme (Source: OGC LandInfra, 7.11.3).</skos:definition>
		<skos:changeNote>Established with version 3.</skos:changeNote>
		<skos:inScheme rdf:resource="http://www.cadastralvocabulary.org/CaLAThe"/>
		<skos:broader rdf:resource="http://www.cadastralvocabulary.org/CaLAThe/Construction"/>
		<skos:narrower rdf:resource="http://www.cadastralvocabulary.org/CaLAThe/BuildingUsePart"/>
		<skos:narrower rdf:resource="http://www.cadastralvocabulary.org/CaLAThe/LA_LegalSpaceBuildingUnit"/>
		<skos:related rdf:resource="http://www.cadastralvocabulary.org/CaLAThe/CarrierParcel"/>
	</skos:Concept>

	<skos:Concept rdf:about="http://www.cadastralvocabulary.org/CaLAThe/CondominiumRight">
		<skos:prefLabel xml:lang="en">Condominium right</skos:prefLabel>
		<skos:prefLabel xml:lang="da">Ejerlejlighedsadkomst</skos:prefLabel>
		<skos:prefLabel xml:lang="tr">Kat mülkiyeti</skos:prefLabel>
		<skos:prefLabel xml:lang="ms">Hak kondominium</skos:prefLabel>
		<skos:altLabel>Apartment ownership</skos:altLabel>
		<skos:definition>Type of co-ownership right.</skos:definition>
		<skos:changeNote>Established with version 1, changed and defined with version 3.</skos:changeNote>
		<skos:inScheme rdf:resource="http://www.cadastralvocabulary.org/CaLAThe"/>
		<skos:broader rdf:resource="http://www.cadastralvocabulary.org/CaLAThe/CoOwnership"/>
		<skos:related rdf:resource="http://www.cadastralvocabulary.org/CaLAThe/Condominium"/>
	</skos:Concept>

	<skos:Concept rdf:about="http://www.cadastralvocabulary.org/CaLAThe/CondominiumScheme">
		<skos:prefLabel xml:lang="en">Condominium scheme</skos:prefLabel>
		<skos:prefLabel xml:lang="da">Ejerlejlighedsfortegnelse mv</skos:prefLabel>
		<skos:prefLabel xml:lang="tr">Bağımsız bölüm listesi</skos:prefLabel>
		<skos:prefLabel xml:lang="ms">Skim kondominium</skos:prefLabel>
		<skos:scopeNote>OGC LandInfra / InfraGML term</skos:scopeNote>
		<skos:definition>Documentation of interest in land in terms of a statement concerning the building parts which make up a number of condominium units and the share of joint facilities of each condominium unit (Source: OGC LandInfra, 4.8.5).</skos:definition>
		<skos:changeNote>Established with version 3.</skos:changeNote>
		<skos:inScheme rdf:resource="http://www.cadastralvocabulary.org/CaLAThe"/>
		<skos:broader rdf:resource="http://www.cadastralvocabulary.org/CaLAThe/Document"/>
	</skos:Concept>

	<skos:Concept rdf:about="http://www.cadastralvocabulary.org/CaLAThe/CondominiumShare">
		<skos:prefLabel xml:lang="en">Condominium share</skos:prefLabel>
		<skos:prefLabel xml:lang="da">Fordelingstal</skos:prefLabel>
		<skos:prefLabel xml:lang="tr">Arsa payı</skos:prefLabel>
		<skos:prefLabel xml:lang="ms">Syer kondominium</skos:prefLabel>
		<skos:changeNote>Established with version 3.</skos:changeNote>
		<skos:inScheme rdf:resource="http://www.cadastralvocabulary.org/CaLAThe"/>
		<skos:broader rdf:resource="http://www.cadastralvocabulary.org/CaLAThe/CoOwnershipShare"/>
	</skos:Concept>

	<skos:Concept rdf:about="http://www.cadastralvocabulary.org/CaLAThe/CondominiumSubdivision">
		<skos:prefLabel xml:lang="en">Condominium subdivision</skos:prefLabel>
		<skos:prefLabel xml:lang="da">Opdeling i ejerlejligheder</skos:prefLabel>
		<skos:prefLabel xml:lang="tr">Bağımsız bölüm ifrazı</skos:prefLabel>
		<skos:prefLabel xml:lang="ms">Pecah bahagi kondominium</skos:prefLabel>
		<skos:scopeNote>OGC LandInfra / InfraGML term</skos:scopeNote>
		<skos:definition>A Subdivision of a multi-storage building into ownership units through a Condominium scheme, which for each unit specifies one or more Building use parts and a Co-ownership share in the joint facilities (Source: OGC LandInfra, 7.10.4.1).</skos:definition>
		<skos:changeNote>Established with version 2. Definition added with version 3.</skos:changeNote>
		<skos:inScheme rdf:resource="http://www.cadastralvocabulary.org/CaLAThe"/>
		<skos:broader rdf:resource="http://www.cadastralvocabulary.org/CaLAThe/Subdivision"/>
		<skos:broader rdf:resource="http://www.cadastralvocabulary.org/CaLAThe/ChangeOfPropertyUnitType"/>
	</skos:Concept>

	<skos:Concept rdf:about="http://www.cadastralvocabulary.org/CaLAThe/Construction">
		<skos:prefLabel xml:lang="en">Construction</skos:prefLabel>
		<skos:prefLabel xml:lang="da">Teknisk anlæg</skos:prefLabel>
		<skos:prefLabel xml:lang="tr">Yapı</skos:prefLabel>
		<skos:prefLabel xml:lang="ms">Pembinaan</skos:prefLabel>
		<skos:altLabel>Building</skos:altLabel>
		<skos:scopeNote>OGC LandInfra / InfraGML term</skos:scopeNote>
		<skos:definition>Assembled or complete part of construction works that results from work on-site [ISO 6707-1:2014] (Source: OGC LandInfra, 4.2.4).</skos:definition>
		<skos:changeNote>Established with version 3.</skos:changeNote>
		<skos:inScheme rdf:resource="http://www.cadastralvocabulary.org/CaLAThe"/>
		<skos:broader rdf:resource="http://www.cadastralvocabulary.org/CaLAThe/TopographicalFeature"/>
		<skos:narrower rdf:resource="http://www.cadastralvocabulary.org/CaLAThe/CondominiumBuilding"/>
		<skos:narrower rdf:resource="http://www.cadastralvocabulary.org/CaLAThe/SuperficieObject"/>
	</skos:Concept>

	<skos:Concept rdf:about="http://www.cadastralvocabulary.org/CaLAThe/ControlPointMonument">
		<skos:prefLabel xml:lang="en">Control point monument</skos:prefLabel>
		<skos:prefLabel xml:lang="da">Fikspunktmærke</skos:prefLabel>
		<skos:prefLabel xml:lang="tr">Kontrol noktası tesisi</skos:prefLabel>
		<skos:prefLabel xml:lang="ms">Monumen titik kawalan</skos:prefLabel>
		<skos:altLabel>Survey monument</skos:altLabel>
		<skos:changeNote>Established with version 1.</skos:changeNote>
		<skos:inScheme rdf:resource="http://www.cadastralvocabulary.org/CaLAThe"/>
		<skos:broader rdf:resource="http://www.cadastralvocabulary.org/CaLAThe/SurveyMark"/>
	</skos:Concept>

	<skos:Concept rdf:about="http://www.cadastralvocabulary.org/CaLAThe/Conveyance">
		<skos:prefLabel xml:lang="en">Conveyance</skos:prefLabel>
		<skos:prefLabel xml:lang="da">Overdragelse </skos:prefLabel>
		<skos:prefLabel xml:lang="tr">Devir</skos:prefLabel>
		<skos:prefLabel xml:lang="ms">Pemindahhakkan</skos:prefLabel>
		<skos:altLabel>Sale</skos:altLabel>
		<skos:altLabel>Purchase</skos:altLabel>
		<skos:definition>An Exchange of Ownership between a Buyer and Seller.</skos:definition>
		<skos:changeNote>Established with version 2.</skos:changeNote>
		<skos:inScheme rdf:resource="http://www.cadastralvocabulary.org/CaLAThe"/>
		<skos:broader rdf:resource="http://www.cadastralvocabulary.org/CaLAThe/Exchange"/>
		<skos:narrower rdf:resource="http://www.cadastralvocabulary.org/CaLAThe/CondominiumAcquisition"/>
		<skos:narrower rdf:resource="http://www.cadastralvocabulary.org/CaLAThe/ParcelAcquisition"/>
	</skos:Concept>

	<skos:Concept rdf:about="http://www.cadastralvocabulary.org/CaLAThe/Coordinate">
		<skos:prefLabel xml:lang="en">Coordinate</skos:prefLabel>
		<skos:prefLabel xml:lang="da">Koordinat</skos:prefLabel>
		<skos:prefLabel xml:lang="tr">Koordinat</skos:prefLabel>
		<skos:prefLabel xml:lang="ms">Koordinat</skos:prefLabel>
		<skos:definition>One of a sequence of numbers designating the position of a point. Note to entry: In a coordinate reference system, the coordinate numbers are qualified by units. (Geolexica, ISO 19111:2019, (E), 3.1.5)</skos:definition>
		<skos:changeNote>Established with version 4</skos:changeNote>
		<skos:exactMatch rdf:resource="https://isotc211.geolexica.org/concepts/2038/"/>
		<skos:inScheme rdf:resource="http://www.cadastralvocabulary.org/CaLAThe"/>
		<skos:broader rdf:resource="http://www.cadastralvocabulary.org/CaLAThe/CoordinateReferenceSystem"/>
	</skos:Concept>

	<skos:Concept rdf:about="http://www.cadastralvocabulary.org/CaLAThe/CoordinateReferenceSystem">
		<skos:prefLabel xml:lang="en">Coordinate reference system</skos:prefLabel>
		<skos:prefLabel xml:lang="da">Koordinatreferencesystem</skos:prefLabel>
		<skos:prefLabel xml:lang="tr">Koordinat referans sistemi</skos:prefLabel>
		<skos:prefLabel xml:lang="ms">Sistem rujukan koordinat</skos:prefLabel>
		<skos:scopeNote>INSPIRE term</skos:scopeNote>
		<skos:definition>(1) Systems for uniquely referencing spatial information in space as a set of coordinates (x, y, z) and/or latitude and longitude and height, based on a geodetic horizontal and vertical datum (Source: INSPIRE glossary). (2) Coordinate system that is related to an object by a datum (Source: ISO 19111:2019, (E), 3.1.9).</skos:definition>
		<skos:changeNote>Established with version 1.</skos:changeNote>
		<skos:exactMatch rdf:resource="http://inspire.ec.europa.eu/glossary/CRS"/>
		<skos:exactMatch rdf:resource="https://isotc211.geolexica.org/concepts/703/"/>
		<skos:inScheme rdf:resource="http://www.cadastralvocabulary.org/CaLAThe"/>
		<skos:broader rdf:resource="http://www.cadastralvocabulary.org/CaLAThe/SpatialReference"/>
		<skos:narrower rdf:resource="http://www.cadastralvocabulary.org/CaLAThe/Coordinate"/>
		<skos:narrower rdf:resource="http://www.cadastralvocabulary.org/CaLAThe/Datum"/>
		<skos:narrower rdf:resource="http://www.cadastralvocabulary.org/CaLAThe/CoordinateTuple"/>
	</skos:Concept>

	<skos:Concept rdf:about="http://www.cadastralvocabulary.org/CaLAThe/CoordinateTuple">
		<skos:prefLabel xml:lang="en">Coordinate tuple</skos:prefLabel>
		<skos:prefLabel xml:lang="da">Koordinat tupel</skos:prefLabel>
		<skos:prefLabel xml:lang="tr">Koordinat üçlüsü</skos:prefLabel>
		<skos:prefLabel xml:lang="ms">Tupel koordinat</skos:prefLabel>
		<skos:scopeNote>ISO 19111,Geolexica term</skos:scopeNote>
		<skos:definition>Tuple composed of coordinates. Note: The number of coordinates in the coordinate tuple equals the dimension of the coordinate system; the order of coordinates in the coordinate tuple is identical to the order of the axes of the coordinate system. (ISO 19111:2019, (E), 3.1.13)</skos:definition>
		<skos:changeNote>Established with version 4</skos:changeNote>
		<skos:exactMatch rdf:resource="https://isotc211.geolexica.org/concepts/2355/"/>
		<skos:inScheme rdf:resource="http://www.cadastralvocabulary.org/CaLAThe"/>
		<skos:broader rdf:resource="http://www.cadastralvocabulary.org/CaLAThe/CoordinateReferenceSystem"/>
	</skos:Concept>

	<skos:Concept rdf:about="http://www.cadastralvocabulary.org/CaLAThe/Corporation">
		<skos:prefLabel xml:lang="en">Corporation</skos:prefLabel>
		<skos:prefLabel xml:lang="da">Virksomhed, Aktieselskab</skos:prefLabel>
		<skos:prefLabel xml:lang="tr">İşletme </skos:prefLabel>
		<skos:prefLabel xml:lang="ms">Perbadanan</skos:prefLabel>
		<skos:scopeNote>STW Thesaurus for Economics term</skos:scopeNote>
		<skos:changeNote>Established with version 1.</skos:changeNote>
		<skos:exactMatch rdf:resource="http://zbw.eu/stw/descriptor/12186-0"/>
		<skos:inScheme rdf:resource="http://www.cadastralvocabulary.org/CaLAThe"/>
		<skos:broader rdf:resource="http://www.cadastralvocabulary.org/CaLAThe/Organisation"/>
		<skos:narrower rdf:resource="http://www.cadastralvocabulary.org/CaLAThe/Bank"/>
	</skos:Concept>

	<skos:Concept rdf:about="http://www.cadastralvocabulary.org/CaLAThe/Correction">
		<skos:prefLabel xml:lang="en">Correction</skos:prefLabel>
		<skos:prefLabel xml:lang="da">Korrektion</skos:prefLabel>
		<skos:prefLabel xml:lang="tr">Düzeltme</skos:prefLabel>
		<skos:prefLabel xml:lang="ms">Pembetulan</skos:prefLabel>
		<skos:scopeNote>OGC LandInfra / InfraGML term</skos:scopeNote>
		<skos:definition>Compensation for an estimated systematic effect (Source: ISO/IEC Guide 99:2007, 2.53; ISO/TS 19159-1:2014, 4.5).</skos:definition>
		<skos:changeNote>Established with version 4</skos:changeNote>
		<skos:inScheme rdf:resource="http://www.cadastralvocabulary.org/CaLAThe"/>
		<skos:broader rdf:resource="http://www.cadastralvocabulary.org/CaLAThe/Observation"/>
	</skos:Concept>

	<skos:Concept rdf:about="http://www.cadastralvocabulary.org/CaLAThe/Curve">
		<skos:prefLabel xml:lang="en">Curve</skos:prefLabel>
		<skos:prefLabel xml:lang="da">Kurve</skos:prefLabel>
		<skos:prefLabel xml:lang="tr">Eğri</skos:prefLabel>
		<skos:prefLabel xml:lang="ms">Garisan</skos:prefLabel>
		<skos:scopeNote>Geolexica term</skos:scopeNote>
		<skos:definition>1-dimensional geometric primitive, representing the continuous image of a line. Note to entry: The boundary of a curve is the set of points at either end of the curve. If the curve is a cycle, the two ends are identical, and the curve (if topologically closed) is considered to not have a boundary. The first point is called the start point, and the last is the end point. Connectivity of the curve is guaranteed by the "continuous image of a line" clause. A topological theorem states that a continuous image of a connected set is connected. (Geolexica ISO 19136-1:2020)</skos:definition>
		<skos:changeNote>Established with version 4</skos:changeNote>
		<skos:exactMatch rdf:resource="https://isotc211.geolexica.org/concepts/101/"/>
		<skos:inScheme rdf:resource="http://www.cadastralvocabulary.org/CaLAThe"/>
		<skos:broader rdf:resource="http://www.cadastralvocabulary.org/CaLAThe/GeometricPrimitive"/>
		<skos:broader rdf:resource="http://www.cadastralvocabulary.org/CaLAThe/Polygon"/>
		<skos:narrower rdf:resource="http://www.cadastralvocabulary.org/CaLAThe/LineString"/>
	</skos:Concept>

	<skos:Concept rdf:about="http://www.cadastralvocabulary.org/CaLAThe/CustomaryLaw">
		<skos:prefLabel xml:lang="en">Customary law</skos:prefLabel>
		<skos:prefLabel xml:lang="da">Sædvaneret</skos:prefLabel>
		<skos:prefLabel xml:lang="tr">Geleneksel hukuk</skos:prefLabel>
		<skos:prefLabel xml:lang="ms">Undang-undang adat</skos:prefLabel>
		<skos:altLabel>Informal right</skos:altLabel>
		<skos:altLabel>Indigenous right</skos:altLabel>
		<skos:altLabel>Custom</skos:altLabel>
		<skos:changeNote>Established with version 1. Custom made preferred term with version 3.</skos:changeNote>
		<skos:exactMatch rdf:resource="http://aims.fao.org/aos/agrovoc/c_10222"/>
		<skos:inScheme rdf:resource="http://www.cadastralvocabulary.org/CaLAThe"/>
		<skos:broader rdf:resource="http://www.cadastralvocabulary.org/CaLAThe/Law"/>
		<skos:narrower rdf:resource="http://www.cadastralvocabulary.org/CaLAThe/CollectiveOwnership"/>
	</skos:Concept>

	<skos:Concept rdf:about="http://www.cadastralvocabulary.org/CaLAThe/Datum">
		<skos:prefLabel xml:lang="en">Datum</skos:prefLabel>
		<skos:prefLabel xml:lang="da">Datum</skos:prefLabel>
		<skos:prefLabel xml:lang="tr">Datum</skos:prefLabel>
		<skos:prefLabel xml:lang="ms">Datum, Data tunggal</skos:prefLabel>
		<skos:scopeNote>Geolexica term</skos:scopeNote>
		<skos:definition>Parameter or set of parameters that realize the position of the origin, the scale, and the orientation of a coordinate system (Geolexica; ISO 19111:2019, (E), 3.1.15)</skos:definition>
		<skos:changeNote>Established with version 4</skos:changeNote>
		<skos:exactMatch rdf:resource="https://isotc211.geolexica.org/concepts/2376/"/>
		<skos:inScheme rdf:resource="http://www.cadastralvocabulary.org/CaLAThe"/>
		<skos:broader rdf:resource="http://www.cadastralvocabulary.org/CaLAThe/CoordinateReferenceSystem"/>
	</skos:Concept>

	<skos:Concept rdf:about="http://www.cadastralvocabulary.org/CaLAThe/Deed">
		<skos:prefLabel xml:lang="en">Deed</skos:prefLabel>
		<skos:prefLabel xml:lang="da">Beseglet dokument, Skøde</skos:prefLabel>
		<skos:prefLabel xml:lang="tr">Sözleşme</skos:prefLabel>
		<skos:prefLabel xml:lang="ms">Surat ikatan </skos:prefLabel>
		<skos:scopeNote>Established with version 1.</skos:scopeNote>
		<skos:exactMatch rdf:resource="http://aims.fao.org/aos/agrovoc/c_c10cdeb5"/>
		<skos:exactMatch rdf:resource="http://eurovoc.europa.eu/164"/>
		<skos:inScheme rdf:resource="http://www.cadastralvocabulary.org/CaLAThe"/>
		<skos:broader rdf:resource="http://www.cadastralvocabulary.org/CaLAThe/Document"/>
		<skos:narrower rdf:resource="http://www.cadastralvocabulary.org/CaLAThe/MortgageDeed"/>
		<skos:narrower rdf:resource="http://www.cadastralvocabulary.org/CaLAThe/TitleDeed"/>
		<skos:narrower rdf:resource="http://www.cadastralvocabulary.org/CaLAThe/RestrictionDeed"/>
	</skos:Concept>

	<skos:Concept rdf:about="http://www.cadastralvocabulary.org/CaLAThe/DesignPoint">
		<skos:prefLabel xml:lang="en">Design point</skos:prefLabel>
		<skos:prefLabel xml:lang="da">Designkoordinat</skos:prefLabel>
		<skos:prefLabel xml:lang="ms">Titik reka bentuk</skos:prefLabel>
		<skos:scopeNote>OGC LandInfra / InfraGML term</skos:scopeNote>
		<skos:definition>The point geometry to be staked out (cf. OGC LandInfra 7.8.7.4 and .5).</skos:definition>
		<skos:changeNote>Established with version 4</skos:changeNote>
		<skos:inScheme rdf:resource="http://www.cadastralvocabulary.org/CaLAThe"/>
		<skos:broader rdf:resource="http://www.cadastralvocabulary.org/CaLAThe/GNSSsensor"/>
		<skos:broader rdf:resource="http://www.cadastralvocabulary.org/CaLAThe/TotalStation"/>
		<skos:narrower rdf:resource="http://www.cadastralvocabulary.org/CaLAThe/Stakeout"/>
	</skos:Concept>

	<skos:Concept rdf:about="http://www.cadastralvocabulary.org/CaLAThe/DigitalImagery">
		<skos:prefLabel xml:lang="en">Digital imagery</skos:prefLabel>
		<skos:prefLabel xml:lang="da">Digitalt billedmateriale</skos:prefLabel>
		<skos:prefLabel xml:lang="tr">Sayısal görüntü</skos:prefLabel>
		<skos:prefLabel xml:lang="ms">Imej digital, Pengimejan digi</skos:prefLabel>
		<skos:definition>Raster graphics image</skos:definition>
		<skos:changeNote>Established with version 1. Edited with version 4</skos:changeNote>
		<skos:inScheme rdf:resource="http://www.cadastralvocabulary.org/CaLAThe"/>
		<skos:broader rdf:resource="http://www.cadastralvocabulary.org/CaLAThe/GeolocatedInformation"/>
		<skos:narrower rdf:resource="http://www.cadastralvocabulary.org/CaLAThe/SatelliteImage"/>
		<skos:narrower rdf:resource="http://www.cadastralvocabulary.org/CaLAThe/AerialPhotograph"/>
		<skos:narrower rdf:resource="http://www.cadastralvocabulary.org/CaLAThe/Orthoimagery"/>
	</skos:Concept>

	<skos:Concept rdf:about="http://www.cadastralvocabulary.org/CaLAThe/DimensionType">
		<skos:prefLabel xml:lang="en">Dimension type</skos:prefLabel>
		<skos:prefLabel xml:lang="da">Dimensionstype</skos:prefLabel>
		<skos:prefLabel xml:lang="tr">Boyut türü</skos:prefLabel>
		<skos:prefLabel xml:lang="ms">Jenis dimensi, Jenis ukuran</skos:prefLabel>
		<skos:scopeNote>OGC LandInfra / InfraGML term</skos:scopeNote>
		<skos:changeNote>Established with version 4</skos:changeNote>
		<skos:inScheme rdf:resource="http://www.cadastralvocabulary.org/CaLAThe"/>
		<skos:broader rdf:resource="http://www.cadastralvocabulary.org/CaLAThe/SpatialUnit"/>
		<skos:narrower rdf:resource="http://www.cadastralvocabulary.org/CaLAThe/2D"/>
		<skos:narrower rdf:resource="http://www.cadastralvocabulary.org/CaLAThe/3D"/>
		<skos:narrower rdf:resource="http://www.cadastralvocabulary.org/CaLAThe/Liminal"/>
	</skos:Concept>

	<skos:Concept rdf:about="http://www.cadastralvocabulary.org/CaLAThe/DistanceObservation">
		<skos:prefLabel xml:lang="en">Distance observation</skos:prefLabel>
		<skos:prefLabel xml:lang="da">Afstandsobservation</skos:prefLabel>
		<skos:prefLabel xml:lang="tr">Mesafe gözlemi</skos:prefLabel>
		<skos:prefLabel xml:lang="ms">Jarak pemerhatian, Jarak cerap</skos:prefLabel>
		<skos:scopeNote>OGC LandInfra / InfraGML term</skos:scopeNote>
		<skos:changeNote>Established with version 4</skos:changeNote>
		<skos:inScheme rdf:resource="http://www.cadastralvocabulary.org/CaLAThe"/>
		<skos:broader rdf:resource="http://www.cadastralvocabulary.org/CaLAThe/Observation"/>
		<skos:broader rdf:resource="http://www.cadastralvocabulary.org/CaLAThe/MeasuringTape"/>
		<skos:broader rdf:resource="http://www.cadastralvocabulary.org/CaLAThe/EletronicDistanceMeter"/>
	</skos:Concept>

	<skos:Concept rdf:about="http://www.cadastralvocabulary.org/CaLAThe/Document">
		<skos:prefLabel xml:lang="en">Document</skos:prefLabel>
		<skos:prefLabel xml:lang="da">Dokument</skos:prefLabel>
		<skos:prefLabel xml:lang="tr">Belge</skos:prefLabel>
		<skos:prefLabel xml:lang="ms">Dokumen</skos:prefLabel>
		<skos:altLabel>Statement</skos:altLabel>
		<skos:scopeNote>GEMET term</skos:scopeNote>
		<skos:definition>Material of any kind, regardless of physical form, which furnishes information, evidence or ideas, including items such as contracts, bills of sale, letters, audio and video recordings, and machine readable data files  (Source: GEMET). Information in permanent form which is approved by one or more signatures (Source: OGC LandInfra, 4.1.7, Compares to ISO 19152:2012 4.1.21 source)</skos:definition>
		<skos:changeNote>Established with version 1. Definition edited and alternative term added with version 3.</skos:changeNote>
		<skos:exactMatch rdf:resource="http://www.eionet.europa.eu/gemet/concept/2282"/>
		<skos:exactMatch rdf:resource="http://aims.fao.org/aos/agrovoc/c_4f435f4f"/>
		<skos:exactMatch rdf:resource="http://eurovoc.europa.eu/486"/>
		<skos:inScheme rdf:resource="http://www.cadastralvocabulary.org/CaLAThe"/>
		<skos:broader rdf:resource="http://www.cadastralvocabulary.org/CaLAThe/Information"/>
		<skos:narrower rdf:resource="http://www.cadastralvocabulary.org/CaLAThe/CadastralSurveyDocument"/>
		<skos:narrower rdf:resource="http://www.cadastralvocabulary.org/CaLAThe/Certificate"/>
		<skos:narrower rdf:resource="http://www.cadastralvocabulary.org/CaLAThe/CondominiumScheme"/>
		<skos:narrower rdf:resource="http://www.cadastralvocabulary.org/CaLAThe/SuperficieObjectScheme"/>
		<skos:narrower rdf:resource="http://www.cadastralvocabulary.org/CaLAThe/EasementDeed"/>
		<skos:narrower rdf:resource="http://www.cadastralvocabulary.org/CaLAThe/CadastralAccount"/>
		<skos:narrower rdf:resource="http://www.cadastralvocabulary.org/CaLAThe/LA_Source"/>
		<skos:narrower rdf:resource="http://www.cadastralvocabulary.org/CaLAThe/Deed"/>
		<skos:related rdf:resource="http://www.cadastralvocabulary.org/CaLAThe/Draftsman"/>
	</skos:Concept>

	<skos:Concept rdf:about="http://www.cadastralvocabulary.org/CaLAThe/DominantPropertyUnit">
		<skos:prefLabel xml:lang="en">Dominant property unit</skos:prefLabel>
		<skos:prefLabel xml:lang="da">Herskende ejendom</skos:prefLabel>
		<skos:prefLabel xml:lang="tr">Hakim taşınmaz</skos:prefLabel>
		<skos:prefLabel xml:lang="ms">Unit harta dominan</skos:prefLabel>
		<skos:definition>Land (Property unit) for which a servitude is granted (Source: Legal Dictionary of Property in Canada - Dualjuridik).</skos:definition>
		<skos:changeNote>Established with version 3.</skos:changeNote>
		<skos:inScheme rdf:resource="http://www.cadastralvocabulary.org/CaLAThe"/>
		<skos:broader rdf:resource="http://www.cadastralvocabulary.org/CaLAThe/Easement"/>
	</skos:Concept>

	<skos:Concept rdf:about="http://www.cadastralvocabulary.org/CaLAThe/Draftsman">
		<skos:prefLabel xml:lang="en">Draftsman</skos:prefLabel>
		<skos:prefLabel xml:lang="da">Koncipist</skos:prefLabel>
		<skos:prefLabel xml:lang="ms">Perangka</skos:prefLabel>
		<skos:scopeNote>OGC LandInfra / InfraGML term</skos:scopeNote>
		<skos:definition>A Professional who prepares or drafts Documents.</skos:definition>
		<skos:changeNote>Established as Draftsman in version 3, revised as Drafter in version 5, and changed again as Draftsman in version 6. Definition is added with version 6.</skos:changeNote>
		<skos:inScheme rdf:resource="http://www.cadastralvocabulary.org/CaLAThe"/>
		<skos:broader rdf:resource="http://www.cadastralvocabulary.org/CaLAThe/Professional"/>
		<skos:related rdf:resource="http://www.cadastralvocabulary.org/CaLAThe/Document"/>
	</skos:Concept>

	<skos:Concept rdf:about="http://www.cadastralvocabulary.org/CaLAThe/Easement">
		<skos:prefLabel xml:lang="en">Easement</skos:prefLabel>
		<skos:prefLabel xml:lang="da">Servitut</skos:prefLabel>
		<skos:prefLabel xml:lang="tr">İrtifak hakkı</skos:prefLabel>
		<skos:prefLabel xml:lang="ms">Esmen</skos:prefLabel>
		<skos:scopeNote>GEMET term Compares to ISO LADM 4.1.19 restriction</skos:scopeNote>
		<skos:definition>The rights of use over the property of another; a burden on a piece of land causing the owner to suffer access by another (Source: GEMET). Accessory interest in land which advantages dominant land or other beneficiary (Source: Legal Dictionary of Property in Canada - Dualjuridik; cf. OGC LandInfra, 4.8.6).</skos:definition>
		<skos:changeNote>Established with version 1. Changed with version 3.</skos:changeNote>
		<skos:exactMatch rdf:resource="http://www.eionet.europa.eu/gemet/concept/11536"/>
		<skos:inScheme rdf:resource="http://www.cadastralvocabulary.org/CaLAThe"/>
		<skos:broader rdf:resource="http://www.cadastralvocabulary.org/CaLAThe/LimitedRight"/>
		<skos:narrower rdf:resource="http://www.cadastralvocabulary.org/CaLAThe/PrivateLawRestriction"/>
		<skos:narrower rdf:resource="http://www.cadastralvocabulary.org/CaLAThe/ServientPropertyUnit"/>
		<skos:narrower rdf:resource="http://www.cadastralvocabulary.org/CaLAThe/PublicLawRestriction"/>
		<skos:narrower rdf:resource="http://www.cadastralvocabulary.org/CaLAThe/DominantPropertyUnit"/>
	</skos:Concept>

	<skos:Concept rdf:about="http://www.cadastralvocabulary.org/CaLAThe/EasementCreation">
		<skos:prefLabel xml:lang="en">Easement creation</skos:prefLabel>
		<skos:prefLabel xml:lang="da">Stiftelse af servitut</skos:prefLabel>
		<skos:prefLabel xml:lang="tr">İrtifak hakkı tesisi</skos:prefLabel>
		<skos:prefLabel xml:lang="ms">Penciptaan esmen</skos:prefLabel>
		<skos:definition>An Activity that establishes a nonpossessory right to use and/or enter onto the Real property of another without possessing.</skos:definition>
		<skos:changeNote>Established with version 2. Scope note and relations added with version 3.</skos:changeNote>
		<skos:inScheme rdf:resource="http://www.cadastralvocabulary.org/CaLAThe"/>
		<skos:broader rdf:resource="http://www.cadastralvocabulary.org/CaLAThe/Exchange"/>
		<skos:related rdf:resource="http://www.cadastralvocabulary.org/CaLAThe/DominantPropertyUnit"/>
		<skos:related rdf:resource="http://www.cadastralvocabulary.org/CaLAThe/ServientPropertyUnit"/>
		<skos:related rdf:resource="http://www.cadastralvocabulary.org/CaLAThe/CondominiumScheme"/>
	</skos:Concept>

	<skos:Concept rdf:about="http://www.cadastralvocabulary.org/CaLAThe/EasementDeed">
		<skos:prefLabel xml:lang="en">Easement deed</skos:prefLabel>
		<skos:prefLabel xml:lang="da">Deklaration, Servitutdokument</skos:prefLabel>
		<skos:prefLabel xml:lang="tr">İrtifak hakkı sözleşmesi</skos:prefLabel>
		<skos:prefLabel xml:lang="ms">Surat ikatan esmen</skos:prefLabel>
		<skos:scopeNote>OGC LandInfra / InfraGML term</skos:scopeNote>
		<skos:changeNote>Established with version 3 as Easement scheme, and changed as Easement deed in version 5.</skos:changeNote>
		<skos:inScheme rdf:resource="http://www.cadastralvocabulary.org/CaLAThe"/>
		<skos:broader rdf:resource="http://www.cadastralvocabulary.org/CaLAThe/Document"/>
	</skos:Concept>

	<skos:Concept rdf:about="http://www.cadastralvocabulary.org/CaLAThe/Edge">
		<skos:prefLabel xml:lang="en">Edge</skos:prefLabel>
		<skos:prefLabel xml:lang="da">Kant</skos:prefLabel>
		<skos:prefLabel xml:lang="tr">Kenar</skos:prefLabel>
		<skos:prefLabel xml:lang="ms">Pinggir, Hujung</skos:prefLabel>
		<skos:scopeNote>Geolexica term</skos:scopeNote>
		<skos:definition>1-dimensional topological primitive. Note to entry: The geometric realization of an edge is a curve. The boundary of an edge is the set of one or two nodes associated to the edge within a topological complex. (Geolexica, ISO 19107:2003)</skos:definition>
		<skos:changeNote>Introduced with version 4</skos:changeNote>
		<skos:exactMatch rdf:resource="https://isotc211.geolexica.org/concepts/146/"/>
		<skos:inScheme rdf:resource="http://www.cadastralvocabulary.org/CaLAThe"/>
		<skos:broader rdf:resource="http://www.cadastralvocabulary.org/CaLAThe/TopologicalPrimitive"/>
		<skos:narrower rdf:resource="http://www.cadastralvocabulary.org/CaLAThe/LA_EdgeBasedSpatialUnit"/>
	</skos:Concept>

	<skos:Concept rdf:about="http://www.cadastralvocabulary.org/CaLAThe/EletronicDistanceMeter">
		<skos:prefLabel xml:lang="en">Electronic distance meter</skos:prefLabel>
		<skos:prefLabel xml:lang="da">Elektrooptisk distancemåler</skos:prefLabel>
		<skos:prefLabel xml:lang="tr">Elektronik uzunluk ölçüsü</skos:prefLabel>
		<skos:prefLabel xml:lang="ms">Meter jarak elektronik</skos:prefLabel>
		<skos:scopeNote>OGC LandInfra / InfraGML term</skos:scopeNote>
		<skos:definition>Instrument for directly measuring distances between the instrument and the sighting points, comprising a transmitter and a receiver (OGC LandInfra 4.6.3, referring to ISO 9849-1:2000)</skos:definition>
		<skos:changeNote>Established with version 4</skos:changeNote>
		<skos:inScheme rdf:resource="http://www.cadastralvocabulary.org/CaLAThe"/>
		<skos:broader rdf:resource="http://www.cadastralvocabulary.org/CaLAThe/SurveyingInstrument"/>
		<skos:narrower rdf:resource="http://www.cadastralvocabulary.org/CaLAThe/DistanceObservation"/>
	</skos:Concept>

	<skos:Concept rdf:about="http://www.cadastralvocabulary.org/CaLAThe/Elevation">
		<skos:prefLabel xml:lang="en">Elevation</skos:prefLabel>
		<skos:prefLabel xml:lang="da">Højde</skos:prefLabel>
		<skos:prefLabel xml:lang="tr">Yükseklik</skos:prefLabel>
		<skos:prefLabel xml:lang="ms">Ketinggian</skos:prefLabel>
		<skos:scopeNote>INSPIRE term</skos:scopeNote>
		<skos:definition>Height above sea level.</skos:definition>
		<skos:changeNote>Established with version 1. Definition is added in version 5.</skos:changeNote>
		<skos:inScheme rdf:resource="http://www.cadastralvocabulary.org/CaLAThe"/>
		<skos:broader rdf:resource="http://www.cadastralvocabulary.org/CaLAThe/TopographicalFeature"/>
	</skos:Concept>

	<skos:Concept rdf:about="http://www.cadastralvocabulary.org/CaLAThe/Engineer">
		<skos:prefLabel xml:lang="en">Engineer</skos:prefLabel>
		<skos:prefLabel xml:lang="da">Ingeniør</skos:prefLabel>
		<skos:prefLabel xml:lang="tr">Mühendis</skos:prefLabel>
		<skos:prefLabel xml:lang="ms">Jurutera</skos:prefLabel>
		<skos:definition>A Professional who is trained in a branch of engineering.</skos:definition>
		<skos:changeNote>Established with version 3. Definition is added with version 6.</skos:changeNote>
		<skos:exactMatch rdf:resource="http://eurovoc.europa.eu/1435"/>
		<skos:exactMatch rdf:resource="http://aims.fao.org/aos/agrovoc/c_2573"/>
		<skos:inScheme rdf:resource="http://www.cadastralvocabulary.org/CaLAThe"/>
		<skos:broader rdf:resource="http://www.cadastralvocabulary.org/CaLAThe/Professional"/>
	</skos:Concept>

	<skos:Concept rdf:about="http://www.cadastralvocabulary.org/CaLAThe/Exchange">
		<skos:prefLabel xml:lang="en">Exchange</skos:prefLabel>
		<skos:prefLabel xml:lang="da">Ejendomsdispositioner</skos:prefLabel>
		<skos:prefLabel xml:lang="tr">Devir</skos:prefLabel>
		<skos:prefLabel xml:lang="ms">Pertukaran</skos:prefLabel>
		<skos:definition>The disposal of Real property or Real rights on a value for value basis.</skos:definition>
		<skos:changeNote>Established with version 2.</skos:changeNote>
		<skos:inScheme rdf:resource="http://www.cadastralvocabulary.org/CaLAThe"/>
		<skos:broader rdf:resource="http://www.cadastralvocabulary.org/CaLAThe/Activity"/>
		<skos:narrower rdf:resource="http://www.cadastralvocabulary.org/CaLAThe/Conveyance"/>
		<skos:narrower rdf:resource="http://www.cadastralvocabulary.org/CaLAThe/Lease"/>
		<skos:narrower rdf:resource="http://www.cadastralvocabulary.org/CaLAThe/Rent"/>
		<skos:narrower rdf:resource="http://www.cadastralvocabulary.org/CaLAThe/Mortgaging"/>
		<skos:narrower rdf:resource="http://www.cadastralvocabulary.org/CaLAThe/ForcedSale"/>
		<skos:narrower rdf:resource="http://www.cadastralvocabulary.org/CaLAThe/EasementCreation"/>
	</skos:Concept>

	<skos:Concept rdf:about="http://www.cadastralvocabulary.org/CaLAThe/Expropriation">
		<skos:prefLabel xml:lang="en">Expropriation</skos:prefLabel>
		<skos:prefLabel xml:lang="da">Ekspropriation</skos:prefLabel>
		<skos:prefLabel xml:lang="tr">Kamulaştırma</skos:prefLabel>
		<skos:prefLabel xml:lang="ms">Perampasan, Pengambilalihan</skos:prefLabel>
		<skos:scopeNote>GEMET term</skos:scopeNote>
		<skos:definition>The compulsory depriving of an Owner of Real property in return for compensation because of public interest.</skos:definition>
		<skos:changeNote>Established with version 2.</skos:changeNote>
		<skos:exactMatch rdf:resource="http://aims.fao.org/aos/agrovoc/c_1798"/>
		<skos:exactMatch rdf:resource="https://www.eionet.europa.eu/gemet/en/concept/3071"/>
		<skos:exactMatch rdf:resource="http://eurovoc.europa.eu/948"/>
		<skos:exactMatch rdf:resource="http://zbw.eu/stw/descriptor/11771-1"/>
		<skos:inScheme rdf:resource="http://www.cadastralvocabulary.org/CaLAThe"/>
		<skos:broader rdf:resource="http://www.cadastralvocabulary.org/CaLAThe/PropertyRestructuring"/>
	</skos:Concept>

	<skos:Concept rdf:about="http://www.cadastralvocabulary.org/CaLAThe/Face">
		<skos:prefLabel xml:lang="en">Face</skos:prefLabel>
		<skos:prefLabel xml:lang="da">Flade</skos:prefLabel>
		<skos:prefLabel xml:lang="tr">Yüzey</skos:prefLabel>
		<skos:prefLabel xml:lang="ms">Permukaan, Pandangan</skos:prefLabel>
		<skos:scopeNote>Geolexica term</skos:scopeNote>
		<skos:definition>2-dimensional topological primitive. Note to entry: The geometric realization of a face is a surface. The boundary of a face is the set of directed edges within the same topological complex that are associated to the face via the boundary relations. These can be organized as rings. (Geolexica, ISO 19107:2003)</skos:definition>
		<skos:changeNote>Introduced with version 4</skos:changeNote>
		<skos:exactMatch rdf:resource="https://isotc211.geolexica.org/concepts/165/"/>
		<skos:inScheme rdf:resource="http://www.cadastralvocabulary.org/CaLAThe"/>
		<skos:broader rdf:resource="http://www.cadastralvocabulary.org/CaLAThe/TopologicalPrimitive"/>
		<skos:narrower rdf:resource="http://www.cadastralvocabulary.org/CaLAThe/LA_FaceBasedSpatialUnit"/>
	</skos:Concept>

	<skos:Concept rdf:about="http://www.cadastralvocabulary.org/CaLAThe/Family">
		<skos:prefLabel xml:lang="en">Family</skos:prefLabel>
		<skos:prefLabel xml:lang="da">Familie</skos:prefLabel>
		<skos:prefLabel xml:lang="tr">Aile</skos:prefLabel>
		<skos:prefLabel xml:lang="ms">Keluarga</skos:prefLabel>
		<skos:scopeNote>GEMET term</skos:scopeNote>
		<skos:definition>A group comprising parents, offsprings and others closely related or associated with them (Source: Lincoln, Boxshall and Clark, 1982).</skos:definition>
		<skos:changeNote>Established with version 1. Definition is revised with version 6.</skos:changeNote>
		<skos:exactMatch rdf:resource="http://www.eionet.europa.eu/gemet/concept/3117"/>
		<skos:exactMatch rdf:resource="http://eurovoc.europa.eu/965"/>
		<skos:inScheme rdf:resource="http://www.cadastralvocabulary.org/CaLAThe"/>
		<skos:broader rdf:resource="http://www.cadastralvocabulary.org/CaLAThe/SocialGroup"/>
	</skos:Concept>

	<skos:Concept rdf:about="http://www.cadastralvocabulary.org/CaLAThe/Farmer">
		<skos:prefLabel xml:lang="en">Farmer</skos:prefLabel>
		<skos:prefLabel xml:lang="da">Landmand</skos:prefLabel>
		<skos:prefLabel xml:lang="tr">Çiftçi</skos:prefLabel>
		<skos:prefLabel xml:lang="ms">Petani</skos:prefLabel>
		<skos:scopeNote>ISO LADM term</skos:scopeNote>
		<skos:definition>A Natural person who is engaged in agriculture, cultivating land or crops or raising animals (such as livestock or fish) for food.</skos:definition>
		<skos:changeNote>Established with version 4. Broader is edited with version 5. Definition is added with version 6.</skos:changeNote>
		<skos:exactMatch rdf:resource="http://aims.fao.org/aos/agrovoc/c_2805"/>
		<skos:exactMatch rdf:resource="http://eurovoc.europa.eu/936"/>
		<skos:inScheme rdf:resource="http://www.cadastralvocabulary.org/CaLAThe"/>
		<skos:broader rdf:resource="http://www.cadastralvocabulary.org/CaLAThe/SocietalRole"/>
	</skos:Concept>

	<skos:Concept rdf:about="http://www.cadastralvocabulary.org/CaLAThe/ForcedSale">
		<skos:prefLabel xml:lang="en">Forced sale</skos:prefLabel>
		<skos:prefLabel xml:lang="da">Tvangsauktion</skos:prefLabel>
		<skos:prefLabel xml:lang="tr">Zoraki satış</skos:prefLabel>
		<skos:prefLabel xml:lang="ms">Jualan paksa</skos:prefLabel>
		<skos:altLabel>Foreclosure</skos:altLabel>
		<skos:altLabel>Compulsory purchase</skos:altLabel>
		<skos:altLabel>Repossesion</skos:altLabel>
		<skos:scopeNote>AGROVOC Multilingual Thesaurus term</skos:scopeNote>
		<skos:definition>A sale of Real property under the process of the court against the consent of the Owner.</skos:definition>
		<skos:changeNote>Established with version 2. Close match http://www.eionet.europa.eu/gemet/concept/3401 deleted with version 4</skos:changeNote>
		<skos:exactMatch rdf:resource="http://aims.fao.org/aos/agrovoc/c_15683"/>
		<skos:inScheme rdf:resource="http://www.cadastralvocabulary.org/CaLAThe"/>
		<skos:broader rdf:resource="http://www.cadastralvocabulary.org/CaLAThe/Exchange"/>
	</skos:Concept>

	<skos:Concept rdf:about="http://www.cadastralvocabulary.org/CaLAThe/Gazetteer">
		<skos:prefLabel xml:lang="en">Gazetteer</skos:prefLabel>
		<skos:prefLabel xml:lang="da">Stednavnefortegnelse</skos:prefLabel>
		<skos:prefLabel xml:lang="tr">Yer adları dizini</skos:prefLabel>
		<skos:prefLabel xml:lang="ms">Gazetir</skos:prefLabel>
		<skos:scopeNote>AGROVOC Multilingual Thesaurus term ISO 19112</skos:scopeNote>
		<skos:definition>(1) A vocabulary consisting of identifiers, location descriptions, and attributes for a set of geospatial features (Source: Breitman, Casanova and  Truszkowski, 2007). (2) Register of location instances of one or more location sub-types, containing some information regarding position. Note: The positional information need not be coordinates, but could be descriptive. (Source: ISO 19112:2019, (E), 3.1.1)</skos:definition>
		<skos:changeNote>Established with version 1. ISO definition added with version 6.</skos:changeNote>
		<skos:exactMatch rdf:resource="http://aims.fao.org/aos/agrovoc/c_49853"/>
		<skos:exactMatch rdf:resource="https://isotc211.geolexica.org/concepts/2344/"/>
		<skos:inScheme rdf:resource="http://www.cadastralvocabulary.org/CaLAThe"/>
		<skos:broader rdf:resource="http://www.cadastralvocabulary.org/CaLAThe/SpatialDataInfrastructure"/>
		<skos:narrower rdf:resource="http://www.cadastralvocabulary.org/CaLAThe/PlaceName"/>
	</skos:Concept>

	<skos:Concept rdf:about="http://www.cadastralvocabulary.org/CaLAThe/GeographicInformationSystem">
		<skos:prefLabel xml:lang="en">Geographic information system</skos:prefLabel>
		<skos:prefLabel xml:lang="da">Geografisk informationssystem</skos:prefLabel>
		<skos:prefLabel xml:lang="tr">Coğrafi bilgi sistemi</skos:prefLabel>
		<skos:prefLabel xml:lang="ms">Sistem maklumat geografi</skos:prefLabel>
		<skos:scopeNote>AGROVOC Multilingual Thesaurus term ISO 19101-1</skos:scopeNote>
		<skos:definition>information system dealing with information concerning phenomena associated with location relative to the Earth (Source: ISO 19101-1:2014, 4.1.20)</skos:definition>
		<skos:changeNote>Established with version 1. Definition added with version 6, and term edited from Geographical to Geographic, to follow ISO and general use</skos:changeNote>
		<skos:exactMatch rdf:resource="https://isotc211.geolexica.org/concepts/207/"/>
		<skos:exactMatch rdf:resource="http://eurovoc.europa.eu/7218"/>
		<skos:inScheme rdf:resource="http://www.cadastralvocabulary.org/CaLAThe"/>
		<skos:broader rdf:resource="http://www.cadastralvocabulary.org/CaLAThe/SpatialDataInfrastructure"/>
		<skos:narrower rdf:resource="http://www.cadastralvocabulary.org/CaLAThe/CadastralSystem"/>
	</skos:Concept>

	<skos:Concept rdf:about="http://www.cadastralvocabulary.org/CaLAThe/GeographicalGridSystem">
		<skos:prefLabel xml:lang="en">Geographical grid system</skos:prefLabel>
		<skos:prefLabel xml:lang="da">Geografiske kvadratnetsystemer</skos:prefLabel>
		<skos:prefLabel xml:lang="tr">Coğrafi grid sistemi</skos:prefLabel>
		<skos:prefLabel xml:lang="ms">Sistem grid geografi</skos:prefLabel>
		<skos:scopeNote>INSPIRE term</skos:scopeNote>
		<skos:definition>Harmonised multi-resolution grid with a common point of origin and standardised location and size of grid cells [INSPIRE Directive] (Source: INSPIRE glossary).</skos:definition>
		<skos:changeNote>Established with version 1.</skos:changeNote>
		<skos:exactMatch rdf:resource="http://inspire.ec.europa.eu/glossary/GeographicalGridSystem"/>
		<skos:inScheme rdf:resource="http://www.cadastralvocabulary.org/CaLAThe"/>
		<skos:broader rdf:resource="http://www.cadastralvocabulary.org/CaLAThe/SpatialReference"/>
	</skos:Concept>

	<skos:Concept rdf:about="http://www.cadastralvocabulary.org/CaLAThe/GeolocatedInformation">
		<skos:prefLabel xml:lang="en">Geolocated information</skos:prefLabel>
		<skos:prefLabel xml:lang="da">Stedbestemt information</skos:prefLabel>
		<skos:prefLabel xml:lang="tr">Coğrafi konumlandırılmış bilgi</skos:prefLabel>
		<skos:prefLabel xml:lang="ms">Maklumat geolokasi</skos:prefLabel>
		<skos:definition>Information which is localized on the surface of the Earth through nominal, ordinal or metric means (cf Stevens, 1946; Stubkjær, 1992)</skos:definition>
		<skos:changeNote>Introduced with version 4</skos:changeNote>
		<skos:inScheme rdf:resource="http://www.cadastralvocabulary.org/CaLAThe"/>
		<skos:broader rdf:resource="http://www.cadastralvocabulary.org/CaLAThe/Information"/>
		<skos:narrower rdf:resource="http://www.cadastralvocabulary.org/CaLAThe/PlaceName"/>
		<skos:narrower rdf:resource="http://www.cadastralvocabulary.org/CaLAThe/SpatialDataInfrastructure"/>
		<skos:narrower rdf:resource="http://www.cadastralvocabulary.org/CaLAThe/TopologicalLocalization"/>
		<skos:narrower rdf:resource="http://www.cadastralvocabulary.org/CaLAThe/Map"/>
		<skos:narrower rdf:resource="http://www.cadastralvocabulary.org/CaLAThe/DigitalImagery"/>
		<skos:narrower rdf:resource="http://www.cadastralvocabulary.org/CaLAThe/SpatialUnit"/>
	</skos:Concept>

	<skos:Concept rdf:about="http://www.cadastralvocabulary.org/CaLAThe/GeometricPrimitive">
		<skos:prefLabel xml:lang="en">Geometric primitive</skos:prefLabel>
		<skos:prefLabel xml:lang="da">Geometrisk objekt</skos:prefLabel>
		<skos:prefLabel xml:lang="tr">Geometrik obje</skos:prefLabel>
		<skos:prefLabel xml:lang="ms">Geometrik primitif</skos:prefLabel>
		<skos:scopeNote>Geolexica term</skos:scopeNote>
		<skos:definition>Geometric object representing a single, connected, homogeneous (isotropic) element of space (ISO 19107:2019, (E), 3.50).</skos:definition>
		<skos:changeNote>Established with version 1.</skos:changeNote>
		<skos:exactMatch rdf:resource="https://isotc211.geolexica.org/concepts/2164/"/>
		<skos:inScheme rdf:resource="http://www.cadastralvocabulary.org/CaLAThe"/>
		<skos:broader rdf:resource="http://www.cadastralvocabulary.org/CaLAThe/SpatialUnit"/>
		<skos:narrower rdf:resource="http://www.cadastralvocabulary.org/CaLAThe/LA_PointBasedSpatialUnit"/>
		<skos:narrower rdf:resource="http://www.cadastralvocabulary.org/CaLAThe/LA_LineBasedSpatialUnit"/>
		<skos:narrower rdf:resource="http://www.cadastralvocabulary.org/CaLAThe/PolygonBasedSpatialUnit"/>
		<skos:narrower rdf:resource="http://www.cadastralvocabulary.org/CaLAThe/Curve"/>
		<skos:narrower rdf:resource="http://www.cadastralvocabulary.org/CaLAThe/Surface"/>
		<skos:narrower rdf:resource="http://www.cadastralvocabulary.org/CaLAThe/Point"/>
		<skos:narrower rdf:resource="http://www.cadastralvocabulary.org/CaLAThe/LA_Point"/>
	</skos:Concept>

	<skos:Concept rdf:about="http://www.cadastralvocabulary.org/CaLAThe/Gift">
		<skos:prefLabel xml:lang="en">Gift</skos:prefLabel>
		<skos:prefLabel xml:lang="da">Gave</skos:prefLabel>
		<skos:prefLabel xml:lang="tr">Bağış</skos:prefLabel>
		<skos:prefLabel xml:lang="ms">Hibah, Hadiah</skos:prefLabel>
		<skos:definition>The voluntarily Transfer of Real property by the Owner to another Party without getting anything in return.</skos:definition>
		<skos:changeNote>Established with version 2.</skos:changeNote>
		<skos:exactMatch rdf:resource="http://eurovoc.europa.eu/501"/>
		<skos:inScheme rdf:resource="http://www.cadastralvocabulary.org/CaLAThe"/>
		<skos:broader rdf:resource="http://www.cadastralvocabulary.org/CaLAThe/Transfer"/>
	</skos:Concept>

	<skos:Concept rdf:about="http://www.cadastralvocabulary.org/CaLAThe/GNSSobservation">
		<skos:prefLabel xml:lang="en">GNSS observation</skos:prefLabel>
		<skos:prefLabel xml:lang="da">GNSS observation</skos:prefLabel>
		<skos:prefLabel xml:lang="tr">GNSS gözlemi</skos:prefLabel>
		<skos:prefLabel xml:lang="ms">Cerapan GNSS</skos:prefLabel>
		<skos:definition>GNSS observation contains all observations to one or more satellite systems. When using differential GNSS, also the information on the reference stations are included. (OGC LandInfra 7.8.3.9)</skos:definition>
		<skos:changeNote>Established with version 4</skos:changeNote>
		<skos:exactMatch rdf:resource="http://docs.opengeospatial.org/is/15-111r1/15-111r1.html#121"/>
		<skos:inScheme rdf:resource="http://www.cadastralvocabulary.org/CaLAThe"/>
		<skos:broader rdf:resource="http://www.cadastralvocabulary.org/CaLAThe/Observation"/>
		<skos:broader rdf:resource="http://www.cadastralvocabulary.org/CaLAThe/GNSSsensor"/>
		<skos:narrower rdf:resource="http://www.cadastralvocabulary.org/CaLAThe/TargetPoint"/>
	</skos:Concept>

	<skos:Concept rdf:about="http://www.cadastralvocabulary.org/CaLAThe/GNSSsensor">
		<skos:prefLabel xml:lang="en">GNSS sensor</skos:prefLabel>
		<skos:prefLabel xml:lang="da">GNSS modtager</skos:prefLabel>
		<skos:prefLabel xml:lang="tr">GNSS alıcısı</skos:prefLabel>
		<skos:prefLabel xml:lang="ms">Penderia GNSS</skos:prefLabel>
		<skos:scopeNote>OGC LandInfra / InfraGML term</skos:scopeNote>
		<skos:definition>GNSS sensors receive the signals from different satellite systems to determine a 3d location of the TargetPoint. External antennas could be also used. If differential GNSS was used GNSS sensor may also contain the sensor information of the reference station. GNSS class will then contain the reference aggregation of a GNNS reference sensor. (OGC LandInfra 7.8.5.13)</skos:definition>
		<skos:changeNote>Established with version 4</skos:changeNote>
		<skos:exactMatch rdf:resource="http://docs.opengeospatial.org/is/15-111r1/15-111r1.html#148"/>
		<skos:inScheme rdf:resource="http://www.cadastralvocabulary.org/CaLAThe"/>
		<skos:broader rdf:resource="http://www.cadastralvocabulary.org/CaLAThe/SurveyingInstrument"/>
		<skos:narrower rdf:resource="http://www.cadastralvocabulary.org/CaLAThe/GNSSobservation"/>
	</skos:Concept>

	<skos:Concept rdf:about="http://www.cadastralvocabulary.org/CaLAThe/GoodFaith">
		<skos:prefLabel xml:lang="en">Good faith</skos:prefLabel>
		<skos:prefLabel xml:lang="da">God tro</skos:prefLabel>
		<skos:prefLabel xml:lang="tr">İyi niyet</skos:prefLabel>
		<skos:prefLabel xml:lang="ms">Niat baik</skos:prefLabel>
		<skos:definition>Principle of honesty or sincerity of intention.</skos:definition>
		<skos:changeNote>Established with version 3.</skos:changeNote>
		<skos:inScheme rdf:resource="http://www.cadastralvocabulary.org/CaLAThe"/>
		<skos:broader rdf:resource="http://www.cadastralvocabulary.org/CaLAThe/RightsHolder"/>
	</skos:Concept>

	<skos:Concept rdf:about="http://www.cadastralvocabulary.org/CaLAThe/GovernmentalOrganisation">
		<skos:prefLabel xml:lang="en">Governmental organisation</skos:prefLabel>
		<skos:prefLabel xml:lang="da">Offentlig forvaltning</skos:prefLabel>
		<skos:prefLabel xml:lang="tr">Devlet kuruluşu</skos:prefLabel>
		<skos:prefLabel xml:lang="ms">Organisasi kerajaan</skos:prefLabel>
		<skos:scopeNote>AGROVOC Multilingual Thesaurus term</skos:scopeNote>
		<skos:definition>Any governmental agency or organization charged with managing and implementing regulations, laws and government policies (Source: AGROVOC).</skos:definition>
		<skos:changeNote>Established with version 1. Edited with version 4. Agency added with ver. 5.</skos:changeNote>
		<skos:exactMatch rdf:resource="http://aims.fao.org/aos/agrovoc/c_50225"/>
		<skos:exactMatch rdf:resource="http://eurovoc.europa.eu/77"/>
		<skos:inScheme rdf:resource="http://www.cadastralvocabulary.org/CaLAThe"/>
		<skos:altLabel>Administrative body</skos:altLabel>
		<skos:altLabel>Agency</skos:altLabel>
		<skos:broader rdf:resource="http://www.cadastralvocabulary.org/CaLAThe/Organisation"/>
		<skos:narrower rdf:resource="http://www.cadastralvocabulary.org/CaLAThe/Registry"/>
	</skos:Concept>


	<skos:Concept rdf:about="http://www.cadastralvocabulary.org/CaLAThe/GroupParty">
		<skos:prefLabel xml:lang="en">Group party</skos:prefLabel>
		<skos:prefLabel xml:lang="da">Gruppe</skos:prefLabel>
		<skos:prefLabel xml:lang="tr">Grup </skos:prefLabel>
		<skos:prefLabel xml:lang="ms">Pihak berkumpulan</skos:prefLabel>
		<skos:scopeNote>ISO LADM term</skos:scopeNote>
		<skos:definition>A Party type consisting of a number of Natural persons.</skos:definition>
		<skos:changeNote>Established with version 1. Definition is changed with version 6.</skos:changeNote>
		<skos:inScheme rdf:resource="http://www.cadastralvocabulary.org/CaLAThe"/>
		<skos:altLabel>LA_GroupParty</skos:altLabel>
		<skos:broader rdf:resource="http://www.cadastralvocabulary.org/CaLAThe/PartyType"/>
		<skos:narrower rdf:resource="http://www.cadastralvocabulary.org/CaLAThe/SocialGroup"/>
		<skos:narrower rdf:resource="http://www.cadastralvocabulary.org/CaLAThe/PlaceBoundParty"/>
	</skos:Concept>

	<skos:Concept rdf:about="http://www.cadastralvocabulary.org/CaLAThe/Hydrography">
		<skos:prefLabel xml:lang="en">Hydrography</skos:prefLabel>
		<skos:prefLabel xml:lang="da">Hydrografi</skos:prefLabel>
		<skos:prefLabel xml:lang="tr">Hidroğrafya</skos:prefLabel>
		<skos:prefLabel xml:lang="ms">Hidrografi</skos:prefLabel>
		<skos:scopeNote>GEMET term</skos:scopeNote>
		<skos:definition>Science which deals with the measurement and description of the physical features of the oceans, lakes, rivers, and their adjoining coastal areas, with particular reference to their control and utilization (Source: GEMET).</skos:definition>
		<skos:changeNote>Established with version 1.</skos:changeNote>
		<skos:exactMatch rdf:resource="https://www.eionet.europa.eu/gemet/en/concept/4109"/>
		<skos:exactMatch rdf:resource="http://aims.fao.org/aos/agrovoc/c_3727"/>
		<skos:inScheme rdf:resource="http://www.cadastralvocabulary.org/CaLAThe"/>
		<skos:broader rdf:resource="http://www.cadastralvocabulary.org/CaLAThe/TopographicalFeature"/>
	</skos:Concept>

	<skos:Concept rdf:about="http://www.cadastralvocabulary.org/CaLAThe/Image">
		<skos:prefLabel xml:lang="en">Image</skos:prefLabel>
		<skos:prefLabel xml:lang="da">Billede, Digitalbillede</skos:prefLabel>
		<skos:prefLabel xml:lang="tr">Görüntü</skos:prefLabel>
		<skos:prefLabel xml:lang="ms">Imej</skos:prefLabel>
		<skos:scopeNote>OGC LandInfra / InfraGML term</skos:scopeNote>
		<skos:definition>Image is the result of an ImageObservation (OCG LandInfra 7.8.7.8)</skos:definition>
		<skos:changeNote>Established with version 4</skos:changeNote>
		<skos:exactMatch rdf:resource="https://isotc211.geolexica.org/concepts/551/"/>
		<skos:inScheme rdf:resource="http://www.cadastralvocabulary.org/CaLAThe"/>
		<skos:broader rdf:resource="http://www.cadastralvocabulary.org/CaLAThe/Camera"/>
		<skos:broader rdf:resource="http://www.cadastralvocabulary.org/CaLAThe/SurveyResult"/>
	</skos:Concept>

	<skos:Concept rdf:about="http://www.cadastralvocabulary.org/CaLAThe/IndividualOwnership">
		<skos:prefLabel xml:lang="en">Individual ownership</skos:prefLabel>
		<skos:prefLabel xml:lang="da">Selveje</skos:prefLabel>
		<skos:prefLabel xml:lang="tr">Bireysel mülkiyet</skos:prefLabel>
		<skos:prefLabel xml:lang="ms">Pemilikan individu</skos:prefLabel>
		<skos:definition>Exercise of ownership towards property by an individual (Source: Legal Dictionary of Property in Canada - Dualjuridik).</skos:definition>
		<skos:changeNote>Established with version 1. Definition added with version 3.</skos:changeNote>
		<skos:inScheme rdf:resource="http://www.cadastralvocabulary.org/CaLAThe"/>
		<skos:broader rdf:resource="http://www.cadastralvocabulary.org/CaLAThe/Ownership"/>
	</skos:Concept>

	<skos:Concept rdf:about="http://www.cadastralvocabulary.org/CaLAThe/Information">
		<skos:prefLabel xml:lang="en">Information</skos:prefLabel>
		<skos:prefLabel xml:lang="da">Information</skos:prefLabel>
		<skos:prefLabel xml:lang="tr">Bilgi</skos:prefLabel>
		<skos:prefLabel xml:lang="ms">Maklumat, Informasi</skos:prefLabel>
		<skos:scopeNote>GEMET General Multilingual Environmental Thesaurus term</skos:scopeNote>
		<skos:definition>All facts, ideas or imaginative works of the mind which have been communicated, published or distributed formally or informally in any format, or the knowledge that is communicated or received. </skos:definition>
		<skos:changeNote>Established as Documentation with version 1. Edited to Information in version 4.</skos:changeNote>
		<skos:exactMatch rdf:resource="https://www.eionet.europa.eu/gemet/en/concept/4303"/>
		<skos:exactMatch rdf:resource="http://zbw.eu/stw/descriptor/16754-4"/>
		<skos:exactMatch rdf:resource="http://aims.fao.org/aos/agrovoc/c_330966"/>
		<skos:exactMatch rdf:resource="http://eurovoc.europa.eu/1422"/>
		<skos:inScheme rdf:resource="http://www.cadastralvocabulary.org/CaLAThe"/>
		<skos:narrower rdf:resource="http://www.cadastralvocabulary.org/CaLAThe/Document"/>
		<skos:narrower rdf:resource="http://www.cadastralvocabulary.org/CaLAThe/Metadata"/>
		<skos:narrower rdf:resource="http://www.cadastralvocabulary.org/CaLAThe/GeolocatedInformation"/>
		<skos:narrower rdf:resource="http://www.cadastralvocabulary.org/CaLAThe/SpatialReference"/>
		<skos:narrower rdf:resource="http://www.cadastralvocabulary.org/CaLAThe/CodeList"/>
	</skos:Concept>

	<skos:Concept rdf:about="http://www.cadastralvocabulary.org/CaLAThe/Inheritance">
		<skos:prefLabel xml:lang="en">Inheritance</skos:prefLabel>
		<skos:prefLabel xml:lang="da">Arv</skos:prefLabel>
		<skos:prefLabel xml:lang="tr">Miras</skos:prefLabel>
		<skos:prefLabel xml:lang="ms">Pewarisan</skos:prefLabel>
		<skos:definition>The Transfer of Real property or Real rights to heirs upon the death of the Owner.</skos:definition>
		<skos:changeNote>Established with version 2.</skos:changeNote>
		<skos:exactMatch rdf:resource="http://zbw.eu/stw/descriptor/16028-5"/>
		<skos:exactMatch rdf:resource="http://eurovoc.europa.eu/3934"/>
		<skos:inScheme rdf:resource="http://www.cadastralvocabulary.org/CaLAThe"/>
		<skos:broader rdf:resource="http://www.cadastralvocabulary.org/CaLAThe/Transfer"/>
	</skos:Concept>

	<skos:Concept rdf:about="http://www.cadastralvocabulary.org/CaLAThe/Judiciary">
		<skos:prefLabel xml:lang="en">Judiciary</skos:prefLabel>
		<skos:prefLabel xml:lang="da">Retsvæsen</skos:prefLabel>
		<skos:prefLabel xml:lang="tr">Yargı</skos:prefLabel>
		<skos:prefLabel xml:lang="ms">Badan kehakiman</skos:prefLabel>
		<skos:scopeNote>STW Thesaurus for Economics term</skos:scopeNote>
		<skos:changeNote>Established with version 1.</skos:changeNote>
		<skos:exactMatch rdf:resource="http://zbw.eu/stw/descriptor/19841-1"/>
		<skos:inScheme rdf:resource="http://www.cadastralvocabulary.org/CaLAThe"/>
		<skos:broader rdf:resource="http://www.cadastralvocabulary.org/CaLAThe/Organisation"/>
	</skos:Concept>

	<skos:Concept rdf:about="http://www.cadastralvocabulary.org/CaLAThe/Land">
		<skos:prefLabel xml:lang="en">Land</skos:prefLabel>
		<skos:prefLabel xml:lang="da">Land</skos:prefLabel>
		<skos:prefLabel xml:lang="tr">Arazi</skos:prefLabel>
		<skos:prefLabel xml:lang="ms">Tanah</skos:prefLabel>
		<skos:definition>The area of earth&#39;s surface, excluding the oceans, usually marked off by natural or political boundaries, or boundaries of ownership (ISO 6707-1:2014).</skos:definition>
		<skos:changeNote>Established with version 1.</skos:changeNote>
		<skos:exactMatch rdf:resource="http://zbw.eu/stw/descriptor/12015-6"/>
		<skos:exactMatch rdf:resource="https://www.eionet.europa.eu/gemet/en/concept/4599"/>
		<skos:exactMatch rdf:resource="http://aims.fao.org/aos/agrovoc/c_4172"/>
		<skos:inScheme rdf:resource="http://www.cadastralvocabulary.org/CaLAThe"/>
		<skos:narrower rdf:resource="http://www.cadastralvocabulary.org/CaLAThe/SpatialFeatureType"/>
	</skos:Concept>

	<skos:Concept rdf:about="http://www.cadastralvocabulary.org/CaLAThe/LandAdministration">
		<skos:prefLabel xml:lang="en">Land administration</skos:prefLabel>
		<skos:prefLabel xml:lang="da">Forvaltning af ejendomsdata</skos:prefLabel>
		<skos:prefLabel xml:lang="tr">Arazi bilgi yönetimi</skos:prefLabel>
		<skos:prefLabel xml:lang="ms">Pentadbiran tanah</skos:prefLabel>
		<skos:scopeNote>ISO LADM term</skos:scopeNote>
		<skos:definition>The process of determining, recording and disseminating information about the relationship between people and land (ISO LADM, 4.1.10).</skos:definition>
		<skos:changeNote>Established with version 3.</skos:changeNote>
		<skos:exactMatch rdf:resource="http://aims.fao.org/aos/agrovoc/c_9000091"/>
		<skos:exactMatch rdf:resource="https://isotc211.geolexica.org/concepts/1300/"/>
		<skos:inScheme rdf:resource="http://www.cadastralvocabulary.org/CaLAThe"/>
	</skos:Concept>

	<skos:Concept rdf:about="http://www.cadastralvocabulary.org/CaLAThe/LandConsolidation">
		<skos:prefLabel xml:lang="en">Land consolidation</skos:prefLabel>
		<skos:prefLabel xml:lang="da">Jordfordeling</skos:prefLabel>
		<skos:prefLabel xml:lang="tr">Arazi toplulaştırması</skos:prefLabel>
		<skos:prefLabel xml:lang="ms">Penyatuan tanah</skos:prefLabel>
		<skos:definition>A Property restructuring of fragmented land units especially in rural areas into Cadastral parcels having more economic and rational size, shape, location, and access.</skos:definition>
		<skos:changeNote>Established with version 2.</skos:changeNote>
		<skos:exactMatch rdf:resource="http://aims.fao.org/aos/agrovoc/c_4173"/>
		<skos:exactMatch rdf:resource="https://www.eionet.europa.eu/gemet/en/concept/4611"/>
		<skos:inScheme rdf:resource="http://www.cadastralvocabulary.org/CaLAThe"/>
		<skos:broader rdf:resource="http://www.cadastralvocabulary.org/CaLAThe/PropertyRestructuring"/>
		<skos:narrower rdf:resource="http://www.cadastralvocabulary.org/CaLAThe/Reallotment"/>
	</skos:Concept>

	<skos:Concept rdf:about="http://www.cadastralvocabulary.org/CaLAThe/LandDivision">
		<skos:prefLabel xml:lang="en">Land division</skos:prefLabel>
		<skos:prefLabel xml:lang="da">Geografisk opdeling</skos:prefLabel>
		<skos:prefLabel xml:lang="tr">Coğrafi birim</skos:prefLabel>
		<skos:prefLabel xml:lang="ms">Pecah sempadan tanah</skos:prefLabel>
		<skos:scopeNote>OGC LandInfra / InfraGML term</skos:scopeNote>
		<skos:definition>Land division may be public (political, judicial, or executive) or private in nature, the latter delimiting ownership in land or in alternative terms: boundaries of real estate, of real property or of immovable property (Source: OGC LandInfra, 7.10.1).</skos:definition>
		<skos:changeNote>Established with version 1. Term changed with version 3 to Land division, and definition added.</skos:changeNote>
		<skos:inScheme rdf:resource="http://www.cadastralvocabulary.org/CaLAThe"/>
		<skos:altLabel>Administrative feature</skos:altLabel>
		<skos:broader rdf:resource="http://www.cadastralvocabulary.org/CaLAThe/SpatialFeatureType"/>
		<skos:narrower rdf:resource="http://www.cadastralvocabulary.org/CaLAThe/AdministrativeUnit"/>
		<skos:narrower rdf:resource="http://www.cadastralvocabulary.org/CaLAThe/RealProperty"/>
		<skos:narrower rdf:resource="http://www.cadastralvocabulary.org/CaLAThe/Marker"/>
		<skos:narrower rdf:resource="http://www.cadastralvocabulary.org/CaLAThe/PlaceName"/>
		<skos:narrower rdf:resource="http://www.cadastralvocabulary.org/CaLAThe/Boundary"/>
	</skos:Concept>

	<skos:Concept rdf:about="http://www.cadastralvocabulary.org/CaLAThe/LandLaw">
		<skos:prefLabel xml:lang="en">Land law</skos:prefLabel>
		<skos:prefLabel xml:lang="da">Ejendomsret (til fast ejendom)</skos:prefLabel>
		<skos:prefLabel xml:lang="tr">Taşınmaz (Gayrimenkul) hukuku</skos:prefLabel>
		<skos:prefLabel xml:lang="ms">Undang-undang tanah</skos:prefLabel>
		<skos:definition>Positive law concerning real estate / immovable property, including property formation, land development, and implementation of spatial planning  (Cf. Mattsson, 2001).</skos:definition>
		<skos:changeNote>Established with version 3.</skos:changeNote>
		<skos:exactMatch rdf:resource="http://aims.fao.org/aos/agrovoc/c_573abb9f"/>
		<skos:inScheme rdf:resource="http://www.cadastralvocabulary.org/CaLAThe"/>
		<skos:altLabel>Property law</skos:altLabel>
		<skos:broader rdf:resource="http://www.cadastralvocabulary.org/CaLAThe/PositiveLaw"/>
		<skos:narrower rdf:resource="http://www.cadastralvocabulary.org/CaLAThe/RealRight"/>
		<skos:narrower rdf:resource="http://www.cadastralvocabulary.org/CaLAThe/PlanningLaw"/>
		<skos:narrower rdf:resource="http://www.cadastralvocabulary.org/CaLAThe/LA_RRR"/>
		<skos:narrower rdf:resource="http://www.cadastralvocabulary.org/CaLAThe/LawOfObligation"/>
	</skos:Concept>

	<skos:Concept rdf:about="http://www.cadastralvocabulary.org/CaLAThe/LandReadjustment">
		<skos:prefLabel xml:lang="en">Land readjustment</skos:prefLabel>
		<skos:prefLabel xml:lang="da">Multifunktionel jordfordeling</skos:prefLabel>
		<skos:prefLabel xml:lang="tr">Arazi ve arsa düzenlemesi</skos:prefLabel>
		<skos:prefLabel xml:lang="ms">Pelarasan semula tanah</skos:prefLabel>
		<skos:definition>A Property restructuring that forms Cadastral parcels available for building according to land use plans.</skos:definition>
		<skos:changeNote>Established with version 2.</skos:changeNote>
		<skos:exactMatch rdf:resource="http://aims.fao.org/aos/agrovoc/c_57156ff8"/>
		<skos:inScheme rdf:resource="http://www.cadastralvocabulary.org/CaLAThe"/>
		<skos:broader rdf:resource="http://www.cadastralvocabulary.org/CaLAThe/PropertyRestructuring"/>
		<skos:narrower rdf:resource="http://www.cadastralvocabulary.org/CaLAThe/Reallotment"/>
	</skos:Concept>

	<skos:Concept rdf:about="http://www.cadastralvocabulary.org/CaLAThe/LandRegistry">
		<skos:prefLabel xml:lang="en">Land registry</skos:prefLabel>
		<skos:prefLabel xml:lang="da">Tingbogen (for fast ejendom)</skos:prefLabel>
		<skos:prefLabel xml:lang="tr">Tapu sicili</skos:prefLabel>
		<skos:prefLabel xml:lang="ms">Daftar tanah</skos:prefLabel>
		<skos:scopeNote>ELRA</skos:scopeNote>
		<skos:definition>A public register, recording property rights and interest, or the existence of deeds or title documents. (Adopted from UNECE, WPLA: Guidelines, 2004, and FAO Agrovoc).</skos:definition>
		<skos:changeNote>Established with version 1. Relations changed with version 5 and 6.</skos:changeNote>
		<skos:inScheme rdf:resource="http://www.cadastralvocabulary.org/CaLAThe"/>
		<skos:broader rdf:resource="http://www.cadastralvocabulary.org/CaLAThe/Registry"/>
		<skos:narrower rdf:resource="http://www.cadastralvocabulary.org/CaLAThe/LandRegister"/>
	</skos:Concept>

	<skos:Concept rdf:about="http://www.cadastralvocabulary.org/CaLAThe/LandRegister">
		<skos:prefLabel xml:lang="en">Land register</skos:prefLabel>
		<skos:prefLabel xml:lang="da">Tingbogen (for fast ejendom)</skos:prefLabel>
		<skos:prefLabel xml:lang="tr">Tapu sicili</skos:prefLabel>
		<skos:prefLabel xml:lang="ms">Daftar tanah</skos:prefLabel>
		<skos:scopeNote>FAO Agrovoc; UNECE, WPLA: Guidelines</skos:scopeNote>
		<skos:definition>A public register, recording property rights and interest, or the existence of deeds or title documents. (Adopted from UNECE, WPLA: Guidelines, 2004, and FAO Agrovoc)</skos:definition>
		<skos:changeNote>Established with version 1. Relations changed with version 5 and 6.</skos:changeNote>
		<skos:closeMatch rdf:resource="https://agrovoc.fao.org/browse/agrovoc/en/page/c_a72beecd"/>
		<skos:broadMatch rdf:resource="http://www.eionet.europa.eu/gemet/concept/4644"/>
		<skos:inScheme rdf:resource="http://www.cadastralvocabulary.org/CaLAThe"/>
		<skos:broader rdf:resource="http://www.cadastralvocabulary.org/CaLAThe/Registry"/>
	</skos:Concept>

	<skos:Concept rdf:about="http://www.cadastralvocabulary.org/CaLAThe/Law">
		<skos:prefLabel xml:lang="en">Law</skos:prefLabel>
		<skos:prefLabel xml:lang="da">Lov, Jura, Ret</skos:prefLabel>
		<skos:prefLabel xml:lang="tr">Hukuk</skos:prefLabel>
		<skos:prefLabel xml:lang="ms">Undang-undang</skos:prefLabel>
		<skos:scopeNote>STW Thesaurus for Economics term</skos:scopeNote>
		<skos:changeNote>Established with version 1.</skos:changeNote>
		<skos:exactMatch rdf:resource="http://zbw.eu/stw/descriptor/15966-1"/>
		<skos:exactMatch rdf:resource="http://aims.fao.org/aos/agrovoc/c_12106"/>
		<skos:exactMatch rdf:resource="https://www.eionet.europa.eu/gemet/en/concept/4719"/>
		<skos:exactMatch rdf:resource="http://eurovoc.europa.eu/3935"/>
		<skos:inScheme rdf:resource="http://www.cadastralvocabulary.org/CaLAThe"/>
		<skos:narrower rdf:resource="http://www.cadastralvocabulary.org/CaLAThe/PartyRoleType"/>
		<skos:narrower rdf:resource="http://www.cadastralvocabulary.org/CaLAThe/CustomaryLaw"/>
		<skos:narrower rdf:resource="http://www.cadastralvocabulary.org/CaLAThe/PositiveLaw"/>
		<skos:narrower rdf:resource="http://www.cadastralvocabulary.org/CaLAThe/NaturalLaw"/>
	</skos:Concept>

	<skos:Concept rdf:about="http://www.cadastralvocabulary.org/CaLAThe/LawOfObligation">
		<skos:prefLabel xml:lang="en">Law of obligation</skos:prefLabel>
		<skos:prefLabel xml:lang="da">Obligationsret</skos:prefLabel>
		<skos:prefLabel xml:lang="tr">Borçlar Hukuku</skos:prefLabel>
		<skos:prefLabel xml:lang="ms">Undang-undang tanggungjawab</skos:prefLabel>
		<skos:scopeNote>Added in version 5 to represent personal rights (cf. Swiss Civil Law, article 959) that can be entered into land book.</skos:scopeNote>
		<skos:inScheme rdf:resource="http://www.cadastralvocabulary.org/CaLAThe"/>
		<skos:broader rdf:resource="http://www.cadastralvocabulary.org/CaLAThe/LandLaw"/>
		<skos:narrower rdf:resource="http://www.cadastralvocabulary.org/CaLAThe/OptionToPurchase"/>
		<skos:narrower rdf:resource="http://www.cadastralvocabulary.org/CaLAThe/PreemptionRight"/>
	</skos:Concept>

	<skos:Concept rdf:about="http://www.cadastralvocabulary.org/CaLAThe/Lawyer">
		<skos:prefLabel xml:lang="en">Lawyer</skos:prefLabel>
		<skos:prefLabel xml:lang="da">Advokat</skos:prefLabel>
		<skos:prefLabel xml:lang="tr">Hukukçu</skos:prefLabel>
		<skos:prefLabel xml:lang="ms">Peguam</skos:prefLabel>
		<skos:definition>A Professional who is authorized to conduct lawsuits for clients or to advise as to legal rights and obligations in other matters.</skos:definition>
		<skos:changeNote>Established with version 3. Definition is added with version 6.</skos:changeNote>
		<skos:exactMatch rdf:resource="http://eurovoc.europa.eu/5141"/>
		<skos:inScheme rdf:resource="http://www.cadastralvocabulary.org/CaLAThe"/>
		<skos:broader rdf:resource="http://www.cadastralvocabulary.org/CaLAThe/Professional"/>
		<skos:narrower rdf:resource="http://www.cadastralvocabulary.org/CaLAThe/LegalAdvisor"/>
	</skos:Concept>

	<skos:Concept rdf:about="http://www.cadastralvocabulary.org/CaLAThe/LA_AdministrativeSource">
		<skos:prefLabel xml:lang="en">LA_AdministrativeSource</skos:prefLabel>
		<skos:scopeNote>ISO LADM term</skos:scopeNote>
		<skos:definition>Source (4.1.21) with the administrative description (where applicable) of the parties (4.1.13) involved, the rights (4.1.20), restrictions (4.1.19) and responsibilities (4.1.18) created and the basic administrative units (4.1.2) affected (Source: ISO LADM, 4.1.1).</skos:definition>
		<skos:changeNote>Established with version 3.</skos:changeNote>
		<skos:exactMatch rdf:resource="https://isotc211.geolexica.org/concepts/1286/"/>
		<skos:inScheme rdf:resource="http://www.cadastralvocabulary.org/CaLAThe"/>
		<skos:broader rdf:resource="http://www.cadastralvocabulary.org/CaLAThe/LA_Source"/>
	</skos:Concept>

	<skos:Concept rdf:about="http://www.cadastralvocabulary.org/CaLAThe/LA_BAUnit">
		<skos:prefLabel xml:lang="en">LA_BAUnit</skos:prefLabel>
		<skos:scopeNote>ISO LADM term</skos:scopeNote>
		<skos:definition>Administrative entity, subject to registration, consisting of zero or more spatial units (4.1.23) against which (one or more) unique and homogeneous rights [e.g. ownership right or land (4.1.9) use right], responsibilities (4.1.18) or restrictions (4.1.19) are associated to the whole entity (Source: ISO LADM, 4.1.2 - here simplified)</skos:definition>
		<skos:changeNote>Established with version 1.</skos:changeNote>
		<skos:exactMatch rdf:resource="http://aims.fao.org/aos/agrovoc/c_3022da1f"/>
		<skos:exactMatch rdf:resource="https://isotc211.geolexica.org/concepts/1570/"/>
		<skos:inScheme rdf:resource="http://www.cadastralvocabulary.org/CaLAThe"/>
		<skos:broader rdf:resource="http://www.cadastralvocabulary.org/CaLAThe/RealProperty"/>
	</skos:Concept>

	<skos:Concept rdf:about="http://www.cadastralvocabulary.org/CaLAThe/LA_BoundaryFaceString">
		<skos:prefLabel xml:lang="en">LA_BoundaryFaceString</skos:prefLabel>
		<skos:changeNote>Established with version 3. Relation edited with version 4.</skos:changeNote>
		<skos:exactMatch rdf:resource="http://aims.fao.org/aos/agrovoc/c_c9ac54c9"/>
		<skos:exactMatch rdf:resource="https://isotc211.geolexica.org/concepts/1289/"/>
		<skos:inScheme rdf:resource="http://www.cadastralvocabulary.org/CaLAThe"/>
		<skos:broader rdf:resource="http://www.cadastralvocabulary.org/CaLAThe/BoundingElement"/>
	</skos:Concept>

	<skos:Concept rdf:about="http://www.cadastralvocabulary.org/CaLAThe/LA_CertifiedSurveyor">
		<skos:prefLabel xml:lang="en">LA_CertifiedSurveyor</skos:prefLabel>
		<skos:scopeNote>ISO LADM</skos:scopeNote>
		<skos:changeNote>Established with version 4</skos:changeNote>
		<skos:inScheme rdf:resource="http://www.cadastralvocabulary.org/CaLAThe"/>
		<skos:broader rdf:resource="http://www.cadastralvocabulary.org/CaLAThe/Surveyor"/>
	</skos:Concept>

	<skos:Concept rdf:about="http://www.cadastralvocabulary.org/CaLAThe/LA_EdgeBasedSpatialUnit">
		<skos:prefLabel xml:lang="en">LA_Edge based spatial unit</skos:prefLabel>
		<skos:scopeNote>ISO LADM term</skos:scopeNote>
		<skos:changeNote>Established with version 1. Edited with version 4</skos:changeNote>
		<skos:exactMatch rdf:resource="http://aims.fao.org/aos/agrovoc/c_268654bb"/>
		<skos:inScheme rdf:resource="http://www.cadastralvocabulary.org/CaLAThe"/>
		<skos:broader rdf:resource="http://www.cadastralvocabulary.org/CaLAThe/Edge"/>
	</skos:Concept>

	<skos:Concept rdf:about="http://www.cadastralvocabulary.org/CaLAThe/LA_FaceBasedSpatialUnit">
		<skos:prefLabel xml:lang="en">LA_Face based spatial unit</skos:prefLabel>
		<skos:scopeNote>ISO LADM term</skos:scopeNote>
		<skos:changeNote>Established with version 1. Edited with version 4.</skos:changeNote>
		<skos:exactMatch rdf:resource="http://aims.fao.org/aos/agrovoc/c_9e450562"/>
		<skos:inScheme rdf:resource="http://www.cadastralvocabulary.org/CaLAThe"/>
		<skos:broader rdf:resource="http://www.cadastralvocabulary.org/CaLAThe/Face"/>
	</skos:Concept>

	<skos:Concept rdf:about="http://www.cadastralvocabulary.org/CaLAThe/LA_LegalSpaceBuildingUnit">
		<skos:prefLabel xml:lang="en">LA_LegalSpaceBuildingUnit</skos:prefLabel>
		<skos:scopeNote>ISO LADM term</skos:scopeNote>
		<skos:definition>Component of building (the legal, recorded or informal space of the physical entity) (Source: ISO LADM, 4.1.6).</skos:definition>
		<skos:changeNote>Established with version 3.</skos:changeNote>
		<skos:inScheme rdf:resource="http://www.cadastralvocabulary.org/CaLAThe"/>
		<skos:broader rdf:resource="http://www.cadastralvocabulary.org/CaLAThe/CondominiumBuilding"/>
	</skos:Concept>

	<skos:Concept rdf:about="http://www.cadastralvocabulary.org/CaLAThe/LA_LineBasedSpatialUnit">
		<skos:prefLabel xml:lang="en">LA_Line based spatial unit</skos:prefLabel>
		<skos:scopeNote>ISO LADM term</skos:scopeNote>
		<skos:changeNote>Established with version 1. Edited to LA_Line .. with version 4</skos:changeNote>
		<skos:inScheme rdf:resource="http://www.cadastralvocabulary.org/CaLAThe"/>
		<skos:broader rdf:resource="http://www.cadastralvocabulary.org/CaLAThe/GeometricPrimitive"/>
	</skos:Concept>

	<skos:Concept rdf:about="http://www.cadastralvocabulary.org/CaLAThe/LA_NodeBasedSpatialUnit">
		<skos:prefLabel xml:lang="en">LA_Node based spatial unit</skos:prefLabel>
		<skos:scopeNote>ISO LADM term</skos:scopeNote>
		<skos:changeNote>Introduced with version 1. Edited with version 4</skos:changeNote>
		<skos:exactMatch rdf:resource="http://aims.fao.org/aos/agrovoc/c_4be99d5b"/>
		<skos:inScheme rdf:resource="http://www.cadastralvocabulary.org/CaLAThe"/>
		<skos:broader rdf:resource="http://www.cadastralvocabulary.org/CaLAThe/Node"/>
	</skos:Concept>

	<skos:Concept rdf:about="http://www.cadastralvocabulary.org/CaLAThe/LA_Point">
		<skos:prefLabel xml:lang="en">LA_Point</skos:prefLabel>
		<skos:scopeNote>LADM term</skos:scopeNote>
		<skos:definition> 0-dimensional geometric primitive, representing a position [ISO 19107:2003, 4.61] (Source: ISO LADM, 4.1.15).</skos:definition>
		<skos:changeNote>Established with version 3.</skos:changeNote>
		<skos:exactMatch rdf:resource="http://aims.fao.org/aos/agrovoc/c_b12823a4"/>
		<skos:inScheme rdf:resource="http://www.cadastralvocabulary.org/CaLAThe"/>
		<skos:broader rdf:resource="http://www.cadastralvocabulary.org/CaLAThe/GeometricPrimitive"/>
	</skos:Concept>

	<skos:Concept rdf:about="http://www.cadastralvocabulary.org/CaLAThe/LA_PointBasedSpatialUnit">
		<skos:prefLabel xml:lang="en">LA_Point based spatial unit</skos:prefLabel>
		<skos:scopeNote>ISO LADM term</skos:scopeNote>
		<skos:changeNote>Established with version 1.0. Changed to LA_Point... with version 4</skos:changeNote>
		<skos:inScheme rdf:resource="http://www.cadastralvocabulary.org/CaLAThe"/>
		<skos:broader rdf:resource="http://www.cadastralvocabulary.org/CaLAThe/GeometricPrimitive"/>
	</skos:Concept>

	<skos:Concept rdf:about="http://www.cadastralvocabulary.org/CaLAThe/PolygonBasedSpatialUnit">
		<skos:prefLabel xml:lang="en">LA_Polygon based spatial unit</skos:prefLabel>
		<skos:scopeNote>ISO LADM term</skos:scopeNote>
		<skos:changeNote>Established with version 1.0. Edited to LA_Polygon.. with version 4</skos:changeNote>
		<skos:inScheme rdf:resource="http://www.cadastralvocabulary.org/CaLAThe"/>
		<skos:broader rdf:resource="http://www.cadastralvocabulary.org/CaLAThe/GeometricPrimitive"/>
	</skos:Concept>

	<skos:Concept rdf:about="http://www.cadastralvocabulary.org/CaLAThe/LA_RequiredRelationship">
		<skos:prefLabel xml:lang="en">LA_RequiredRelationship</skos:prefLabel>
		<skos:scopeNote>LADM term</skos:scopeNote>
		<skos:changeNote>Established with version 3, revised as concept in version 5.</skos:changeNote>
		<skos:exactMatch rdf:resource="https://isotc211.geolexica.org/concepts/1362/"/>
		<skos:inScheme rdf:resource="http://www.cadastralvocabulary.org/CaLAThe"/>
		<skos:broader rdf:resource="http://www.cadastralvocabulary.org/CaLAThe/RealProperty"/>
	</skos:Concept>

	<skos:Concept rdf:about="http://www.cadastralvocabulary.org/CaLAThe/LA_Restriction">
		<skos:prefLabel xml:lang="en">LA_Restriction</skos:prefLabel>
		<skos:scopeNote>ISO LADM term</skos:scopeNote>
		<skos:definition>Formal or informal obligation to refrain from doing something (Source: ISO LADM, 4.1.18).</skos:definition>
		<skos:changeNote>Established with version 3.</skos:changeNote>
		<skos:exactMatch rdf:resource="https://isotc211.geolexica.org/concepts/1573/"/>
		<skos:inScheme rdf:resource="http://www.cadastralvocabulary.org/CaLAThe"/>
		<skos:broader rdf:resource="http://www.cadastralvocabulary.org/CaLAThe/LimitedRight"/>
	</skos:Concept>

	<skos:Concept rdf:about="http://www.cadastralvocabulary.org/CaLAThe/LA_Right">
		<skos:prefLabel xml:lang="en">LA_Right</skos:prefLabel>
		<skos:scopeNote>ISO LADM term</skos:scopeNote>
		<skos:definition>Action, activity or class of actions that a system participant may perform on or using an associated resource [ISO 19132:2007, 4.38] (Source: ISO LADM, 4.1.20).</skos:definition>
		<skos:changeNote>Established with version 3.</skos:changeNote>
		<skos:exactMatch rdf:resource="https://isotc211.geolexica.org/concepts/680/"/>
		<skos:inScheme rdf:resource="http://www.cadastralvocabulary.org/CaLAThe"/>
		<skos:broader rdf:resource="http://www.cadastralvocabulary.org/CaLAThe/RealRight"/>
	</skos:Concept>

	<skos:Concept rdf:about="http://www.cadastralvocabulary.org/CaLAThe/LA_RRR">
		<skos:prefLabel xml:lang="en">LA_RRR</skos:prefLabel>
		<skos:scopeNote>ISO LADM term</skos:scopeNote>
		<skos:definition>LA_RRR is an abstract class with three specialization classes: LA_Right, with rights as instances, LA_Restriction, with restrictions as instances, and LA_Responsibility, with responsibilities as instances. In principle, all rights, restrictions and responsibilities are based on an administrative source, as instances from class LA_AdministrativeSource (Source: ISO LADM, 5.4).</skos:definition>
		<skos:changeNote>Established with version 3.</skos:changeNote>
		<skos:inScheme rdf:resource="http://www.cadastralvocabulary.org/CaLAThe"/>
		<skos:broader rdf:resource="http://www.cadastralvocabulary.org/CaLAThe/LandLaw"/>
	</skos:Concept>

	<skos:Concept rdf:about="http://www.cadastralvocabulary.org/CaLAThe/LA_Source">
		<skos:prefLabel xml:lang="en">LA_Source</skos:prefLabel>
		<skos:scopeNote>ISO LADM term</skos:scopeNote>
		<skos:definition>Document providing legal and/or administrative facts on which the land administration (LA) object [right (4.1.20), restriction (4.1.19), responsibility (4.1.18), basic administrative unit (4.1.2), party (4.1.13), or spatial unit (4.1.23)] is based on (Source: ISO LADM, 4.1.21).  </skos:definition>
		<skos:changeNote>Established with version 3.</skos:changeNote>
		<skos:exactMatch rdf:resource="http://aims.fao.org/aos/agrovoc/c_10265135"/>
		<skos:exactMatch rdf:resource="https://isotc211.geolexica.org/concepts/1574/"/>
		<skos:inScheme rdf:resource="http://www.cadastralvocabulary.org/CaLAThe"/>
		<skos:broader rdf:resource="http://www.cadastralvocabulary.org/CaLAThe/Document"/>
		<skos:narrower rdf:resource="http://www.cadastralvocabulary.org/CaLAThe/LA_AdministrativeSource"/>
		<skos:narrower rdf:resource="http://www.cadastralvocabulary.org/CaLAThe/LA_SpatialSource"/>
	</skos:Concept>

	<skos:Concept rdf:about="http://www.cadastralvocabulary.org/CaLAThe/LA_SpatialSource">
		<skos:prefLabel xml:lang="en">LA_SpatialSource</skos:prefLabel>
		<skos:scopeNote>ISO LADM term</skos:scopeNote>
		<skos:definition>Source (4.1.21) with the spatial representation of one (part of) or more spatial units (4.1.23) (Source: LADM, 2012, 4.1.22).</skos:definition>
		<skos:changeNote>Established with version 3.</skos:changeNote>
		<skos:exactMatch rdf:resource="http://aims.fao.org/aos/agrovoc/c_cf5b0fc7"/>
		<skos:exactMatch rdf:resource="https://isotc211.geolexica.org/concepts/1316/"/>
		<skos:inScheme rdf:resource="http://www.cadastralvocabulary.org/CaLAThe"/>
		<skos:broader rdf:resource="http://www.cadastralvocabulary.org/CaLAThe/LA_Source"/>
	</skos:Concept>

	<skos:Concept rdf:about="http://www.cadastralvocabulary.org/CaLAThe/Lease">
		<skos:prefLabel xml:lang="en">Lease</skos:prefLabel>
		<skos:prefLabel xml:lang="da">Lejemål, Forpagtning</skos:prefLabel>
		<skos:prefLabel xml:lang="ms">Pajakan</skos:prefLabel>
		<skos:definition>An Exchange between the Lessor and the Lessee that gives the Lessee certain rights over the Real property for a specified term and usually for a specified Rent.</skos:definition>
		<skos:changeNote>Established with version 2. Relation to Leasehold added with version 3.</skos:changeNote>
		<skos:exactMatch rdf:resource="http://aims.fao.org/aos/agrovoc/c_4240"/>
		<skos:exactMatch rdf:resource="https://www.eionet.europa.eu/gemet/en/concept/11611"/>
		<skos:exactMatch rdf:resource="http://eurovoc.europa.eu/4598"/>
		<skos:exactMatch rdf:resource="https://isotc211.geolexica.org/concepts/1230/"/>
		<skos:inScheme rdf:resource="http://www.cadastralvocabulary.org/CaLAThe"/>
		<skos:broader rdf:resource="http://www.cadastralvocabulary.org/CaLAThe/Exchange"/>
		<skos:related rdf:resource="http://www.cadastralvocabulary.org/CaLAThe/Leasehold"/>
	</skos:Concept>

	<skos:Concept rdf:about="http://www.cadastralvocabulary.org/CaLAThe/Leasehold">
		<skos:prefLabel xml:lang="en">Leasehold</skos:prefLabel>
		<skos:prefLabel xml:lang="da">Forpagtning</skos:prefLabel>
		<skos:prefLabel xml:lang="ms">Pegangan pajakan</skos:prefLabel>
		<skos:scopeNote>EULIS / ELRA term</skos:scopeNote>
		<skos:definition>The right to possess immovable property for an agreed period of time in return for an agreed consideration  (Source: EULIS / ELRA glossary).</skos:definition>
		<skos:changeNote>Established with version 3.</skos:changeNote>
		<skos:exactMatch rdf:resource="http://aims.fao.org/aos/agrovoc/c_d80e0cd0"/>
		<skos:inScheme rdf:resource="http://www.cadastralvocabulary.org/CaLAThe"/>
		<skos:broader rdf:resource="http://www.cadastralvocabulary.org/CaLAThe/RealRight"/>
		<skos:related rdf:resource="http://www.cadastralvocabulary.org/CaLAThe/Lease"/>
	</skos:Concept>

	<skos:Concept rdf:about="http://www.cadastralvocabulary.org/CaLAThe/LegalAdvisor">
		<skos:prefLabel xml:lang="en">Legal advisor</skos:prefLabel>
		<skos:prefLabel xml:lang="da">Juridisk rådgiver</skos:prefLabel>
		<skos:prefLabel xml:lang="tr">Yasal danışman</skos:prefLabel>
		<skos:prefLabel xml:lang="ms">Penasihat undang-undang</skos:prefLabel>
		<skos:changeNote>Established with version 1.</skos:changeNote>
		<skos:exactMatch rdf:resource="http://eurovoc.europa.eu/3989"/>
		<skos:inScheme rdf:resource="http://www.cadastralvocabulary.org/CaLAThe"/>
		<skos:broader rdf:resource="http://www.cadastralvocabulary.org/CaLAThe/Lawyer"/>
	</skos:Concept>

	<skos:Concept rdf:about="http://www.cadastralvocabulary.org/CaLAThe/LegalBoundaryDetermination">
		<skos:prefLabel xml:lang="en">Legal boundary determination</skos:prefLabel>
		<skos:prefLabel xml:lang="da">Skelforretning</skos:prefLabel>
		<skos:prefLabel xml:lang="tr">Hükmen sınır belirleme</skos:prefLabel>
		<skos:prefLabel xml:lang="ms">Penentuan sah sempadan</skos:prefLabel>
		<skos:changeNote>Established with version 2.</skos:changeNote>
		<skos:inScheme rdf:resource="http://www.cadastralvocabulary.org/CaLAThe"/>
		<skos:broader rdf:resource="http://www.cadastralvocabulary.org/CaLAThe/BoundarySurveyAndMarking"/>
	</skos:Concept>

	<skos:Concept rdf:about="http://www.cadastralvocabulary.org/CaLAThe/LegalPerson">
		<skos:prefLabel xml:lang="en">Legal person</skos:prefLabel>
		<skos:prefLabel xml:lang="da">Juridisk person</skos:prefLabel>
		<skos:prefLabel xml:lang="tr">Tüzel kişi</skos:prefLabel>
		<skos:prefLabel xml:lang="ms">Pengamal undang-undang</skos:prefLabel>
		<skos:definition>An Organisation endowed with a Legal personality.</skos:definition>
		<skos:changeNote>Established with version 1. Definition and relation to Organisation added with version 3. Broader edited with version 4. Definition changed with version 6.</skos:changeNote>
		<skos:exactMatch rdf:resource="http://eurovoc.europa.eu/2337"/>
		<skos:inScheme rdf:resource="http://www.cadastralvocabulary.org/CaLAThe"/>
		<skos:broader rdf:resource="http://www.cadastralvocabulary.org/CaLAThe/Organisation"/>
	</skos:Concept>

	<skos:Concept rdf:about="http://www.cadastralvocabulary.org/CaLAThe/LegalPersonality">
		<skos:prefLabel xml:lang="en">Legal personality</skos:prefLabel>
		<skos:prefLabel xml:lang="da">Retsevne, Retlig status</skos:prefLabel>
		<skos:prefLabel xml:lang="tr">Tüzel kişilik</skos:prefLabel>
		<skos:prefLabel xml:lang="ms">Personaliti undang-undang</skos:prefLabel>
		<skos:definition>The lawful characteristics and qualities of a Party.</skos:definition>
		<skos:changeNote>Established with version 1. Edited from Personal right to Legal personality with version 5 to comply with dictionaries, incl EuroVoc. Definition is added with version 6.</skos:changeNote>
		<skos:exactMatch rdf:resource="http://eurovoc.europa.eu/4274"/>
		<skos:inScheme rdf:resource="http://www.cadastralvocabulary.org/CaLAThe"/>
		<skos:broader rdf:resource="http://www.cadastralvocabulary.org/CaLAThe/NaturalPersonRole"/>
		<skos:narrower rdf:resource="http://www.cadastralvocabulary.org/CaLAThe/Signatory"/>
	</skos:Concept>

	<skos:Concept rdf:about="http://www.cadastralvocabulary.org/CaLAThe/Lessee">
		<skos:prefLabel xml:lang="en">Lessee</skos:prefLabel>
		<skos:prefLabel xml:lang="da">Forpagter</skos:prefLabel>
		<skos:prefLabel xml:lang="tr">Kiracı</skos:prefLabel>
		<skos:prefLabel xml:lang="ms">Penerima pajak</skos:prefLabel>
		<skos:scopeNote>EULIS / ELRA term</skos:scopeNote>
		<skos:definition>A Party to whom a Lease is granted.</skos:definition>
		<skos:changeNote>Established with version 3. Definition is changed with version 6.</skos:changeNote>
		<skos:inScheme rdf:resource="http://www.cadastralvocabulary.org/CaLAThe"/>
		<skos:broader rdf:resource="http://www.cadastralvocabulary.org/CaLAThe/RightsHolder"/>
	</skos:Concept>

	<skos:Concept rdf:about="http://www.cadastralvocabulary.org/CaLAThe/Lessor">
		<skos:prefLabel xml:lang="en">Lessor</skos:prefLabel>
		<skos:prefLabel xml:lang="da">Bortforpagter</skos:prefLabel>
		<skos:prefLabel xml:lang="tr">Kiraya veren</skos:prefLabel>
		<skos:prefLabel xml:lang="ms">Pemberi pajak</skos:prefLabel>
		<skos:scopeNote>EULIS / ELRA term</skos:scopeNote>
		<skos:definition>A Party who grants a Lease.</skos:definition>
		<skos:changeNote>Established with version 3. Definition is changed with version 6.</skos:changeNote>
		<skos:inScheme rdf:resource="http://www.cadastralvocabulary.org/CaLAThe"/>
		<skos:broader rdf:resource="http://www.cadastralvocabulary.org/CaLAThe/RightsHolder"/>
	</skos:Concept>

	<skos:Concept rdf:about="http://www.cadastralvocabulary.org/CaLAThe/LevelObservation">
		<skos:prefLabel xml:lang="en">Level observation</skos:prefLabel>
		<skos:prefLabel xml:lang="da">Højdemåling</skos:prefLabel>
		<skos:prefLabel xml:lang="tr">Düzey gözlemi</skos:prefLabel>
		<skos:prefLabel xml:lang="ms">Aras cerapan</skos:prefLabel>
		<skos:scopeNote>OGC LandInfra / InfraGML term</skos:scopeNote>
		<skos:changeNote>Established with version 4</skos:changeNote>
		<skos:inScheme rdf:resource="http://www.cadastralvocabulary.org/CaLAThe"/>
		<skos:broader rdf:resource="http://www.cadastralvocabulary.org/CaLAThe/LevelingInstrument"/>
		<skos:broader rdf:resource="http://www.cadastralvocabulary.org/CaLAThe/Observation"/>
	</skos:Concept>

	<skos:Concept rdf:about="http://www.cadastralvocabulary.org/CaLAThe/LevelingInstrument">
		<skos:prefLabel xml:lang="en">Leveling instrument</skos:prefLabel>
		<skos:prefLabel xml:lang="da">Nivellerinstrument</skos:prefLabel>
		<skos:prefLabel xml:lang="tr">Nivelman aracı</skos:prefLabel>
		<skos:prefLabel xml:lang="ms">Alat pengarasan</skos:prefLabel>
		<skos:definition>Level sensors are used to determine the height difference between two locations (OGC LandInfra 7.8.5.11)</skos:definition>
		<skos:changeNote>Established with version 4</skos:changeNote>
		<skos:exactMatch rdf:resource="http://docs.opengeospatial.org/is/15-111r1/15-111r1.html#146"/>
		<skos:inScheme rdf:resource="http://www.cadastralvocabulary.org/CaLAThe"/>
		<skos:broader rdf:resource="http://www.cadastralvocabulary.org/CaLAThe/SurveyingInstrument"/>
		<skos:narrower rdf:resource="http://www.cadastralvocabulary.org/CaLAThe/LevelObservation"/>
	</skos:Concept>

	<skos:Concept rdf:about="http://www.cadastralvocabulary.org/CaLAThe/LicensedSurveyor">
		<skos:prefLabel xml:lang="en">Licensed surveyor</skos:prefLabel>
		<skos:prefLabel xml:lang="da">Landinspektør med beskikkelse</skos:prefLabel>
		<skos:prefLabel xml:lang="tr">Lisanslı haritacı</skos:prefLabel>
		<skos:prefLabel xml:lang="ms">Juruukur berlesen</skos:prefLabel>
		<skos:scopeNote>OGC LandInfra / InfraGML term</skos:scopeNote>
		<skos:definition>A publicly appointed Surveyor, authorized to perform Property formation on behalf of the state.</skos:definition>
		<skos:changeNote>Established with version 1.  Definition is added with version 4, and changed with version 6.</skos:changeNote>
		<skos:inScheme rdf:resource="http://www.cadastralvocabulary.org/CaLAThe"/>
		<skos:broader rdf:resource="http://www.cadastralvocabulary.org/CaLAThe/Surveyor"/>
	</skos:Concept>

	<skos:Concept rdf:about="http://www.cadastralvocabulary.org/CaLAThe/Lien">
		<skos:prefLabel xml:lang="en">Lien</skos:prefLabel>
		<skos:prefLabel xml:lang="da">Tilbageholdsret</skos:prefLabel>
		<skos:prefLabel xml:lang="tr">Rehin hakkı</skos:prefLabel>
		<skos:prefLabel xml:lang="ms">Lien</skos:prefLabel>
		<skos:changeNote>Established with version 3.</skos:changeNote>
		<skos:inScheme rdf:resource="http://www.cadastralvocabulary.org/CaLAThe"/>
		<skos:broader rdf:resource="http://www.cadastralvocabulary.org/CaLAThe/Mortgage"/>
	</skos:Concept>

	<skos:Concept rdf:about="http://www.cadastralvocabulary.org/CaLAThe/Liminal">
		<skos:prefLabel xml:lang="en">Liminal</skos:prefLabel>
		<skos:scopeNote>ISO 19152:2012 and OGC LandInfra / InfraGML term</skos:scopeNote>
		<skos:definition>Spatial unit on the threshold between 2D and 3D representationsm (ISO 19152:2012, 4.1.12, cf. OGC LandInfra 7.10.6 SpatialUnit)</skos:definition>
		<skos:changeNote>Established with version 4. Added definition with version 6.</skos:changeNote>
		<skos:inScheme rdf:resource="http://www.cadastralvocabulary.org/CaLAThe"/>
		<skos:broader rdf:resource="http://www.cadastralvocabulary.org/CaLAThe/DimensionType"/>
	</skos:Concept>

	<skos:Concept rdf:about="http://www.cadastralvocabulary.org/CaLAThe/LimitedRight">
		<skos:prefLabel xml:lang="en">Limited right</skos:prefLabel>
		<skos:prefLabel xml:lang="da">Begrænset ejendomsret</skos:prefLabel>
		<skos:prefLabel xml:lang="tr">Sınırlı ayni hak</skos:prefLabel>
		<skos:prefLabel xml:lang="ms">Hak terhad</skos:prefLabel>
		<skos:changeNote>Established with version 3.</skos:changeNote>
		<skos:inScheme rdf:resource="http://www.cadastralvocabulary.org/CaLAThe"/>
		<skos:broader rdf:resource="http://www.cadastralvocabulary.org/CaLAThe/RealRight"/>
		<skos:narrower rdf:resource="http://www.cadastralvocabulary.org/CaLAThe/Usufruct"/>
		<skos:narrower rdf:resource="http://www.cadastralvocabulary.org/CaLAThe/Easement"/>
		<skos:narrower rdf:resource="http://www.cadastralvocabulary.org/CaLAThe/SecurityInterest"/>
		<skos:narrower rdf:resource="http://www.cadastralvocabulary.org/CaLAThe/LA_Restriction"/>
	</skos:Concept>

	<skos:Concept rdf:about="http://www.cadastralvocabulary.org/CaLAThe/LineString">
		<skos:prefLabel xml:lang="en">Line string</skos:prefLabel>
		<skos:prefLabel xml:lang="da">Kurve, Dannet af rette linjer</skos:prefLabel>
		<skos:prefLabel xml:lang="tr">Düz çizgi</skos:prefLabel>
		<skos:prefLabel xml:lang="ms">Rantaian garisan</skos:prefLabel>
		<skos:scopeNote>Geolexica term</skos:scopeNote>
		<skos:definition>Curve composed of straight-line segments (Geolexica ISO 19136-1:2020)</skos:definition>
		<skos:changeNote>Established with version 4</skos:changeNote>
		<skos:exactMatch rdf:resource="https://isotc211.geolexica.org/concepts/270/"/>
		<skos:inScheme rdf:resource="http://www.cadastralvocabulary.org/CaLAThe"/>
		<skos:broader rdf:resource="http://www.cadastralvocabulary.org/CaLAThe/Curve"/>
		<skos:broader rdf:resource="http://www.cadastralvocabulary.org/CaLAThe/BEString"/>
		<skos:narrower rdf:resource="http://www.cadastralvocabulary.org/CaLAThe/Point"/>
	</skos:Concept>

	<skos:Concept rdf:about="http://www.cadastralvocabulary.org/CaLAThe/LI_LandSurveyor">
		<skos:prefLabel xml:lang="en">LI_LandSurveyor</skos:prefLabel>
		<skos:scopeNote>OGC LandInfra</skos:scopeNote>
		<skos:changeNote>Established with version 4</skos:changeNote>
		<skos:inScheme rdf:resource="http://www.cadastralvocabulary.org/CaLAThe"/>
		<skos:broader rdf:resource="http://www.cadastralvocabulary.org/CaLAThe/Surveyor"/>
		<skos:broader rdf:resource="http://www.cadastralvocabulary.org/CaLAThe/Signatory"/>
	</skos:Concept>

	<skos:Concept rdf:about="http://www.cadastralvocabulary.org/CaLAThe/LI_Sensor">
		<skos:prefLabel xml:lang="en">LI_Sensor</skos:prefLabel>
		<skos:scopeNote>OGC LandInfra / InfraGML term</skos:scopeNote>
		<skos:definition>Element of a measuring system that is directly affected by a phenomenon, body, or substance carrying a quantity to be measured (Source: ISO/TC 211 Glossary of Terms - English).</skos:definition>
		<skos:changeNote>Established with version 4</skos:changeNote>
		<skos:exactMatch rdf:resource="https://isotc211.geolexica.org/concepts/1108/"/>
		<skos:inScheme rdf:resource="http://www.cadastralvocabulary.org/CaLAThe"/>
		<skos:broader rdf:resource="http://www.cadastralvocabulary.org/CaLAThe/SurveyingInstrument"/>
	</skos:Concept>

	<skos:Concept rdf:about="http://www.cadastralvocabulary.org/CaLAThe/MainParcel">
		<skos:prefLabel xml:lang="en">Main Parcel</skos:prefLabel>
		<skos:prefLabel xml:lang="da">Hovedparcel</skos:prefLabel>
		<skos:prefLabel xml:lang="tr">Ana parsel (taşınmaz)</skos:prefLabel>
		<skos:prefLabel xml:lang="ms">Petak utama</skos:prefLabel>
		<skos:scopeNote>OGC LandInfra / InfraGML term</skos:scopeNote>
		<skos:definition>Optional indication of a current LandParcel which is part of a LandPropertyUnit with more LandParcels, and which is chosen as reference for all LandParcels in the LandPropertyUnit. May be applied in jurisdictions where legal provisions do not recognize the concept of LandPropertyUnit (LandInfra 7.10.2.5)</skos:definition>
		<skos:changeNote>Established with version 4</skos:changeNote>
		<skos:inScheme rdf:resource="http://www.cadastralvocabulary.org/CaLAThe"/>
		<skos:broader rdf:resource="http://www.cadastralvocabulary.org/CaLAThe/CadastralParcel"/>
	</skos:Concept>

	<skos:Concept rdf:about="http://www.cadastralvocabulary.org/CaLAThe/Map">
		<skos:prefLabel xml:lang="en">Map</skos:prefLabel>
		<skos:prefLabel xml:lang="da">Kort, Landkort</skos:prefLabel>
		<skos:prefLabel xml:lang="tr">Harita</skos:prefLabel>
		<skos:prefLabel xml:lang="ms">Peta</skos:prefLabel>
		<skos:scopeNote>GEMET term</skos:scopeNote>
		<skos:definition>A representation, normally on a flat medium, that displays the physical and political features of a surface area of the earth, showing them in their respective forms, sizes and relationships according to some convention of representation.</skos:definition>
		<skos:changeNote>Established with version 1.</skos:changeNote>
		<skos:exactMatch rdf:resource="http://www.eionet.europa.eu/gemet/concept/5011"/>
		<skos:exactMatch rdf:resource="http://aims.fao.org/aos/agrovoc/c_b43d8acf"/>
		<skos:exactMatch rdf:resource="http://zbw.eu/stw/descriptor/14814-1"/>
		<skos:inScheme rdf:resource="http://www.cadastralvocabulary.org/CaLAThe"/>
		<skos:broader rdf:resource="http://www.cadastralvocabulary.org/CaLAThe/GeolocatedInformation"/>
		<skos:narrower rdf:resource="http://www.cadastralvocabulary.org/CaLAThe/CadastralMap"/>
		<skos:narrower rdf:resource="http://www.cadastralvocabulary.org/CaLAThe/TopographicMap"/>
	</skos:Concept>

	<skos:Concept rdf:about="http://www.cadastralvocabulary.org/CaLAThe/Marker">
		<skos:prefLabel xml:lang="en">Marker</skos:prefLabel>
		<skos:prefLabel xml:lang="da">Markør</skos:prefLabel>
		<skos:prefLabel xml:lang="tr">Sınır işareti</skos:prefLabel>
		<skos:prefLabel xml:lang="ms">Penanda</skos:prefLabel>
		<skos:definition>Pole, plate, or other, used for marking and/or naming a location.</skos:definition>
		<skos:changeNote>Established with version 1. Definition is added in version 5.</skos:changeNote>
		<skos:inScheme rdf:resource="http://www.cadastralvocabulary.org/CaLAThe"/>
		<skos:broader rdf:resource="http://www.cadastralvocabulary.org/CaLAThe/LandDivision"/>
		<skos:narrower rdf:resource="http://www.cadastralvocabulary.org/CaLAThe/SurveyMark"/>
		<skos:narrower rdf:resource="http://www.cadastralvocabulary.org/CaLAThe/StreetSign"/>
	</skos:Concept>

	<skos:Concept rdf:about="http://www.cadastralvocabulary.org/CaLAThe/MeasuringTape">
		<skos:prefLabel xml:lang="en">Measuring tape</skos:prefLabel>
		<skos:prefLabel xml:lang="da">Målebånd</skos:prefLabel>
		<skos:prefLabel xml:lang="tr">Şerit metre</skos:prefLabel>
		<skos:prefLabel xml:lang="ms">Pita ukur</skos:prefLabel>
		<skos:changeNote>Established with version 4</skos:changeNote>
		<skos:inScheme rdf:resource="http://www.cadastralvocabulary.org/CaLAThe"/>
		<skos:broader rdf:resource="http://www.cadastralvocabulary.org/CaLAThe/SurveyingInstrument"/>
		<skos:narrower rdf:resource="http://www.cadastralvocabulary.org/CaLAThe/DistanceObservation"/>
	</skos:Concept>

	<skos:Concept rdf:about="http://www.cadastralvocabulary.org/CaLAThe/Metadata">
		<skos:prefLabel xml:lang="en">Metadata</skos:prefLabel>
		<skos:prefLabel xml:lang="da">Metadata</skos:prefLabel>
		<skos:prefLabel xml:lang="tr">Metaveri</skos:prefLabel>
		<skos:prefLabel xml:lang="ms">Metadata</skos:prefLabel>
		<skos:scopeNote>ISO 19115-1</skos:scopeNote>
		<skos:definition>Information about a resource. (Source:  ISO 19115-1:2014, 4.10)</skos:definition>
		<skos:changeNote>Established with version 2. Broader relation changed with version 3 and 4</skos:changeNote>
		<skos:exactMatch rdf:resource="https://www.geolexica.org/concepts/1650/"/>
		<skos:exactMatch rdf:resource="http://aims.fao.org/aos/agrovoc/c_49829"/>
		<skos:exactMatch rdf:resource="http://eurovoc.europa.eu/c_40f54e0c"/>
		<skos:inScheme rdf:resource="http://www.cadastralvocabulary.org/CaLAThe"/>
		<skos:broader rdf:resource="http://www.cadastralvocabulary.org/CaLAThe/Information"/>
	</skos:Concept>

	<skos:Concept rdf:about="http://www.cadastralvocabulary.org/CaLAThe/Mortgage">
		<skos:prefLabel xml:lang="en">Mortgage</skos:prefLabel>
		<skos:prefLabel xml:lang="da">Pantehæftelse</skos:prefLabel>
		<skos:prefLabel xml:lang="tr">İpote</skos:prefLabel>
		<skos:prefLabel xml:lang="ms">Gadai janji</skos:prefLabel>
		<skos:scopeNote>STW Thesaurus for Economics term</skos:scopeNote>
		<skos:definition>A security right to secure payment of a debt or other financial obligation (Source: EULIS / ELRA glossary).</skos:definition>
		<skos:changeNote>Established with version 1. Changed with v3 as narrower of Security right.</skos:changeNote>
		<skos:exactMatch rdf:resource="http://zbw.eu/stw/descriptor/13775-4"/>
		<skos:exactMatch rdf:resource="http://aims.fao.org/aos/agrovoc/c_4946"/>
		<skos:exactMatch rdf:resource="http://eurovoc.europa.eu/1281"/>
		<skos:inScheme rdf:resource="http://www.cadastralvocabulary.org/CaLAThe"/>
		<skos:altLabel>LA_Mortgage</skos:altLabel>
		<skos:broader rdf:resource="http://www.cadastralvocabulary.org/CaLAThe/SecurityInterest"/>
		<skos:narrower rdf:resource="http://www.cadastralvocabulary.org/CaLAThe/Lien"/>
	</skos:Concept>

	<skos:Concept rdf:about="http://www.cadastralvocabulary.org/CaLAThe/MortgageDeed">
		<skos:prefLabel xml:lang="en">Mortgage deed</skos:prefLabel>
		<skos:prefLabel xml:lang="da">Pantebrev</skos:prefLabel>
		<skos:prefLabel xml:lang="tr">İpotek sözleşmesi</skos:prefLabel>
		<skos:prefLabel xml:lang="ms">Surat ikatan gadai janji</skos:prefLabel>
		<skos:changeNote>Established with version 1.</skos:changeNote>
		<skos:inScheme rdf:resource="http://www.cadastralvocabulary.org/CaLAThe"/>
		<skos:broader rdf:resource="http://www.cadastralvocabulary.org/CaLAThe/Deed"/>
	</skos:Concept>

	<skos:Concept rdf:about="http://www.cadastralvocabulary.org/CaLAThe/Mortgagee">
		<skos:prefLabel xml:lang="en">Mortgagee</skos:prefLabel>
		<skos:prefLabel xml:lang="da">Panthaver</skos:prefLabel>
		<skos:prefLabel xml:lang="tr">İpote alacaklısı</skos:prefLabel>
		<skos:prefLabel xml:lang="ms">Pemegang gadai janji</skos:prefLabel>
		<skos:definition>A Party that lends money through a Mortgage loan and thus obtain legal mortgage in Real property as collateral for the loan.</skos:definition>
		<skos:changeNote>Established with version 1. Definition is added with version 6.</skos:changeNote>
		<skos:inScheme rdf:resource="http://www.cadastralvocabulary.org/CaLAThe"/>
		<skos:broader rdf:resource="http://www.cadastralvocabulary.org/CaLAThe/RightsHolder"/>
	</skos:Concept>

	<skos:Concept rdf:about="http://www.cadastralvocabulary.org/CaLAThe/Mortgaging">
		<skos:prefLabel xml:lang="en">Mortgaging</skos:prefLabel>
		<skos:prefLabel xml:lang="da">Pantsætning</skos:prefLabel>
		<skos:prefLabel xml:lang="tr">İpotek tesisi</skos:prefLabel>
		<skos:prefLabel xml:lang="ms">Menggadaikan</skos:prefLabel>
		<skos:definition>An Exchange between a Mortgagee (or creditor) and a Mortgagor (debtor) implying a loan of money for which re-payment is secured by giving the Mortgagee the right to sell the concerned Real property and keep the value of unpaid mortgage and interest, when the loan is not paid off in accordance with the agreed stipulations. </skos:definition>
		<skos:changeNote>Established with version 2.</skos:changeNote>
		<skos:inScheme rdf:resource="http://www.cadastralvocabulary.org/CaLAThe"/>
		<skos:broader rdf:resource="http://www.cadastralvocabulary.org/CaLAThe/Exchange"/>
	</skos:Concept>

	<skos:Concept rdf:about="http://www.cadastralvocabulary.org/CaLAThe/Mortgagor">
		<skos:prefLabel xml:lang="en">Mortgagor</skos:prefLabel>
		<skos:prefLabel xml:lang="da">Låntager</skos:prefLabel>
		<skos:prefLabel xml:lang="tr">İpotek borçlusu</skos:prefLabel>
		<skos:prefLabel xml:lang="ms">Penggadai</skos:prefLabel>
		<skos:definition>A Party that borrows money through a Mortgage loan and thus pledge Real property as collateral for the loan.</skos:definition>
		<skos:changeNote>Established with version 2. Definition is added with version 6.</skos:changeNote>
		<skos:inScheme rdf:resource="http://www.cadastralvocabulary.org/CaLAThe"/>
		<skos:broader rdf:resource="http://www.cadastralvocabulary.org/CaLAThe/RightsHolder"/>
	</skos:Concept>

	<skos:Concept rdf:about="http://www.cadastralvocabulary.org/CaLAThe/NaturalLaw">
		<skos:prefLabel xml:lang="en">Natural law</skos:prefLabel>
		<skos:prefLabel xml:lang="da">Naturret</skos:prefLabel>
		<skos:prefLabel xml:lang="tr">Doğal hukuk</skos:prefLabel>
		<skos:prefLabel xml:lang="ms">Undang-undang semula jadi</skos:prefLabel>
		<skos:definition>Determinism qualifying the law in a State where the legal order is not established by convention (Source: Legal Dictionary of Property in Canada - Dualjuridik).</skos:definition>
		<skos:changeNote>Established with version 3.</skos:changeNote>
		<skos:exactMatch rdf:resource="http://zbw.eu/stw/descriptor/15965-3"/>
		<skos:exactMatch rdf:resource="http://eurovoc.europa.eu/7399"/>
		<skos:inScheme rdf:resource="http://www.cadastralvocabulary.org/CaLAThe"/>
		<skos:broader rdf:resource="http://www.cadastralvocabulary.org/CaLAThe/Law"/>
	</skos:Concept>

	<skos:Concept rdf:about="http://www.cadastralvocabulary.org/CaLAThe/NaturalPerson">
		<skos:prefLabel xml:lang="en">Natural person</skos:prefLabel>
		<skos:prefLabel xml:lang="da">Fysisk person</skos:prefLabel>
		<skos:prefLabel xml:lang="tr">Gerçek kişi</skos:prefLabel>
		<skos:prefLabel xml:lang="ms">Manusia biasa</skos:prefLabel>
		<skos:definition>Individual human being.</skos:definition>
		<skos:changeNote>Established with version 1. Narrower to Legal subject deleted with ver. 5; replaced by Legal personality. Definition is added with version 6.</skos:changeNote>
		<skos:exactMatch rdf:resource="http://eurovoc.europa.eu/2338"/>
		<skos:inScheme rdf:resource="http://www.cadastralvocabulary.org/CaLAThe"/>
		<skos:broader rdf:resource="http://www.cadastralvocabulary.org/CaLAThe/PartyType"/>
	</skos:Concept>

	<skos:Concept rdf:about="http://www.cadastralvocabulary.org/CaLAThe/NaturalPersonRole">
		<skos:prefLabel xml:lang="en">Natural person role</skos:prefLabel>
		<skos:prefLabel xml:lang="da">Rolle for fysisk person</skos:prefLabel>
		<skos:prefLabel xml:lang="tr">Gerçek kişi rolü</skos:prefLabel>
		<skos:prefLabel xml:lang="ms">Peranan manusia biasa</skos:prefLabel>
		<skos:definition>A Party role type which an individual human being may play.</skos:definition>
		<skos:changeNote>Established with version 1. Definition is added with version 6.</skos:changeNote>
		<skos:inScheme rdf:resource="http://www.cadastralvocabulary.org/CaLAThe"/>
		<skos:broader rdf:resource="http://www.cadastralvocabulary.org/CaLAThe/PartyRoleType"/>
		<skos:narrower rdf:resource="http://www.cadastralvocabulary.org/CaLAThe/OfficialRole"/>
		<skos:narrower rdf:resource="http://www.cadastralvocabulary.org/CaLAThe/SocietalRole"/>
		<skos:narrower rdf:resource="http://www.cadastralvocabulary.org/CaLAThe/Professional"/>
		<skos:narrower rdf:resource="http://www.cadastralvocabulary.org/CaLAThe/LegalPersonality"/>
	</skos:Concept>

	<skos:Concept rdf:about="http://www.cadastralvocabulary.org/CaLAThe/Neighbor">
		<skos:prefLabel xml:lang="en">Neighbor</skos:prefLabel>
		<skos:prefLabel xml:lang="da">Nabo</skos:prefLabel>
		<skos:prefLabel xml:lang="tr">Komşu</skos:prefLabel>
		<skos:prefLabel xml:lang="ms">Jiran</skos:prefLabel>
		<skos:definition>Natural persons, Groups and Organisations who share boundary or are located in the neighbourhood.</skos:definition>
		<skos:changeNote>Established with version 4. Context changed with version 5 (no relation to Signatory). Definition is added with version 6.</skos:changeNote>
		<skos:inScheme rdf:resource="http://www.cadastralvocabulary.org/CaLAThe"/>
		<skos:broader rdf:resource="http://www.cadastralvocabulary.org/CaLAThe/SocietalRole"/>
	</skos:Concept>

	<skos:Concept rdf:about="http://www.cadastralvocabulary.org/CaLAThe/Node">
		<skos:prefLabel xml:lang="en">Node</skos:prefLabel>
		<skos:prefLabel xml:lang="da">Knude</skos:prefLabel>
		<skos:prefLabel xml:lang="tr">Düğüm noktası</skos:prefLabel>
		<skos:prefLabel xml:lang="ms">Nod</skos:prefLabel>
		<skos:scopeNote>ISO 19107:2019</skos:scopeNote>
		<skos:definition>0-dimensional topological primitive (ISO 19107:2019, (E), 3.69)</skos:definition>
		<skos:changeNote>Established with version 1. Edited with versions 4 and 6</skos:changeNote>
		<skos:exactMatch rdf:resource="https://isotc211.geolexica.org/concepts/309/"/>
		<skos:exactMatch rdf:resource="http://aims.fao.org/aos/agrovoc/c_5204"/>
		<skos:inScheme rdf:resource="http://www.cadastralvocabulary.org/CaLAThe"/>
		<skos:broader rdf:resource="http://www.cadastralvocabulary.org/CaLAThe/TopologicalPrimitive"/>
		<skos:narrower rdf:resource="http://www.cadastralvocabulary.org/CaLAThe/LA_NodeBasedSpatialUnit"/>
	</skos:Concept>

	<skos:Concept rdf:about="http://www.cadastralvocabulary.org/CaLAThe/Notary">
		<skos:prefLabel xml:lang="en">Notary</skos:prefLabel>
		<skos:prefLabel xml:lang="da">Notar</skos:prefLabel>
		<skos:prefLabel xml:lang="tr">Noter</skos:prefLabel>
		<skos:prefLabel xml:lang="ms">Notari</skos:prefLabel>
		<skos:definition>A public Official who is authorized to authenticate Deeds and other Documents by an appropriate certificate on behalf of the state.</skos:definition>
		<skos:changeNote>Established with version 1. Definition is added with version 6.</skos:changeNote>
		<skos:exactMatch rdf:resource="http://aims.fao.org/aos/agrovoc/c_72efbdb8"/>
		<skos:exactMatch rdf:resource="http://eurovoc.europa.eu/2085"/>
		<skos:inScheme rdf:resource="http://www.cadastralvocabulary.org/CaLAThe"/>
		<skos:broader rdf:resource="http://www.cadastralvocabulary.org/CaLAThe/Professional"/>
	</skos:Concept>

	<skos:Concept rdf:about="http://www.cadastralvocabulary.org/CaLAThe/NUTSRegion">
		<skos:prefLabel xml:lang="en">NUTS Region</skos:prefLabel>
		<skos:prefLabel xml:lang="da">Regional statistikenhed</skos:prefLabel>
		<skos:prefLabel xml:lang="tr">İstatistiki Bölge Birimleri</skos:prefLabel>
		<skos:prefLabel xml:lang="ms">Wilayah NUTS</skos:prefLabel>
		<skos:scopeNote>INSPIRE term</skos:scopeNote>
		<skos:definition>Territorial unit for statistics defined in the framework of the Regulation (EC) No 1059/2003 of the European Parliament and of the Council of 26 May 2003 (INSPIRE feature concept dictionary).</skos:definition>
		<skos:changeNote>Established with version 2.</skos:changeNote>
		<skos:exactMatch rdf:resource="http://inspire.ec.europa.eu/featureconcept/NUTSRegion"/>
		<skos:inScheme rdf:resource="http://www.cadastralvocabulary.org/CaLAThe"/>
		<skos:broader rdf:resource="http://www.cadastralvocabulary.org/CaLAThe/AdministrativeUnit"/>
	</skos:Concept>

	<skos:Concept rdf:about="http://www.cadastralvocabulary.org/CaLAThe/Observation">
		<skos:prefLabel xml:lang="en">Observation</skos:prefLabel>
		<skos:prefLabel xml:lang="da">Observation</skos:prefLabel>
		<skos:prefLabel xml:lang="tr">Gözlem</skos:prefLabel>
		<skos:prefLabel xml:lang="ms">Pemerhatian, cerapan</skos:prefLabel>
		<skos:scopeNote>OGC LandInfra / InfraGML term</skos:scopeNote>
		<skos:definition>Act of measuring or otherwise determining the value of a property (Source: ISO 19156:2011, 4.11).</skos:definition>
		<skos:changeNote>Established with version 4</skos:changeNote>
		<skos:exactMatch rdf:resource="http://aims.fao.org/aos/agrovoc/c_fc54b25b"/>
		<skos:exactMatch rdf:resource="http://eurovoc.europa.eu/2085"/>
		<skos:inScheme rdf:resource="http://www.cadastralvocabulary.org/CaLAThe"/>
		<skos:broader rdf:resource="http://www.cadastralvocabulary.org/CaLAThe/SurveyingInstrument"/>
		<skos:narrower rdf:resource="http://www.cadastralvocabulary.org/CaLAThe/DistanceObservation"/>
		<skos:narrower rdf:resource="http://www.cadastralvocabulary.org/CaLAThe/AngelObservation"/>
		<skos:narrower rdf:resource="http://www.cadastralvocabulary.org/CaLAThe/TPSobservation"/>
		<skos:narrower rdf:resource="http://www.cadastralvocabulary.org/CaLAThe/LevelObservation"/>
		<skos:narrower rdf:resource="http://www.cadastralvocabulary.org/CaLAThe/GNSSobservation"/>
		<skos:narrower rdf:resource="http://www.cadastralvocabulary.org/CaLAThe/Correction"/>
	</skos:Concept>

	<skos:Concept rdf:about="http://www.cadastralvocabulary.org/CaLAThe/OfficialRole">
		<skos:prefLabel xml:lang="en">Official role</skos:prefLabel>
		<skos:prefLabel xml:lang="da">Embedsmand</skos:prefLabel>
		<skos:prefLabel xml:lang="tr">Resmi rol</skos:prefLabel>
		<skos:prefLabel xml:lang="ms">Peranan rasmi</skos:prefLabel>
		<skos:definition>A Natural person who has a position of responsibility in a governmental organization.</skos:definition>
		<skos:changeNote>Established with version 1. Alternative label is added with version 3, and then removed with version 4. Definition is added with version 6.</skos:changeNote>
		<skos:inScheme rdf:resource="http://www.cadastralvocabulary.org/CaLAThe"/>
		<skos:broader rdf:resource="http://www.cadastralvocabulary.org/CaLAThe/NaturalPersonRole"/>
		<skos:narrower rdf:resource="http://www.cadastralvocabulary.org/CaLAThe/Registrar"/>
	</skos:Concept>

	<skos:Concept rdf:about="http://www.cadastralvocabulary.org/CaLAThe/OptionToPurchase">
		<skos:prefLabel xml:lang="en">Option to purchase</skos:prefLabel>
		<skos:prefLabel xml:lang="da">Køberet</skos:prefLabel>
		<skos:prefLabel xml:lang="tr">Alım hakkı</skos:prefLabel>
		<skos:prefLabel xml:lang="ms">Opsyen beli</skos:prefLabel>
		<skos:scopeNote>EULIS / ELRA term.</skos:scopeNote>
		<skos:definition>A right that entitles a person to compel the owner to sell or grant the property, but does not impose on him any duty to buy (EULIS / ELRA glossary).</skos:definition>
		<skos:changeNote>Established with version 3.</skos:changeNote>
		<skos:inScheme rdf:resource="http://www.cadastralvocabulary.org/CaLAThe"/>
		<skos:broader rdf:resource="http://www.cadastralvocabulary.org/CaLAThe/LawOfObligation"/>
	</skos:Concept>

	<skos:Concept rdf:about="http://www.cadastralvocabulary.org/CaLAThe/OrdinalScale">
		<skos:prefLabel xml:lang="en">Ordinal scale</skos:prefLabel>
		<skos:prefLabel xml:lang="da">Ordinalskala</skos:prefLabel>
		<skos:prefLabel xml:lang="tr">Ordinal ölçek</skos:prefLabel>
		<skos:prefLabel xml:lang="ms">Skala ordinal</skos:prefLabel>
		<skos:scopeNote>Stevens, S. S. (7 June 1946). "On the Theory of Scales of Measurement". Science. 103 (2684): 677-680. ISO 19108:2002</skos:scopeNote>
		<skos:definition>Scale which provides a basis for measuring only the relative position of an object. (ISO 19108:2002) Note: The ordinal scale may be used for ordering of geospatial features, e.g. floors/ stories, or elements of a road network</skos:definition>
		<skos:changeNote>Established with version 1. Definition added with version 5. Term edited from Ordinal reference frame to Ordinal scale, and definition edited to reflect ISO 19108:2002 with version 6.</skos:changeNote>
		<skos:exactMatch rdf:resource="https://isotc211.geolexica.org/concepts/322/"/>
		<skos:inScheme rdf:resource="http://www.cadastralvocabulary.org/CaLAThe"/>
		<skos:broader rdf:resource="http://www.cadastralvocabulary.org/CaLAThe/SpatialReference"/>
	</skos:Concept>

	<skos:Concept rdf:about="http://www.cadastralvocabulary.org/CaLAThe/Organisation">
		<skos:prefLabel xml:lang="en">Organisation</skos:prefLabel>
		<skos:prefLabel xml:lang="da">Organisation</skos:prefLabel>
		<skos:prefLabel xml:lang="tr">Kuruluş</skos:prefLabel>
		<skos:prefLabel xml:lang="ms">Organisasi</skos:prefLabel>
		<skos:scopeNote>GEMET term</skos:scopeNote>
		<skos:definition>A purpose-oriented administrative and functional structure, specified in writing.</skos:definition>
		<skos:changeNote>Established with version 1. Relation to Legal person added in version 3 and edited to Narrower in version 4. Definition supplemented in version 4, and changed in version 6.</skos:changeNote>
		<skos:exactMatch rdf:resource="http://aims.fao.org/aos/agrovoc/c_37968"/>
		<skos:exactMatch rdf:resource="http://www.eionet.europa.eu/gemet/concept/13286"/>
		<skos:exactMatch rdf:resource="http://zbw.eu/stw/descriptor/12091-4"/>
		<skos:inScheme rdf:resource="http://www.cadastralvocabulary.org/CaLAThe"/>
		<skos:broader rdf:resource="http://www.cadastralvocabulary.org/CaLAThe/PartyType"/>
		<skos:narrower rdf:resource="http://www.cadastralvocabulary.org/CaLAThe/GovernmentalOrganisation"/>
		<skos:narrower rdf:resource="http://www.cadastralvocabulary.org/CaLAThe/Judiciary"/>
		<skos:narrower rdf:resource="http://www.cadastralvocabulary.org/CaLAThe/Corporation"/>
		<skos:narrower rdf:resource="http://www.cadastralvocabulary.org/CaLAThe/Association"/>
		<skos:narrower rdf:resource="http://www.cadastralvocabulary.org/CaLAThe/LegalPerson"/>
	</skos:Concept>

	<skos:Concept rdf:about="http://www.cadastralvocabulary.org/CaLAThe/Orthoimagery">
		<skos:prefLabel xml:lang="en">Orthoimagery</skos:prefLabel>
		<skos:prefLabel xml:lang="da">Ortofoto</skos:prefLabel>
		<skos:prefLabel xml:lang="tr">Ortogörüntü</skos:prefLabel>
		<skos:prefLabel xml:lang="ms">Ortoimej</skos:prefLabel>
		<skos:scopeNote>INSPIRE term</skos:scopeNote>
		<skos:definition>Georeferenced image data of the Earths surface, from either satellite or airborne sensors.</skos:definition>
		<skos:changeNote>Established with version 1. Definition added and matches edited with version 6.</skos:changeNote>
		<skos:exactMatch rdf:resource="https://inspire.ec.europa.eu/theme/oi"/>
		<skos:inScheme rdf:resource="http://www.cadastralvocabulary.org/CaLAThe"/>
		<skos:broader rdf:resource="http://www.cadastralvocabulary.org/CaLAThe/DigitalImagery"/>
	</skos:Concept>

	<skos:Concept rdf:about="http://www.cadastralvocabulary.org/CaLAThe/Owner">
		<skos:prefLabel xml:lang="en">Owner</skos:prefLabel>
		<skos:prefLabel xml:lang="da">Ejer</skos:prefLabel>
		<skos:prefLabel xml:lang="tr">Malik, Sahip</skos:prefLabel>
		<skos:prefLabel xml:lang="ms">Pemilik</skos:prefLabel>
		<skos:scopeNote>STW Thesaurus for Economics term</skos:scopeNote>
		<skos:definition>Subject of ownership and holder of the prerogatives that are attached to it (Source: Legal Dictionary of Property in Canada - Dualjuridik).</skos:definition>
		<skos:changeNote>Established with version 1. Definition added with version 3.</skos:changeNote>
		<skos:exactMatch rdf:resource="http://zbw.eu/stw/descriptor/19161-2"/>
		<skos:exactMatch rdf:resource="http://data.europa.eu/snb/verification/1faf8d450f"/>
		<skos:exactMatch rdf:resource="https://isotc211.geolexica.org/concepts/1241/"/>
		<skos:inScheme rdf:resource="http://www.cadastralvocabulary.org/CaLAThe"/>
		<skos:broader rdf:resource="http://www.cadastralvocabulary.org/CaLAThe/RightsHolder"/>
		<skos:broader rdf:resource="http://www.cadastralvocabulary.org/CaLAThe/Signatory"/>
		<skos:narrower rdf:resource="http://www.cadastralvocabulary.org/CaLAThe/Title"/>
	</skos:Concept>

	<skos:Concept rdf:about="http://www.cadastralvocabulary.org/CaLAThe/Ownership">
		<skos:prefLabel xml:lang="en">Ownership</skos:prefLabel>
		<skos:prefLabel xml:lang="da">Ejendomsret (til fast ejendom)</skos:prefLabel>
		<skos:prefLabel xml:lang="tr">Mülkiyet</skos:prefLabel>
		<skos:prefLabel xml:lang="ms">Pemilikan</skos:prefLabel>
		<skos:scopeNote>GEMET term</skos:scopeNote>
		<skos:definition>Collection of rights to use and enjoy property, including right to transmit it to others. The complete dominion, title, or proprietary right in a thing or claim (Source: Black, 1991). Possessive relationship with a title established between an owner and their property (Source: Legal Dictionary of Property in Canada - Dualjuridik). Includes the right to grant a lease, an easement, or a security interest and other lesser rights. Ownership in land includes buildings and fixture on the land parcel, unless lawful process is performed in terms of establishment of condominium units  (Source: OGC LandInfra, 4.8.13)</skos:definition>
		<skos:changeNote>Established with version 1. Changed and defined with version 3.</skos:changeNote>
		<skos:exactMatch rdf:resource="http://aims.fao.org/aos/agrovoc/c_5466"/>
		<skos:exactMatch rdf:resource="https://www.eionet.europa.eu/gemet/en/concept/5971"/>
		<skos:exactMatch rdf:resource="http://zbw.eu/stw/descriptor/10005-5"/>
		<skos:exactMatch rdf:resource="http://eurovoc.europa.eu/3929"/>
		<skos:inScheme rdf:resource="http://www.cadastralvocabulary.org/CaLAThe"/>
		<skos:altLabel>Freehold</skos:altLabel>
		<skos:altLabel>Private ownership</skos:altLabel>
		<skos:broader rdf:resource="http://www.cadastralvocabulary.org/CaLAThe/RealRight"/>
		<skos:narrower rdf:resource="http://www.cadastralvocabulary.org/CaLAThe/IndividualOwnership"/>
		<skos:narrower rdf:resource="http://www.cadastralvocabulary.org/CaLAThe/PublicOwnership"/>
		<skos:narrower rdf:resource="http://www.cadastralvocabulary.org/CaLAThe/CoOwnership"/>
		<skos:narrower rdf:resource="http://www.cadastralvocabulary.org/CaLAThe/AdversePossession"/>
	</skos:Concept>

	<skos:Concept rdf:about="http://www.cadastralvocabulary.org/CaLAThe/ParcelAcquisition">
		<skos:prefLabel xml:lang="en">Parcel acquisition</skos:prefLabel>
		<skos:prefLabel xml:lang="da">Erhvervelse af del af fast eje</skos:prefLabel>
		<skos:prefLabel xml:lang="tr">Parsel edinimi</skos:prefLabel>
		<skos:prefLabel xml:lang="ms">Pengambilan petak</skos:prefLabel>
		<skos:scopeNote>OGC LandIfra / InfraGML term</skos:scopeNote>
		<skos:definition>A Conveyance of a Cadastral parcel from a Buyer to a Seller (Source: OGC LandInfra, 7.10.4.1).</skos:definition>
		<skos:changeNote>Established with version 3.</skos:changeNote>
		<skos:inScheme rdf:resource="http://www.cadastralvocabulary.org/CaLAThe"/>
		<skos:broader rdf:resource="http://www.cadastralvocabulary.org/CaLAThe/Conveyance"/>
	</skos:Concept>

	<skos:Concept rdf:about="http://www.cadastralvocabulary.org/CaLAThe/ParcelEstablishment">
		<skos:prefLabel xml:lang="en">Parcel establishment</skos:prefLabel>
		<skos:prefLabel xml:lang="da">Matrikulering</skos:prefLabel>
		<skos:prefLabel xml:lang="tr">Parsel oluşturma</skos:prefLabel>
		<skos:prefLabel xml:lang="ms">Penubuhan petak</skos:prefLabel>
		<skos:scopeNote>OGC LandInfra / InfraGML term</skos:scopeNote>
		<skos:definition>A Property formation either through an initial cadastral Survey or change of existing Cadastral parcels (Source: OGC 7.10.4.1).</skos:definition>
		<skos:changeNote>Established with version 3. Edited to refer to Property formation only in version4</skos:changeNote>
		<skos:inScheme rdf:resource="http://www.cadastralvocabulary.org/CaLAThe"/>
		<skos:broader rdf:resource="http://www.cadastralvocabulary.org/CaLAThe/PropertyFormation"/>
	</skos:Concept>

	<skos:Concept rdf:about="http://www.cadastralvocabulary.org/CaLAThe/Partition">
		<skos:prefLabel xml:lang="en">Partition</skos:prefLabel>
		<skos:prefLabel xml:lang="da">Skifte, Fraskillelse</skos:prefLabel>
		<skos:prefLabel xml:lang="tr">Taksim</skos:prefLabel>
		<skos:prefLabel xml:lang="ms">Pecah bahagian</skos:prefLabel>
		<skos:scopeNote>EULIS / ELRA term</skos:scopeNote>
		<skos:definition>Division of a Real property into separate portions representing the Party shares of the owners in the Real property.</skos:definition>
		<skos:changeNote>Established with version 3. Related to broader: Transfer with version 5</skos:changeNote>
		<skos:inScheme rdf:resource="http://www.cadastralvocabulary.org/CaLAThe"/>
		<skos:broader rdf:resource="http://www.cadastralvocabulary.org/CaLAThe/Transfer"/>
	</skos:Concept>

	<skos:Concept rdf:about="http://www.cadastralvocabulary.org/CaLAThe/Party">
		<skos:prefLabel xml:lang="en">Party</skos:prefLabel>
		<skos:prefLabel xml:lang="da">Aktør</skos:prefLabel>
		<skos:prefLabel xml:lang="tr">Aktör</skos:prefLabel>
		<skos:prefLabel xml:lang="ms">Pihak</skos:prefLabel>
		<skos:scopeNote>ISO LADM and OGC LandInfra / InfraGML term</skos:scopeNote>
		<skos:definition>A Natural person or a Group of natural persons or an Organisation that play Professional (role), Official role, Societal role or Legal personality in a lawful processes.</skos:definition>
		<skos:changeNote>Established with version 1. Definition is changed with version 6.</skos:changeNote>
		<skos:exactMatch rdf:resource="https://isotc211.geolexica.org/concepts/1242/"/>
		<skos:inScheme rdf:resource="http://www.cadastralvocabulary.org/CaLAThe"/>
		<skos:altLabel>LA_Party</skos:altLabel>
		<skos:narrower rdf:resource="http://www.cadastralvocabulary.org/CaLAThe/PartyRoleType"/>
		<skos:narrower rdf:resource="http://www.cadastralvocabulary.org/CaLAThe/PartyType"/>
	</skos:Concept>

	<skos:Concept rdf:about="http://www.cadastralvocabulary.org/CaLAThe/PartyMember">
		<skos:prefLabel xml:lang="en">Party member</skos:prefLabel>
		<skos:prefLabel xml:lang="da">Gruppemedlem</skos:prefLabel>
		<skos:prefLabel xml:lang="tr">Grup üyesi</skos:prefLabel>
		<skos:prefLabel xml:lang="ms">Ahli pihak</skos:prefLabel>
		<skos:scopeNote>ISO LADM term</skos:scopeNote>
		<skos:definition>One of the Parties composing a Group party.</skos:definition>
		<skos:changeNote>Established with version 1. Definition is added with version 6.</skos:changeNote>
		<skos:exactMatch rdf:resource="https://isotc211.geolexica.org/concepts/1310/"/>
		<skos:inScheme rdf:resource="http://www.cadastralvocabulary.org/CaLAThe"/>
		<skos:altLabel>LA_PartyMember</skos:altLabel>
		<skos:broader rdf:resource="http://www.cadastralvocabulary.org/CaLAThe/RightsHolder"/>
		<skos:related rdf:resource="http://www.cadastralvocabulary.org/CaLAThe/PlaceBoundParty"/>
	</skos:Concept>

	<skos:Concept rdf:about="http://www.cadastralvocabulary.org/CaLAThe/PartyRoleType">
		<skos:prefLabel xml:lang="en">Party role type</skos:prefLabel>
		<skos:prefLabel xml:lang="da">Aktørrolle</skos:prefLabel>
		<skos:prefLabel xml:lang="tr">Aktör rolü</skos:prefLabel>
		<skos:prefLabel xml:lang="ms">Jenis peranan pihak</skos:prefLabel>
		<skos:scopeNote>ISO LADM term</skos:scopeNote>
		<skos:changeNote>Established with version 1.</skos:changeNote>
		<skos:inScheme rdf:resource="http://www.cadastralvocabulary.org/CaLAThe"/>
		<skos:broader rdf:resource="http://www.cadastralvocabulary.org/CaLAThe/Party"/>
		<skos:broader rdf:resource="http://www.cadastralvocabulary.org/CaLAThe/Law"/>
		<skos:narrower rdf:resource="http://www.cadastralvocabulary.org/CaLAThe/RightsHolder"/>
		<skos:narrower rdf:resource="http://www.cadastralvocabulary.org/CaLAThe/NaturalPersonRole"/>
	</skos:Concept>

	<skos:Concept rdf:about="http://www.cadastralvocabulary.org/CaLAThe/PartyShare">
		<skos:prefLabel xml:lang="en">Party share</skos:prefLabel>
		<skos:prefLabel xml:lang="da">Andel</skos:prefLabel>
		<skos:prefLabel xml:lang="tr">Pay</skos:prefLabel>
		<skos:prefLabel xml:lang="ms">Syer pihak</skos:prefLabel>
		<skos:changeNote>Established with version 1 and specified as narrower of Co-ownership share in version 3.</skos:changeNote>
		<skos:inScheme rdf:resource="http://www.cadastralvocabulary.org/CaLAThe"/>
		<skos:broader rdf:resource="http://www.cadastralvocabulary.org/CaLAThe/CoOwnershipShare"/>
		<skos:related rdf:resource="http://www.cadastralvocabulary.org/CaLAThe/PartyMember"/>
	</skos:Concept>

	<skos:Concept rdf:about="http://www.cadastralvocabulary.org/CaLAThe/PartyType">
		<skos:prefLabel xml:lang="en">Party type</skos:prefLabel>
		<skos:prefLabel xml:lang="da">Aktørtype</skos:prefLabel>
		<skos:prefLabel xml:lang="tr">Aktör tipi</skos:prefLabel>
		<skos:prefLabel xml:lang="ms">Jenis pihak</skos:prefLabel>
		<skos:scopeNote>ISO LADM term</skos:scopeNote>
		<skos:changeNote>Established with version 1.0</skos:changeNote>
		<skos:inScheme rdf:resource="http://www.cadastralvocabulary.org/CaLAThe"/>
		<skos:broader rdf:resource="http://www.cadastralvocabulary.org/CaLAThe/Party"/>
		<skos:narrower rdf:resource="http://www.cadastralvocabulary.org/CaLAThe/NaturalPerson"/>
		<skos:narrower rdf:resource="http://www.cadastralvocabulary.org/CaLAThe/GroupParty"/>
		<skos:narrower rdf:resource="http://www.cadastralvocabulary.org/CaLAThe/Organisation"/>
	</skos:Concept>

	<skos:Concept rdf:about="http://www.cadastralvocabulary.org/CaLAThe/PlaceBoundParty">
		<skos:prefLabel xml:lang="en">Place bound party</skos:prefLabel>
		<skos:prefLabel xml:lang="da">Stedbestemt gruppe</skos:prefLabel>
		<skos:prefLabel xml:lang="ms">Pihak yang dibenarkan</skos:prefLabel>
		<skos:changeNote>Established with version 1.0</skos:changeNote>
		<skos:inScheme rdf:resource="http://www.cadastralvocabulary.org/CaLAThe"/>
		<skos:broader rdf:resource="http://www.cadastralvocabulary.org/CaLAThe/GroupParty"/>
		<skos:related rdf:resource="http://www.cadastralvocabulary.org/CaLAThe/PartyMember"/>
	</skos:Concept>

	<skos:Concept rdf:about="http://www.cadastralvocabulary.org/CaLAThe/PlaceName">
		<skos:prefLabel xml:lang="en">Place name</skos:prefLabel>
		<skos:prefLabel xml:lang="da">Stednavn</skos:prefLabel>
		<skos:prefLabel xml:lang="tr">Yer adı</skos:prefLabel>
		<skos:prefLabel xml:lang="ms">Nama tempat</skos:prefLabel>
		<skos:definition>One or several proper nouns used to identify a real world entity.</skos:definition>
		<skos:changeNote>Established with version 2. Definition added with version 4. Related Match added with version 6.</skos:changeNote>
		<skos:inScheme rdf:resource="http://www.cadastralvocabulary.org/CaLAThe"/>
		<skos:altLabel>Geographical name</skos:altLabel>
		<skos:broader rdf:resource="http://www.cadastralvocabulary.org/CaLAThe/Gazetteer"/>
		<skos:broader rdf:resource="http://www.cadastralvocabulary.org/CaLAThe/LandDivision"/>
		<skos:broader rdf:resource="http://www.cadastralvocabulary.org/CaLAThe/GeolocatedInformation"/>
		<skos:narrower rdf:resource="http://www.cadastralvocabulary.org/CaLAThe/PostalAddress"/>
	</skos:Concept>

	<skos:Concept rdf:about="http://www.cadastralvocabulary.org/CaLAThe/PlanningLaw">
		<skos:prefLabel xml:lang="en">Planning law</skos:prefLabel>
		<skos:prefLabel xml:lang="da">Arealplanlægning</skos:prefLabel>
		<skos:prefLabel xml:lang="tr">Planlama hukuku</skos:prefLabel>
		<skos:prefLabel xml:lang="ms">Undang-undang perancangan</skos:prefLabel>
		<skos:scopeNote>GEMET term</skos:scopeNote>
		<skos:definition>A binding rule or body of rules prescribed by a government to organize, designate and regulate land use within its domain through zoning laws, subdivision regulations, rent and sign controls, growth management and other measures designed to protect human health and ecological integrity (Source: GEMET)</skos:definition>
		<skos:changeNote>Established with version 1.0. Broader relation changed from Property law to Land law with version 3. </skos:changeNote>
		<skos:inScheme rdf:resource="http://www.cadastralvocabulary.org/CaLAThe"/>
		<skos:broader rdf:resource="http://www.cadastralvocabulary.org/CaLAThe/LandLaw"/>
		<skos:narrower rdf:resource="http://www.cadastralvocabulary.org/CaLAThe/PublicLawRestriction"/>
	</skos:Concept>

	<skos:Concept rdf:about="http://www.cadastralvocabulary.org/CaLAThe/Point">
		<skos:prefLabel xml:lang="en">Point</skos:prefLabel>
		<skos:prefLabel xml:lang="da">Punkt</skos:prefLabel>
		<skos:prefLabel xml:lang="tr">Nokta</skos:prefLabel>
		<skos:prefLabel xml:lang="ms">Titik</skos:prefLabel>
		<skos:scopeNote>Geolexica term</skos:scopeNote>
		<skos:definition>(Ground control point) Point on the earth that has an accurately known geographic position (Source: ISO 19115-2:2019, (E), 3.17; ISO 19115-2:2009(E))</skos:definition>
		<skos:changeNote>Established with version 4</skos:changeNote>
		<skos:exactMatch rdf:resource="https://isotc211.geolexica.org/concepts/336/"/>
		<skos:inScheme rdf:resource="http://www.cadastralvocabulary.org/CaLAThe"/>
		<skos:broader rdf:resource="http://www.cadastralvocabulary.org/CaLAThe/GeometricPrimitive"/>
		<skos:broader rdf:resource="http://www.cadastralvocabulary.org/CaLAThe/LineString"/>
	</skos:Concept>

	<skos:Concept rdf:about="http://www.cadastralvocabulary.org/CaLAThe/PointCloud">
		<skos:prefLabel xml:lang="en">Point cloud</skos:prefLabel>
		<skos:prefLabel xml:lang="da">Punktsky</skos:prefLabel>
		<skos:prefLabel xml:lang="tr">Nokta bulutu</skos:prefLabel>
		<skos:prefLabel xml:lang="ms">Awan titik</skos:prefLabel>
		<skos:scopeNote>OGC LandInfra / InfraGML term</skos:scopeNote>
		<skos:definition>Collection of data points in 3D space. Note to entry: The distance between points is generally non-uniform and hence all three coordinates (Cartesian or spherical) for each point must be specifically encoded.(Source: ISO/TS 19130-2:2014, 4.51).</skos:definition>
		<skos:changeNote>Established with version 4</skos:changeNote>
		<skos:exactMatch rdf:resource="https://isotc211.geolexica.org/concepts/1408/"/>
		<skos:inScheme rdf:resource="http://www.cadastralvocabulary.org/CaLAThe"/>
		<skos:broader rdf:resource="http://www.cadastralvocabulary.org/CaLAThe/TerrestrialLaserScanner"/>
		<skos:broader rdf:resource="http://www.cadastralvocabulary.org/CaLAThe/SurveyResult"/>
	</skos:Concept>

	<skos:Concept rdf:about="http://www.cadastralvocabulary.org/CaLAThe/Polygon">
		<skos:prefLabel xml:lang="en">Polygon</skos:prefLabel>
		<skos:prefLabel xml:lang="da">Polygon</skos:prefLabel>
		<skos:prefLabel xml:lang="tr">Poligon, Çoklu doğru</skos:prefLabel>
		<skos:prefLabel xml:lang="ms">Poligon</skos:prefLabel>
		<skos:scopeNote>Geolexica term</skos:scopeNote>
		<skos:definition>Planar surface defined by 1 exterior boundary and 0 or more interior boundaries (Geolexica, ISO 19136-1:2020)</skos:definition>
		<skos:changeNote>Established with version 4</skos:changeNote>
		<skos:exactMatch rdf:resource="https://isotc211.geolexica.org/concepts/695/"/>
		<skos:inScheme rdf:resource="http://www.cadastralvocabulary.org/CaLAThe"/>
		<skos:broader rdf:resource="http://www.cadastralvocabulary.org/CaLAThe/Surface"/>
		<skos:narrower rdf:resource="http://www.cadastralvocabulary.org/CaLAThe/Curve"/>
	</skos:Concept>

	<skos:Concept rdf:about="http://www.cadastralvocabulary.org/CaLAThe/PositiveLaw">
		<skos:prefLabel xml:lang="en">Positive law</skos:prefLabel>
		<skos:prefLabel xml:lang="da">Positiv ret</skos:prefLabel>
		<skos:prefLabel xml:lang="tr">Pozitif hukuk</skos:prefLabel>
		<skos:prefLabel xml:lang="ms">Perundangan utama</skos:prefLabel>
		<skos:definition>Conventional legal order prevailing in a State and expressing itself through statutes and jurisprudence (Source: Legal Dictionary of Property in Canada - Dualjuridik).</skos:definition>
		<skos:changeNote>Established with version 3.</skos:changeNote>
		<skos:inScheme rdf:resource="http://www.cadastralvocabulary.org/CaLAThe"/>
		<skos:altLabel>Legal basis</skos:altLabel>
		<skos:altLabel>Formal right</skos:altLabel>
		<skos:broader rdf:resource="http://www.cadastralvocabulary.org/CaLAThe/Law"/>
		<skos:narrower rdf:resource="http://www.cadastralvocabulary.org/CaLAThe/LandLaw"/>
	</skos:Concept>

	<skos:Concept rdf:about="http://www.cadastralvocabulary.org/CaLAThe/PostalAddress">
		<skos:prefLabel xml:lang="en">Postal address</skos:prefLabel>
		<skos:prefLabel xml:lang="da">Postadresse</skos:prefLabel>
		<skos:prefLabel xml:lang="tr">Posta adresi</skos:prefLabel>
		<skos:prefLabel xml:lang="ms">Alamat pos</skos:prefLabel>
		<skos:scopeNote>INSPIRE term</skos:scopeNote>
		<skos:definition>Set of information which, for a postal item, allows the unambiguous determination of an actual or potential delivery point, usually combined with the specification of an addressee and/or mailee. (INSPIRE Source: Universal Postal Union 2006). Structured information that allows the unambiguous determination of an [real world] object for purposes of identification and location (Geolexica)</skos:definition>
		<skos:changeNote>Established with version 1. Edited in version 3 as Postal address to comply with INPSIRE specifications. Definitions edited with version 4</skos:changeNote>
		<skos:exactMatch rdf:resource="http://inspire.ec.europa.eu/glossary/PostalAddress"/>
		<skos:exactMatch rdf:resource="http://publications.europa.eu/resource/authority/address-type/ADR_POSTAL"/>
		<skos:exactMatch rdf:resource="https://isotc211.geolexica.org/concepts/2117/"/>
		<skos:inScheme rdf:resource="http://www.cadastralvocabulary.org/CaLAThe"/>
		<skos:altLabel>Address</skos:altLabel>
		<skos:broader rdf:resource="http://www.cadastralvocabulary.org/CaLAThe/PlaceName"/>
		<skos:broader rdf:resource="http://www.cadastralvocabulary.org/CaLAThe/RoadNetwork"/>
		<skos:narrower rdf:resource="http://www.cadastralvocabulary.org/CaLAThe/StreetSign"/>
	</skos:Concept>

	<skos:Concept rdf:about="http://www.cadastralvocabulary.org/CaLAThe/PreemptionRight">
		<skos:prefLabel xml:lang="en">Pre-emption right</skos:prefLabel>
		<skos:prefLabel xml:lang="da">Forkøbsret</skos:prefLabel>
		<skos:prefLabel xml:lang="tr">Ön alım hakkı</skos:prefLabel>
		<skos:prefLabel xml:lang="ms">Hak keutamaan</skos:prefLabel>
		<skos:definition>The owner of land has contracted that if he decides to sell the land he first will offer it to the other contracting party.</skos:definition>
		<skos:exactMatch rdf:resource="http://aims.fao.org/aos/agrovoc/c_9c081fdc"/>
		<skos:exactMatch rdf:resource="https://www.eionet.europa.eu/gemet/en/concept/11623"/>
		<skos:exactMatch rdf:resource="http://eurovoc.europa.eu/546"/>
		<skos:inScheme rdf:resource="http://www.cadastralvocabulary.org/CaLAThe"/>
		<skos:broader rdf:resource="http://www.cadastralvocabulary.org/CaLAThe/LawOfObligation"/>
	</skos:Concept>

	<skos:Concept rdf:about="http://www.cadastralvocabulary.org/CaLAThe/PrivateLawRestriction">
		<skos:prefLabel xml:lang="en">Private law restriction</skos:prefLabel>
		<skos:prefLabel xml:lang="da">Privatretlig regulering</skos:prefLabel>
		<skos:prefLabel xml:lang="tr">Özel hukuk kısıtlaması</skos:prefLabel>
		<skos:prefLabel xml:lang="ms">Sekatan undang-undang sivil</skos:prefLabel>
		<skos:changeNote>Established with version 1.</skos:changeNote>
		<skos:inScheme rdf:resource="http://www.cadastralvocabulary.org/CaLAThe"/>
		<skos:broader rdf:resource="http://www.cadastralvocabulary.org/CaLAThe/Easement"/>
		<skos:narrower rdf:resource="http://www.cadastralvocabulary.org/CaLAThe/RightOfWay"/>
	</skos:Concept>

	<skos:Concept rdf:about="http://www.cadastralvocabulary.org/CaLAThe/Professional">
		<skos:prefLabel xml:lang="en">Professional</skos:prefLabel>
		<skos:prefLabel xml:lang="da">Professionel</skos:prefLabel>
		<skos:prefLabel xml:lang="tr">Profesyonel</skos:prefLabel>
		<skos:prefLabel xml:lang="ms">Profesional</skos:prefLabel>
		<skos:scopeNote>OGC LandInfra / InfraGML term</skos:scopeNote>
		<skos:definition>A Natural person generally with tertiary education, who through a license is bound to act according to the standards of a professional association.</skos:definition>
		<skos:changeNote>Established with version 3. Definition is added with version 6.</skos:changeNote>
		<skos:inScheme rdf:resource="http://www.cadastralvocabulary.org/CaLAThe"/>
		<skos:altLabel>Professional role</skos:altLabel>
		<skos:broader rdf:resource="http://www.cadastralvocabulary.org/CaLAThe/NaturalPersonRole"/>
		<skos:narrower rdf:resource="http://www.cadastralvocabulary.org/CaLAThe/Notary"/>
		<skos:narrower rdf:resource="http://www.cadastralvocabulary.org/CaLAThe/Surveyor"/>
		<skos:narrower rdf:resource="http://www.cadastralvocabulary.org/CaLAThe/Draftsman"/>
		<skos:narrower rdf:resource="http://www.cadastralvocabulary.org/CaLAThe/Lawyer"/>
		<skos:narrower rdf:resource="http://www.cadastralvocabulary.org/CaLAThe/Engineer"/>
	</skos:Concept>

	<skos:Concept rdf:about="http://www.cadastralvocabulary.org/CaLAThe/ProfessionalSociety">
		<skos:prefLabel xml:lang="en">Professional society</skos:prefLabel>
		<skos:prefLabel xml:lang="da">Professionsforening</skos:prefLabel>
		<skos:prefLabel xml:lang="tr">Profesyonel cemiyet</skos:prefLabel>
		<skos:prefLabel xml:lang="ms">Persatuan profesional</skos:prefLabel>
		<skos:scopeNote>GEMET term</skos:scopeNote>
		<skos:definition>A group of persons engaged in the same profession, business, trade or craft that is organized or formally structured to attain common ends (Source: Random House, 1997).</skos:definition>
		<skos:changeNote>Established with version 3.</skos:changeNote>
		<skos:exactMatch rdf:resource="http://www.eionet.europa.eu/gemet/concept/14847"/>
		<skos:exactMatch rdf:resource="http://aims.fao.org/aos/agrovoc/c_50290"/>
		<skos:inScheme rdf:resource="http://www.cadastralvocabulary.org/CaLAThe"/>
		<skos:altLabel>Professional association</skos:altLabel>
		<skos:broader rdf:resource="http://www.cadastralvocabulary.org/CaLAThe/Association"/>
	</skos:Concept>

	<skos:Concept rdf:about="http://www.cadastralvocabulary.org/CaLAThe/PropertyEnquiryCertificate">
		<skos:prefLabel xml:lang="en">Property enquiry certificate</skos:prefLabel>
		<skos:prefLabel xml:lang="da"></skos:prefLabel>
		<skos:prefLabel xml:lang="tr"></skos:prefLabel>
		<skos:prefLabel xml:lang="ms">Sijil siasatan harta</skos:prefLabel>
		<skos:scopeNote>esd-toolkit.eu term</skos:scopeNote>
		<skos:definition>When a property is being sold in the UK, a solicitor will carry out conveyancing duties which normally include a property search. The local authority can carry out these searches and provide a Property Enquiry Certificate, detailing issues relating to Planning, Building Control, Environmental Health, Housing, Roads, etc (Source: esd-toolkit.eu).</skos:definition>
		<skos:changeNote>Established with version 1.  Â´in the UKÂ´ added to definition with version 6.</skos:changeNote>
		<skos:exactMatch rdf:resource="http://id.esd-toolkit.eu/service/1060"/>
		<skos:inScheme rdf:resource="http://www.cadastralvocabulary.org/CaLAThe"/>
		<skos:broader rdf:resource="http://www.cadastralvocabulary.org/CaLAThe/Certificate"/>
	</skos:Concept>

	<skos:Concept rdf:about="http://www.cadastralvocabulary.org/CaLAThe/PropertyFormation">
		<skos:prefLabel xml:lang="en">Property formation</skos:prefLabel>
		<skos:prefLabel xml:lang="da">Ejendomsdannelse</skos:prefLabel>
		<skos:prefLabel xml:lang="tr">Taşınmaz oluşturma</skos:prefLabel>
		<skos:prefLabel xml:lang="ms">Pembentukan harta</skos:prefLabel>
		<skos:definition>An Activity establishing or changing boundaries of Real property or Real rights, performed by a Professional according to Law.</skos:definition>
		<skos:changeNote>Established with version 2.0. Related to ParcelEstablishment with version 3. ParcelEstablishment made narrower with version 4</skos:changeNote>
		<skos:inScheme rdf:resource="http://www.cadastralvocabulary.org/CaLAThe"/>
		<skos:altLabel>Cadastral activity</skos:altLabel>
		<skos:broader rdf:resource="http://www.cadastralvocabulary.org/CaLAThe/Activity"/>
		<skos:narrower rdf:resource="http://www.cadastralvocabulary.org/CaLAThe/ChangeOfPropertyUnitType"/>
		<skos:narrower rdf:resource="http://www.cadastralvocabulary.org/CaLAThe/TransferOfPartOfProperty"/>
		<skos:narrower rdf:resource="http://www.cadastralvocabulary.org/CaLAThe/Amalgamation"/>
		<skos:narrower rdf:resource="http://www.cadastralvocabulary.org/CaLAThe/Subdivision"/>
		<skos:narrower rdf:resource="http://www.cadastralvocabulary.org/CaLAThe/PropertyRestructuring"/>
		<skos:narrower rdf:resource="http://www.cadastralvocabulary.org/CaLAThe/SuperficieObjectEstablishment"/>
		<skos:narrower rdf:resource="http://www.cadastralvocabulary.org/CaLAThe/ParcelEstablishment"/>
	</skos:Concept>

	<skos:Concept rdf:about="http://www.cadastralvocabulary.org/CaLAThe/PropertyRestructuring">
		<skos:prefLabel xml:lang="en">Property restructuring</skos:prefLabel>
		<skos:prefLabel xml:lang="da">Områdevis ejendomsændring</skos:prefLabel>
		<skos:prefLabel xml:lang="tr">Taşınmaz yapılandırma</skos:prefLabel>
		<skos:prefLabel xml:lang="ms">Penstrukturan semula harta</skos:prefLabel>
		<skos:definition>Property formation addressing a larger number of Real properties within a single case.</skos:definition>
		<skos:changeNote>Established with version 2.0.</skos:changeNote>
		<skos:inScheme rdf:resource="http://www.cadastralvocabulary.org/CaLAThe"/>
		<skos:broader rdf:resource="http://www.cadastralvocabulary.org/CaLAThe/PropertyFormation"/>
		<skos:narrower rdf:resource="http://www.cadastralvocabulary.org/CaLAThe/LandConsolidation"/>
		<skos:narrower rdf:resource="http://www.cadastralvocabulary.org/CaLAThe/LandReadjustment"/>
		<skos:narrower rdf:resource="http://www.cadastralvocabulary.org/CaLAThe/Expropriation"/>
	</skos:Concept>

	<skos:Concept rdf:about="http://www.cadastralvocabulary.org/CaLAThe/PropertyUnitType">
		<skos:prefLabel xml:lang="en">Property unit type</skos:prefLabel>
		<skos:prefLabel xml:lang="da">Ejendomstype</skos:prefLabel>
		<skos:prefLabel xml:lang="tr">Taşınmaz cinsi</skos:prefLabel>
		<skos:prefLabel xml:lang="ms">Jenis unit harta</skos:prefLabel>
		<skos:definition>Code list of admitted property unit types within a jurisdiction (Adopted from LA_BAUnitType).</skos:definition>
		<skos:changeNote>Established with version 1. Definition is added in version 5.</skos:changeNote>
		<skos:inScheme rdf:resource="http://www.cadastralvocabulary.org/CaLAThe"/>
		<skos:broader rdf:resource="http://www.cadastralvocabulary.org/CaLAThe/RealProperty"/>
	</skos:Concept>

	<skos:Concept rdf:about="http://www.cadastralvocabulary.org/CaLAThe/ProtectedSite">
		<skos:prefLabel xml:lang="en">Protected site</skos:prefLabel>
		<skos:prefLabel xml:lang="da">Beskyttet lokalitet</skos:prefLabel>
		<skos:prefLabel xml:lang="tr">Korunan alan</skos:prefLabel>
		<skos:prefLabel xml:lang="ms">Tapak yang dilindungi</skos:prefLabel>
		<skos:scopeNote>INSPIRE term</skos:scopeNote>
		<skos:definition>An area designated or managed according to jurisdiction legislation to achieve specific conservation objectives (Adopted from INSPIRE, http://inspire.ec.europa.eu/featureconcept/ProtectedSite).	</skos:definition>
		<skos:changeNote>Established with version 2. Definition is added in version 5.</skos:changeNote>
		<skos:exactMatch rdf:resource="http://inspire.ec.europa.eu/glossary/ProtectedSite"/>
		<skos:exactMatch rdf:resource="http://aims.fao.org/aos/agrovoc/c_37952"/>
		<skos:exactMatch rdf:resource="https://www.eionet.europa.eu/gemet/en/concept/6740"/>
		<skos:exactMatch rdf:resource="http://zbw.eu/stw/descriptor/19628-1"/>
		<skos:exactMatch rdf:resource="http://eurovoc.europa.eu/4801"/>
		<skos:inScheme rdf:resource="http://www.cadastralvocabulary.org/CaLAThe"/>
		<skos:broader rdf:resource="http://www.cadastralvocabulary.org/CaLAThe/AdministrativeUnit"/>
	</skos:Concept>

	<skos:Concept rdf:about="http://www.cadastralvocabulary.org/CaLAThe/PublicLawRestriction">
		<skos:prefLabel xml:lang="en">Public law restriction</skos:prefLabel>
		<skos:prefLabel xml:lang="da">Offentligretlig regulering</skos:prefLabel>
		<skos:prefLabel xml:lang="tr">Kamu hukuku kısıtlaması</skos:prefLabel>
		<skos:prefLabel xml:lang="ms">Sekatan undang-undang awam</skos:prefLabel>
		<skos:changeNote>Established with version 1.</skos:changeNote>
		<skos:inScheme rdf:resource="http://www.cadastralvocabulary.org/CaLAThe"/>
		<skos:broader rdf:resource="http://www.cadastralvocabulary.org/CaLAThe/Easement"/>
		<skos:broader rdf:resource="http://www.cadastralvocabulary.org/CaLAThe/PlanningLaw"/>
		<skos:narrower rdf:resource="http://www.cadastralvocabulary.org/CaLAThe/RightOfWay"/>
	</skos:Concept>

	<skos:Concept rdf:about="http://www.cadastralvocabulary.org/CaLAThe/PublicOwnership">
		<skos:prefLabel xml:lang="en">Public ownership</skos:prefLabel>
		<skos:prefLabel xml:lang="da">Offentlig ejendom</skos:prefLabel>
		<skos:prefLabel xml:lang="tr">Kamu taşınmazı</skos:prefLabel>
		<skos:prefLabel xml:lang="ms">Pemilikan awam</skos:prefLabel>
		<skos:scopeNote>AGROVOC Multilingual Thesaurus term</skos:scopeNote>
		<skos:changeNote>Established with version 1.</skos:changeNote>
		<skos:exactMatch rdf:resource="http://aims.fao.org/aos/agrovoc/c_6350"/>
		<skos:exactMatch rdf:resource="http://eurovoc.europa.eu/2812"/>
		<skos:inScheme rdf:resource="http://www.cadastralvocabulary.org/CaLAThe"/>
		<skos:broader rdf:resource="http://www.cadastralvocabulary.org/CaLAThe/Ownership"/>
	</skos:Concept>

	<skos:Concept rdf:about="http://www.cadastralvocabulary.org/CaLAThe/RealProperty">
		<skos:prefLabel xml:lang="en">Real property</skos:prefLabel>
		<skos:prefLabel xml:lang="da">Bestemt fast ejendom</skos:prefLabel>
		<skos:prefLabel xml:lang="tr">Taşınmaz, Gayrimenkul</skos:prefLabel>
		<skos:prefLabel xml:lang="ms">Harta tanah</skos:prefLabel>
		<skos:definition>1. One or more Cadastral parcels, which are owned by the same party, and recorded as a unit according jurisdiction provisions, or 2. Condominium, or 3. Superficie object</skos:definition>
		<skos:changeNote>Established with version 1.0. Changed narrower from Building use part to Condominium with version 3. Definition is added in version 5, and the concept is renamed Real property, while the previous term Property unit is maintained as altLabel.</skos:changeNote>
		<skos:inScheme rdf:resource="http://www.cadastralvocabulary.org/CaLAThe"/>
		<skos:altLabel>Basic property unit</skos:altLabel>
		<skos:altLabel>Immovable property</skos:altLabel>
		<skos:altLabel>Property unit</skos:altLabel>
		<skos:broader rdf:resource="http://www.cadastralvocabulary.org/CaLAThe/LandDivision"/>
		<skos:narrower rdf:resource="http://www.cadastralvocabulary.org/CaLAThe/CadastralParcel"/>
		<skos:narrower rdf:resource="http://www.cadastralvocabulary.org/CaLAThe/PropertyUnitType"/>
		<skos:narrower rdf:resource="http://www.cadastralvocabulary.org/CaLAThe/Condominium"/>
		<skos:narrower rdf:resource="http://www.cadastralvocabulary.org/CaLAThe/SuperficieObject"/>
		<skos:narrower rdf:resource="http://www.cadastralvocabulary.org/CaLAThe/LA_BAUnit"/>
		<skos:narrower rdf:resource="http://www.cadastralvocabulary.org/CaLAThe/LA_RequiredRelationship"/>
	</skos:Concept>

	<skos:Concept rdf:about="http://www.cadastralvocabulary.org/CaLAThe/RealRight">
		<skos:prefLabel xml:lang="en">Real right</skos:prefLabel>
		<skos:prefLabel xml:lang="da">Ejendomsret</skos:prefLabel>
		<skos:prefLabel xml:lang="tr">Ayni hak</skos:prefLabel>
		<skos:prefLabel xml:lang="ms">Hak mutlak</skos:prefLabel>
		<skos:altLabel>Interest in land</skos:altLabel>
		<skos:altLabel>Estate</skos:altLabel>
		<skos:scopeNote>EULIS / ELRA term</skos:scopeNote>
		<skos:definition>Prerogative that can be opposed to all, conferring a direct or indirect access to property. (Source: Dualjuridik) A right relating to land that is binding on third parties even if they are unaware of it. (ius in rem) (Source: EULIS / ELRA glossary)</skos:definition>
		<skos:changeNote>Established with version 1. Term changed and definitions added with version 3.</skos:changeNote>
		<skos:inScheme rdf:resource="http://www.cadastralvocabulary.org/CaLAThe"/>
		<skos:broader rdf:resource="http://www.cadastralvocabulary.org/CaLAThe/LandLaw"/>
		<skos:narrower rdf:resource="http://www.cadastralvocabulary.org/CaLAThe/Ownership"/>
		<skos:narrower rdf:resource="http://www.cadastralvocabulary.org/CaLAThe/Leasehold"/>
		<skos:narrower rdf:resource="http://www.cadastralvocabulary.org/CaLAThe/LimitedRight"/>
		<skos:narrower rdf:resource="http://www.cadastralvocabulary.org/CaLAThe/LA_Right"/>
	</skos:Concept>

	<skos:Concept rdf:about="http://www.cadastralvocabulary.org/CaLAThe/Reallotment">
		<skos:prefLabel xml:lang="en">Reallotment</skos:prefLabel>
		<skos:prefLabel xml:lang="da">Arealoverførsel</skos:prefLabel>
		<skos:prefLabel xml:lang="tr">Dağıtım, Tahsis</skos:prefLabel>
		<skos:prefLabel xml:lang="ms">Pembahagian semula</skos:prefLabel>
		<skos:definition>Reallocation of Real rights into new Real properties through Property formation procedures.</skos:definition>
		<skos:inScheme rdf:resource="http://www.cadastralvocabulary.org/CaLAThe"/>
		<skos:broader rdf:resource="http://www.cadastralvocabulary.org/CaLAThe/LandConsolidation"/>
		<skos:broader rdf:resource="http://www.cadastralvocabulary.org/CaLAThe/LandReadjustment"/>
		<skos:broader rdf:resource="http://www.cadastralvocabulary.org/CaLAThe/TransferOfPartOfProperty"/>
	</skos:Concept>

	<skos:Concept rdf:about="http://www.cadastralvocabulary.org/CaLAThe/Registrar">
		<skos:prefLabel xml:lang="en">Registrar</skos:prefLabel>
		<skos:prefLabel xml:lang="da">Registrator</skos:prefLabel>
		<skos:prefLabel xml:lang="tr">Tapu sicil muhafızı</skos:prefLabel>
		<skos:prefLabel xml:lang="ms">Pendaftar</skos:prefLabel>
		<skos:definition>An Official role for keeping a Registry or official records.</skos:definition>
		<skos:changeNote>Established with version 1. Definition is added with version 6.</skos:changeNote>
		<skos:exactMatch rdf:resource="http://publications.europa.eu/resource/authority/role/REGISTRAR"/>
		<skos:inScheme rdf:resource="http://www.cadastralvocabulary.org/CaLAThe"/>
		<skos:broader rdf:resource="http://www.cadastralvocabulary.org/CaLAThe/OfficialRole"/>
	</skos:Concept>

	<skos:Concept rdf:about="http://www.cadastralvocabulary.org/CaLAThe/Registry">
		<skos:prefLabel xml:lang="en">Registry</skos:prefLabel>
		<skos:prefLabel xml:lang="da">Registerforvaltning</skos:prefLabel>
		<skos:prefLabel xml:lang="tr">Sicil</skos:prefLabel>
		<skos:prefLabel xml:lang="ms">Daftar</skos:prefLabel>
		<skos:scopeNote>Public administration</skos:scopeNote>
		<skos:definition>1. Official records of people or things relating to a business or other activity 2. Organization or place that keeps official records (Source: Adopted from Cambridge Dictionary, Business English)</skos:definition>
		<skos:changeNote>Added in version 5. Changed broader and other relations in version 6.</skos:changeNote>
		<skos:closeMatch rdf:resource="https://agrovoc.fao.org/browse/agrovoc/en/page/c_6491"/>
		<skos:inScheme rdf:resource="http://www.cadastralvocabulary.org/CaLAThe"/>
		<skos:broader rdf:resource="http://www.cadastralvocabulary.org/CaLAThe/GovernmentalOrganisation"/>
		<skos:narrower rdf:resource="http://www.cadastralvocabulary.org/CaLAThe/LandRegistry"/>
		<skos:narrower rdf:resource="http://www.cadastralvocabulary.org/CaLAThe/Cadastre"/>
	</skos:Concept>

	<skos:Concept rdf:about="http://www.cadastralvocabulary.org/CaLAThe/Rent">
		<skos:prefLabel xml:lang="en">Rent</skos:prefLabel>
		<skos:prefLabel xml:lang="da">Leje </skos:prefLabel>
		<skos:prefLabel xml:lang="tr">Kira </skos:prefLabel>
		<skos:prefLabel xml:lang="ms">Sewa</skos:prefLabel>
		<skos:definition>A periodic sum paid under a Lease agreement in return for the use of Real property. </skos:definition>
		<skos:changeNote>Established with version 2.</skos:changeNote>
		<skos:exactMatch rdf:resource="http://aims.fao.org/aos/agrovoc/c_6503"/>
		<skos:inScheme rdf:resource="http://www.cadastralvocabulary.org/CaLAThe"/>
		<skos:broader rdf:resource="http://www.cadastralvocabulary.org/CaLAThe/Exchange"/>
	</skos:Concept>

	<skos:Concept rdf:about="http://www.cadastralvocabulary.org/CaLAThe/Representation">
		<skos:prefLabel xml:lang="en">Representation</skos:prefLabel>
		<skos:prefLabel xml:lang="da">Repræsentation</skos:prefLabel>
		<skos:prefLabel xml:lang="tr">Temsiliyet</skos:prefLabel>
		<skos:prefLabel xml:lang="ms">Perwakilan</skos:prefLabel>
		<skos:scopeNote>GEMET term</skos:scopeNote>
		<skos:definition>Any conduct or action undertaken on behalf of a person, group, business or government, often as an elected or appointed voice (Source: Random House, 1997).</skos:definition>
		<skos:changeNote>Established with version 1.</skos:changeNote>
		<skos:exactMatch rdf:resource="http://www.eionet.europa.eu/gemet/concept/7118"/>
		<skos:inScheme rdf:resource="http://www.cadastralvocabulary.org/CaLAThe"/>
		<skos:broader rdf:resource="http://www.cadastralvocabulary.org/CaLAThe/RightsHolder"/>
	</skos:Concept>

	<skos:Concept rdf:about="http://www.cadastralvocabulary.org/CaLAThe/RestrictionDeed">
		<skos:prefLabel xml:lang="en">Restriction deed</skos:prefLabel>
		<skos:prefLabel xml:lang="da">Servitutdokument</skos:prefLabel>
		<skos:prefLabel xml:lang="tr">İrtifak sözleşmesi</skos:prefLabel>
		<skos:prefLabel xml:lang="ms">Peraturan surat ikatan</skos:prefLabel>
		<skos:changeNote>Established with version 1.</skos:changeNote>
		<skos:inScheme rdf:resource="http://www.cadastralvocabulary.org/CaLAThe"/>
		<skos:broader rdf:resource="http://www.cadastralvocabulary.org/CaLAThe/Deed"/>
	</skos:Concept>

	<skos:Concept rdf:about="http://www.cadastralvocabulary.org/CaLAThe/RightOfSuperficie">
		<skos:prefLabel xml:lang="en">Right of superficies</skos:prefLabel>
		<skos:prefLabel xml:lang="da">Superficiærfæste</skos:prefLabel>
		<skos:prefLabel xml:lang="tr">Üst hakkı</skos:prefLabel>
		<skos:prefLabel xml:lang="ms">Hak ke atas superfisi</skos:prefLabel>
		<skos:scopeNote>OGC LandInfra / InfraGML term</skos:scopeNote>
		<skos:definition>Real property right which enables its proprietor - the âsuperficiaryâ - to have or acquire for himself buildings, constructions or plants (vegetation) in, on or above an immovable thing owned by someone else (Dutch Civil Code Article 5:101; http://www.dutchcivillaw.com/legislation/dcctitle5588.htm)</skos:definition>
		<skos:changeNote>Established with version 3. Definition is added in version 5.</skos:changeNote>
		<skos:inScheme rdf:resource="http://www.cadastralvocabulary.org/CaLAThe"/>
		<skos:altLabel>Building lease</skos:altLabel>
		<skos:broader rdf:resource="http://www.cadastralvocabulary.org/CaLAThe/CoOwnership"/>
		<skos:related rdf:resource="http://www.cadastralvocabulary.org/CaLAThe/SuperficieObject"/>
	</skos:Concept>

	<skos:Concept rdf:about="http://www.cadastralvocabulary.org/CaLAThe/RightOfWay">
		<skos:prefLabel xml:lang="en">Right of way</skos:prefLabel>
		<skos:prefLabel xml:lang="da">Vejret</skos:prefLabel>
		<skos:prefLabel xml:lang="tr">Geçit hakkı</skos:prefLabel>
		<skos:prefLabel xml:lang="ms">Hak lalu lalang</skos:prefLabel>
		<skos:definition>Right to circulate given to the holder of the ownership of dominant land (Source: Legal Dictionary of Property in Canada - Dualjuridik).</skos:definition>
		<skos:changeNote>Established with version 1. Definition added with ver. 3.</skos:changeNote>
		<skos:inScheme rdf:resource="http://www.cadastralvocabulary.org/CaLAThe"/>
		<skos:broader rdf:resource="http://www.cadastralvocabulary.org/CaLAThe/PrivateLawRestriction"/>
		<skos:broader rdf:resource="http://www.cadastralvocabulary.org/CaLAThe/PublicLawRestriction"/>
	</skos:Concept>

	<skos:Concept rdf:about="http://www.cadastralvocabulary.org/CaLAThe/RightsHolder">
		<skos:prefLabel xml:lang="en">Rights holder</skos:prefLabel>
		<skos:prefLabel xml:lang="da">Rettighedshaver</skos:prefLabel>
		<skos:prefLabel xml:lang="tr">Hak sahibi</skos:prefLabel>
		<skos:prefLabel xml:lang="ms">Pemegang hak</skos:prefLabel>
		<skos:definition>A Party that holds rights related to Real property.</skos:definition>
		<skos:changeNote>Established with version 2. Alternative relation with version 3. Changed from Rightholder to Rights holder in version 5. Definition is added with version 6.</skos:changeNote>
		<skos:inScheme rdf:resource="http://www.cadastralvocabulary.org/CaLAThe"/>
		<skos:altLabel>Holder</skos:altLabel>
		<skos:broader rdf:resource="http://www.cadastralvocabulary.org/CaLAThe/PartyRoleType"/>
		<skos:narrower rdf:resource="http://www.cadastralvocabulary.org/CaLAThe/Owner"/>
		<skos:narrower rdf:resource="http://www.cadastralvocabulary.org/CaLAThe/Mortgagee"/>
		<skos:narrower rdf:resource="http://www.cadastralvocabulary.org/CaLAThe/Representation"/>
		<skos:narrower rdf:resource="http://www.cadastralvocabulary.org/CaLAThe/PartyMember"/>
		<skos:narrower rdf:resource="http://www.cadastralvocabulary.org/CaLAThe/LegalPerson"/>
		<skos:narrower rdf:resource="http://www.cadastralvocabulary.org/CaLAThe/Mortgagor"/>
		<skos:narrower rdf:resource="http://www.cadastralvocabulary.org/CaLAThe/Lessor"/>
		<skos:narrower rdf:resource="http://www.cadastralvocabulary.org/CaLAThe/Lessee"/>
		<skos:narrower rdf:resource="http://www.cadastralvocabulary.org/CaLAThe/GoodFaith"/>
		<skos:related rdf:resource="http://www.cadastralvocabulary.org/CaLAThe/Document"/>
	</skos:Concept>

	<skos:Concept rdf:about="http://www.cadastralvocabulary.org/CaLAThe/RoadNetwork">
		<skos:prefLabel xml:lang="en">Road network</skos:prefLabel>
		<skos:prefLabel xml:lang="da">Vejnet</skos:prefLabel>
		<skos:prefLabel xml:lang="tr">Yol ağı</skos:prefLabel>
		<skos:prefLabel xml:lang="ms">Rangkaian jalan raya</skos:prefLabel>
		<skos:scopeNote>GEMET INSPIRE theme</skos:scopeNote>
		<skos:definition>Transportation infrastructure, modelled as a spatial network (Adopted from Barthelemy, 2010: Spatial Networks)</skos:definition>
		<skos:changeNote>Established with version 4. Definition added with version 6.</skos:changeNote>
		<skos:exactMatch rdf:resource="http://eurovoc.europa.eu/3438"/>
		<skos:inScheme rdf:resource="http://www.cadastralvocabulary.org/CaLAThe"/>
		<skos:broader rdf:resource="http://www.cadastralvocabulary.org/CaLAThe/TopologicalLocalization"/>
		<skos:narrower rdf:resource="http://www.cadastralvocabulary.org/CaLAThe/PostalAddress"/>
	</skos:Concept>

	<skos:Concept rdf:about="http://www.cadastralvocabulary.org/CaLAThe/SatelliteImage">
		<skos:prefLabel xml:lang="en">Satellite image</skos:prefLabel>
		<skos:prefLabel xml:lang="da">Satellitbillede</skos:prefLabel>
		<skos:prefLabel xml:lang="tr">Uydu görüntüsü</skos:prefLabel>
		<skos:prefLabel xml:lang="ms">Imej satelit</skos:prefLabel>
		<skos:scopeNote>GEMET term</skos:scopeNote>
		<skos:definition>A pictorial representation of data projected onto a two-dimensional grid of individual picture elements (pixels) and acquired from a human-made vessel placed in orbit round a planet, moon or star (Source: GEMET).</skos:definition>
		<skos:changeNote>Established with version 1.</skos:changeNote>
		<skos:exactMatch rdf:resource="http://www.eionet.europa.eu/gemet/concept/6253"/>
		<skos:inScheme rdf:resource="http://www.cadastralvocabulary.org/CaLAThe"/>
		<skos:broader rdf:resource="http://www.cadastralvocabulary.org/CaLAThe/DigitalImagery"/>
	</skos:Concept>

	<skos:Concept rdf:about="http://www.cadastralvocabulary.org/CaLAThe/SecurityInterest">
		<skos:prefLabel xml:lang="en">Security interest</skos:prefLabel>
		<skos:prefLabel xml:lang="da">Sikkerhedsret</skos:prefLabel>
		<skos:prefLabel xml:lang="tr">Rehin hakkı</skos:prefLabel>
		<skos:prefLabel xml:lang="ms">Kepentingan keselamatan</skos:prefLabel>
		<skos:changeNote>Established with version 3.</skos:changeNote>
		<skos:inScheme rdf:resource="http://www.cadastralvocabulary.org/CaLAThe"/>
		<skos:broader rdf:resource="http://www.cadastralvocabulary.org/CaLAThe/LimitedRight"/>
		<skos:narrower rdf:resource="http://www.cadastralvocabulary.org/CaLAThe/Mortgage"/>
	</skos:Concept>

	<skos:Concept rdf:about="http://www.cadastralvocabulary.org/CaLAThe/Seller">
		<skos:prefLabel xml:lang="en">Seller</skos:prefLabel>
		<skos:prefLabel xml:lang="da">Sælger</skos:prefLabel>
		<skos:prefLabel xml:lang="tr">Satıcı</skos:prefLabel>
		<skos:prefLabel xml:lang="ms">Penjual</skos:prefLabel>
		<skos:scopeNote>OGC LandInfra / InfraGML term</skos:scopeNote>
		<skos:changeNote>Established with version 4</skos:changeNote>
		<skos:inScheme rdf:resource="http://www.cadastralvocabulary.org/CaLAThe"/>
		<skos:broader rdf:resource="http://www.cadastralvocabulary.org/CaLAThe/Signatory"/>
	</skos:Concept>

	<skos:Concept rdf:about="http://www.cadastralvocabulary.org/CaLAThe/ServientPropertyUnit">
		<skos:prefLabel xml:lang="en">Servient property unit</skos:prefLabel>
		<skos:prefLabel xml:lang="da">Tjenende ejendom</skos:prefLabel>
		<skos:prefLabel xml:lang="tr">Yükümlü taşınmaz</skos:prefLabel>
		<skos:prefLabel xml:lang="ms">Unit harta yang menanggung</skos:prefLabel>
		<skos:definition>Land (Property unit) submitted to a servitude to benefit a dominant land (Source: Legal Dictionary of Property in Canada - Dualjuridik).</skos:definition>
		<skos:changeNote>Established with version 1. Definition and alt. relation added with version 3.</skos:changeNote>
		<skos:inScheme rdf:resource="http://www.cadastralvocabulary.org/CaLAThe"/>
		<skos:altLabel>Servient land</skos:altLabel>
		<skos:broader rdf:resource="http://www.cadastralvocabulary.org/CaLAThe/Easement"/>
	</skos:Concept>

	<skos:Concept rdf:about="http://www.cadastralvocabulary.org/CaLAThe/Signatory">
		<skos:prefLabel xml:lang="en">Signatory</skos:prefLabel>
		<skos:prefLabel xml:lang="da">Underskriver</skos:prefLabel>
		<skos:prefLabel xml:lang="tr">İmza sahibi</skos:prefLabel>
		<skos:prefLabel xml:lang="ms">Penandatangan</skos:prefLabel>
		<skos:scopeNote>OGC LandInfra / InfraGML term</skos:scopeNote>
		<skos:definition>A Natural person who signs a Document.</skos:definition>
		<skos:changeNote>Added with version 3. Context modified in version 5, with introduction of Legal personality. Definition is changed with version 6.</skos:changeNote>
		<skos:exactMatch rdf:resource="http://publications.europa.eu/resource/authority/role/SIGN"/>
		<skos:inScheme rdf:resource="http://www.cadastralvocabulary.org/CaLAThe"/>
		<skos:altLabel>LI_SigningRole</skos:altLabel>
		<skos:broader rdf:resource="http://www.cadastralvocabulary.org/CaLAThe/LegalPersonality"/>
		<skos:narrower rdf:resource="http://www.cadastralvocabulary.org/CaLAThe/Buyer"/>
		<skos:narrower rdf:resource="http://www.cadastralvocabulary.org/CaLAThe/Seller"/>
		<skos:narrower rdf:resource="http://www.cadastralvocabulary.org/CaLAThe/Owner"/>
	</skos:Concept>

	<skos:Concept rdf:about="http://www.cadastralvocabulary.org/CaLAThe/Site">
		<skos:prefLabel xml:lang="en">Site</skos:prefLabel>
		<skos:prefLabel xml:lang="da">Lokalitet</skos:prefLabel>
		<skos:prefLabel xml:lang="tr">Şantiye</skos:prefLabel>
		<skos:prefLabel xml:lang="ms">Tapak</skos:prefLabel>
		<skos:scopeNote>OGC LandInfra / InfraGML term</skos:scopeNote>
		<skos:definition>The area of land or water where construction work or other development is undertaken [ISO 6707-1:2014] (OGC LandInfra, 4.2.9).</skos:definition>
		<skos:changeNote>Established with version 3.</skos:changeNote>
		<skos:inScheme rdf:resource="http://www.cadastralvocabulary.org/CaLAThe"/>
		<skos:broader rdf:resource="http://www.cadastralvocabulary.org/CaLAThe/AdministrativeUnit"/>
	</skos:Concept>

	<skos:Concept rdf:about="http://www.cadastralvocabulary.org/CaLAThe/SocialGroup">
		<skos:prefLabel xml:lang="en">Social group</skos:prefLabel>
		<skos:prefLabel xml:lang="da">Samfundsgruppe</skos:prefLabel>
		<skos:prefLabel xml:lang="tr">Sosyal grup</skos:prefLabel>
		<skos:prefLabel xml:lang="ms">Kumpulan sosial</skos:prefLabel>
		<skos:scopeNote>GEMET term</skos:scopeNote>
		<skos:definition>A number of Natural persons who interact with one another according to certain societal norms and share certain feeling of unity.</skos:definition>
		<skos:changeNote>Established with version 1. Definition is changed with version 6.</skos:changeNote>
		<skos:exactMatch rdf:resource="http://aims.fao.org/aos/agrovoc/c_15520"/>
		<skos:exactMatch rdf:resource="http://www.eionet.europa.eu/gemet/concept/7796"/>
		<skos:exactMatch rdf:resource="http://zbw.eu/stw/descriptor/15714-0"/>
		<skos:inScheme rdf:resource="http://www.cadastralvocabulary.org/CaLAThe"/>
		<skos:broader rdf:resource="http://www.cadastralvocabulary.org/CaLAThe/GroupParty"/>
		<skos:narrower rdf:resource="http://www.cadastralvocabulary.org/CaLAThe/Family"/>
		<skos:narrower rdf:resource="http://www.cadastralvocabulary.org/CaLAThe/Tribe"/>
		<skos:related rdf:resource="http://www.cadastralvocabulary.org/CaLAThe/Association"/>
	</skos:Concept>

	<skos:Concept rdf:about="http://www.cadastralvocabulary.org/CaLAThe/SocietalRole">
		<skos:prefLabel xml:lang="en">Societal role</skos:prefLabel>
		<skos:prefLabel xml:lang="da">Rolle i samfundet</skos:prefLabel>
		<skos:prefLabel xml:lang="tr">Toplumsal rol</skos:prefLabel>
		<skos:prefLabel xml:lang="ms">Peranan masyarakat</skos:prefLabel>
		<skos:definition>A Natural person role gained and performed according to social norms.</skos:definition>
		<skos:changeNote>Established with version 2. Farmer and Neighbor added to narrower with version 5. Definition is added with version 6.</skos:changeNote>
		<skos:inScheme rdf:resource="http://www.cadastralvocabulary.org/CaLAThe"/>
		<skos:broader rdf:resource="http://www.cadastralvocabulary.org/CaLAThe/NaturalPersonRole"/>
		<skos:narrower rdf:resource="http://www.cadastralvocabulary.org/CaLAThe/Chief"/>
		<skos:narrower rdf:resource="http://www.cadastralvocabulary.org/CaLAThe/Farmer"/>
		<skos:narrower rdf:resource="http://www.cadastralvocabulary.org/CaLAThe/Neighbor"/>
	</skos:Concept>

	<skos:Concept rdf:about="http://www.cadastralvocabulary.org/CaLAThe/SpatialDataInfrastructure">
		<skos:prefLabel xml:lang="en">Spatial data infrastructure</skos:prefLabel>
		<skos:prefLabel xml:lang="da">Geografisk infrastruktur</skos:prefLabel>
		<skos:prefLabel xml:lang="tr">Coğrafi veri altyapısı</skos:prefLabel>
		<skos:prefLabel xml:lang="ms">Infrastruktur data spatial</skos:prefLabel>
		<skos:scopeNote>Joinup, EU Commission</skos:scopeNote>
		<skos:definition>A framework of policies, institutional arrangements, technologies, data, and people that enable the effective sharing and use of geographic information</skos:definition>
		<skos:changeNote>Established with version 1. Definition added with version 6.</skos:changeNote>
		<skos:inScheme rdf:resource="http://www.cadastralvocabulary.org/CaLAThe"/>
		<skos:broader rdf:resource="http://www.cadastralvocabulary.org/CaLAThe/GeolocatedInformation"/>
		<skos:narrower rdf:resource="http://www.cadastralvocabulary.org/CaLAThe/GeographicInformationSystem"/>
		<skos:narrower rdf:resource="http://www.cadastralvocabulary.org/CaLAThe/Gazetteer"/>
	</skos:Concept>

	<skos:Concept rdf:about="http://www.cadastralvocabulary.org/CaLAThe/SpatialFeatureType">
		<skos:prefLabel xml:lang="en">Spatial feature type</skos:prefLabel>
		<skos:prefLabel xml:lang="da">Geografiske objekter</skos:prefLabel>
		<skos:prefLabel xml:lang="tr">Coğrafi detay</skos:prefLabel>
		<skos:prefLabel xml:lang="ms">Jenis fitur spatial</skos:prefLabel>
		<skos:definition>Classification of spatial objects.</skos:definition>
		<skos:changeNote>Established with version 1. Edited with version 4.</skos:changeNote>
		<skos:inScheme rdf:resource="http://www.cadastralvocabulary.org/CaLAThe"/>
		<skos:broader rdf:resource="http://www.cadastralvocabulary.org/CaLAThe/Land"/>
		<skos:narrower rdf:resource="http://www.cadastralvocabulary.org/CaLAThe/LandDivision"/>
		<skos:narrower rdf:resource="http://www.cadastralvocabulary.org/CaLAThe/TopographicalFeature"/>
	</skos:Concept>

	<skos:Concept rdf:about="http://www.cadastralvocabulary.org/CaLAThe/TopologicalLocalization">
		<skos:prefLabel xml:lang="en">Spatial network</skos:prefLabel>
		<skos:prefLabel xml:lang="da">Geometrisk netværk</skos:prefLabel>
		<skos:prefLabel xml:lang="tr">Topolojik konumlama</skos:prefLabel>
		<skos:prefLabel xml:lang="ms">Rangkaian spatial</skos:prefLabel>
		<skos:definition>A Spatial network is a graph, where the topological primitive: node represents a location, while the topological primitive: edge represents the adjacency relationship between locations. A Spatial network is thus constrained by some geometry and embedded in a two- or three-dimensional space (cf. Ulrich, Nourbakhsh, 2000; Barthelemy, 2011)</skos:definition>
		<skos:changeNote>Introduced with version 4. Changed term to Spatial network with version 6. Edited definition.</skos:changeNote>
		<skos:inScheme rdf:resource="http://www.cadastralvocabulary.org/CaLAThe"/>
		<skos:broader rdf:resource="http://www.cadastralvocabulary.org/CaLAThe/GeolocatedInformation"/>
		<skos:narrower rdf:resource="http://www.cadastralvocabulary.org/CaLAThe/RoadNetwork"/>
	</skos:Concept>

	<skos:Concept rdf:about="http://www.cadastralvocabulary.org/CaLAThe/SpatialReference">
		<skos:prefLabel xml:lang="en">Spatial reference</skos:prefLabel>
		<skos:prefLabel xml:lang="da">Rumlig reference</skos:prefLabel>
		<skos:prefLabel xml:lang="tr">Coğrafi referans</skos:prefLabel>
		<skos:prefLabel xml:lang="ms">Rujukan spatial</skos:prefLabel>
		<skos:scopeNote>Geolexica and INSPIRE term</skos:scopeNote>
		<skos:definition>Description of position in the real world. Note to entry: This may take the form of a label, code or coordinate tuple. (Geolexica ISO 19111:2019)</skos:definition>
		<skos:changeNote>Established with version 1. Edited with version 4 to comply with Geolexica</skos:changeNote>
		<skos:exactMatch rdf:resource="https://isotc211.geolexica.org/concepts/421/"/>
		<skos:inScheme rdf:resource="http://www.cadastralvocabulary.org/CaLAThe"/>
		<skos:broader rdf:resource="http://www.cadastralvocabulary.org/CaLAThe/Information"/>
		<skos:narrower rdf:resource="http://www.cadastralvocabulary.org/CaLAThe/OrdinalScale"/>
		<skos:narrower rdf:resource="http://www.cadastralvocabulary.org/CaLAThe/GeographicalGridSystem"/>
		<skos:narrower rdf:resource="http://www.cadastralvocabulary.org/CaLAThe/CoordinateReferenceSystem"/>
	</skos:Concept>

	<skos:Concept rdf:about="http://www.cadastralvocabulary.org/CaLAThe/SpatialUnit">
		<skos:prefLabel xml:lang="en">Spatial unit</skos:prefLabel>
		<skos:prefLabel xml:lang="da">Rumlig enhed</skos:prefLabel>
		<skos:prefLabel xml:lang="tr">Konumsal birim</skos:prefLabel>
		<skos:prefLabel xml:lang="ms">Unit spatial</skos:prefLabel>
		<skos:scopeNote>ISO LADM and OGC LandInfra / InfraGML term</skos:scopeNote>
		<skos:definition>Contiguous geometrical entity, which is delimited and located on or close to the surface of the Earth through the bounding elements of its boundary. Compares to ISO 19152:2012 4.1.23 spatial unit (Source: OGC LandInfra, 4.8.14).</skos:definition>
		<skos:changeNote>Established with version 1.0. Replaced by SpatialType with version 3. Narrower of Geolocated information with version 4</skos:changeNote>
		<skos:exactMatch rdf:resource="http://aims.fao.org/aos/agrovoc/c_9df6243d"/>
		<skos:exactMatch rdf:resource="https://isotc211.geolexica.org/concepts/1363/"/>
		<skos:inScheme rdf:resource="http://www.cadastralvocabulary.org/CaLAThe"/>
		<skos:altLabel>LA_SpatialUnit</skos:altLabel>
		<skos:broader rdf:resource="http://www.cadastralvocabulary.org/CaLAThe/GeolocatedInformation"/>
		<skos:narrower rdf:resource="http://www.cadastralvocabulary.org/CaLAThe/TextLabelType"/>
		<skos:narrower rdf:resource="http://www.cadastralvocabulary.org/CaLAThe/GeometricPrimitive"/>
		<skos:narrower rdf:resource="http://www.cadastralvocabulary.org/CaLAThe/BoundingElement"/>
		<skos:narrower rdf:resource="http://www.cadastralvocabulary.org/CaLAThe/DimensionType"/>
		<skos:narrower rdf:resource="http://www.cadastralvocabulary.org/CaLAThe/TopologicalPrimitive"/>
	</skos:Concept>

	<skos:Concept rdf:about="http://www.cadastralvocabulary.org/CaLAThe/Stakeout">
		<skos:prefLabel xml:lang="en">Stakeout</skos:prefLabel>
		<skos:prefLabel xml:lang="da">Afsætning</skos:prefLabel>
		<skos:prefLabel xml:lang="tr">Aplikasyon</skos:prefLabel>
		<skos:prefLabel xml:lang="ms">Pemancangan</skos:prefLabel>
		<skos:scopeNote>OGC LandInfra / InfraGML term</skos:scopeNote>
		<skos:definition>Stakeout results contains the differences between the design and the resulted TargetPoint. The design point geometry is hold in the DesignPoint (OGC LandInfra 7.8.7.4)</skos:definition>
		<skos:changeNote>Established with version 4</skos:changeNote>
		<skos:exactMatch rdf:resource="http://docs.opengeospatial.org/is/15-111r1/15-111r1.html#162"/>
		<skos:inScheme rdf:resource="http://www.cadastralvocabulary.org/CaLAThe"/>
		<skos:broader rdf:resource="http://www.cadastralvocabulary.org/CaLAThe/TargetPoint"/>
		<skos:broader rdf:resource="http://www.cadastralvocabulary.org/CaLAThe/DesignPoint"/>
	</skos:Concept>

	<skos:Concept rdf:about="http://www.cadastralvocabulary.org/CaLAThe/StreetSign">
		<skos:prefLabel xml:lang="en">Street sign</skos:prefLabel>
		<skos:prefLabel xml:lang="da">Gadeskilt</skos:prefLabel>
		<skos:prefLabel xml:lang="tr">Sokak adı tabelası</skos:prefLabel>
		<skos:prefLabel xml:lang="ms">Tanda jalan</skos:prefLabel>
		<skos:definition>A sign that designates a street and is placed at intersections during a street addressing project (Source: Farvacque-Vitkovic et al, 2005)</skos:definition>
		<skos:changeNote>Established with version 1. Edited with version 4.</skos:changeNote>
		<skos:exactMatch rdf:resource="http://vocabulary.worldbank.org/thesaurus/1935900"/>
		<skos:exactMatch rdf:resource="http://data.europa.eu/cpv/cpv/34992300"/>
		<skos:inScheme rdf:resource="http://www.cadastralvocabulary.org/CaLAThe"/>
		<skos:altLabel>Plate</skos:altLabel>
		<skos:broader rdf:resource="http://www.cadastralvocabulary.org/CaLAThe/Marker"/>
		<skos:broader rdf:resource="http://www.cadastralvocabulary.org/CaLAThe/PostalAddress"/>
	</skos:Concept>

	<skos:Concept rdf:about="http://www.cadastralvocabulary.org/CaLAThe/StringDirection">
		<skos:prefLabel xml:lang="en">String direction</skos:prefLabel>
		<skos:scopeNote>OGC LandInfra / InfraGML term</skos:scopeNote>
		<skos:definition>For exterior boundary elements, the direction shall be counterclockwise (anti-clockwise) and for interior boundary elements (holes), the direction shall be clockwise. (OGC LandInfra 7.10.7)</skos:definition>
		<skos:inScheme rdf:resource="http://www.cadastralvocabulary.org/CaLAThe"/>
		<skos:broader rdf:resource="http://www.cadastralvocabulary.org/CaLAThe/BEString"/>
	</skos:Concept>

	<skos:Concept rdf:about="http://www.cadastralvocabulary.org/CaLAThe/StringType">
		<skos:prefLabel xml:lang="en">String type</skos:prefLabel>
		<skos:changeNote>Established with version 4</skos:changeNote>
		<skos:inScheme rdf:resource="http://www.cadastralvocabulary.org/CaLAThe"/>
		<skos:broader rdf:resource="http://www.cadastralvocabulary.org/CaLAThe/BEString"/>
		<skos:narrower rdf:resource="http://www.cadastralvocabulary.org/CaLAThe/LineString"/>
	</skos:Concept>

	<skos:Concept rdf:about="http://www.cadastralvocabulary.org/CaLAThe/Subdivision">
		<skos:prefLabel xml:lang="en">Subdivision</skos:prefLabel>
		<skos:prefLabel xml:lang="da">Udstykning</skos:prefLabel>
		<skos:prefLabel xml:lang="tr">Ayırma</skos:prefLabel>
		<skos:prefLabel xml:lang="ms">Pecah bahagian</skos:prefLabel>
		<skos:definition>Property formation where a Cadastral parcel is divided into smaller Cadastral parcels.</skos:definition>
		<skos:changeNote>Established with version 2.</skos:changeNote>
		<skos:inScheme rdf:resource="http://www.cadastralvocabulary.org/CaLAThe"/>
		<skos:broader rdf:resource="http://www.cadastralvocabulary.org/CaLAThe/PropertyFormation"/>
		<skos:narrower rdf:resource="http://www.cadastralvocabulary.org/CaLAThe/CondominiumSubdivision"/>
		<skos:narrower rdf:resource="http://www.cadastralvocabulary.org/CaLAThe/BoundarySurveyAndMarking"/>
	</skos:Concept>

	<skos:Concept rdf:about="http://www.cadastralvocabulary.org/CaLAThe/Sublease">
		<skos:prefLabel xml:lang="en">Sublease</skos:prefLabel>
		<skos:prefLabel xml:lang="da">Fremleje</skos:prefLabel>
		<skos:prefLabel xml:lang="tr">Devren kiralama</skos:prefLabel>
		<skos:prefLabel xml:lang="ms">Subpajakan</skos:prefLabel>
		<skos:definition>A lease granted by a lessee.</skos:definition>
		<skos:inScheme rdf:resource="http://www.cadastralvocabulary.org/CaLAThe"/>
		<skos:broader rdf:resource="http://www.cadastralvocabulary.org/CaLAThe/Leasehold"/>
	</skos:Concept>

	<skos:Concept rdf:about="http://www.cadastralvocabulary.org/CaLAThe/SuperficieObject">
		<skos:prefLabel xml:lang="en">Superficie object</skos:prefLabel>
		<skos:prefLabel xml:lang="da">Bygning på fremmed grund mv</skos:prefLabel>
		<skos:prefLabel xml:lang="tr">Üst hakkı nesnesi</skos:prefLabel>
		<skos:prefLabel xml:lang="ms">Objek superfisi</skos:prefLabel>
		<skos:scopeNote>OGC LandInfra / InfraGML term</skos:scopeNote>
		<skos:definition>A SuperficieObject comprises a building or other construction, including pipes, cables or tunnels, established and owned by a party (other than the owner of the LandParcels on which the superficie object is constructed) according to a granting Statement. (Source: OGC LandInfra 7.10.2.6, referring to http://www.dutchcivillaw.com/content/dutchcivillaw022.htm).</skos:definition>
		<skos:changeNote>Established with version 3.</skos:changeNote>
		<skos:inScheme rdf:resource="http://www.cadastralvocabulary.org/CaLAThe"/>
		<skos:altLabel>3D object</skos:altLabel>
		<skos:broader rdf:resource="http://www.cadastralvocabulary.org/CaLAThe/Construction"/>
		<skos:broader rdf:resource="http://www.cadastralvocabulary.org/CaLAThe/RealProperty"/>
		<skos:related rdf:resource="http://www.cadastralvocabulary.org/CaLAThe/CarrierParcel"/>
		<skos:related rdf:resource="http://www.cadastralvocabulary.org/CaLAThe/RightOfSuperficie"/>
	</skos:Concept>

	<skos:Concept rdf:about="http://www.cadastralvocabulary.org/CaLAThe/SuperficieObjectEstablishment">
		<skos:prefLabel xml:lang="en">Superficie object establishment</skos:prefLabel>
		<skos:prefLabel xml:lang="da"></skos:prefLabel>
		<skos:prefLabel xml:lang="tr">Üst hakkı tesisi</skos:prefLabel>
		<skos:prefLabel xml:lang="ms">Penubuhan objek superfisi</skos:prefLabel>
		<skos:scopeNote>OGC LandInfra / InfraGML term</skos:scopeNote>
		<skos:definition>Determination of objects (e.g. Construction) to be subject to the Right of superficies.</skos:definition>
		<skos:changeNote>Established with version 3.</skos:changeNote>
		<skos:inScheme rdf:resource="http://www.cadastralvocabulary.org/CaLAThe"/>
		<skos:altLabel>3D object identification</skos:altLabel>
		<skos:broader rdf:resource="http://www.cadastralvocabulary.org/CaLAThe/PropertyFormation"/>
	</skos:Concept>

	<skos:Concept rdf:about="http://www.cadastralvocabulary.org/CaLAThe/SuperficieObjectScheme">
		<skos:prefLabel xml:lang="en">Superficie object scheme</skos:prefLabel>
		<skos:prefLabel xml:lang="da">Dokument om superficieobjekt</skos:prefLabel>
		<skos:prefLabel xml:lang="tr">Üst hakkı sözleşmesi</skos:prefLabel>
		<skos:prefLabel xml:lang="ms">Skim objek superfisi</skos:prefLabel>
		<skos:scopeNote>OGC LandInfra / InfraGML term</skos:scopeNote>
		<skos:changeNote>Established with version 3.</skos:changeNote>
		<skos:inScheme rdf:resource="http://www.cadastralvocabulary.org/CaLAThe"/>
		<skos:altLabel>3D object scheme</skos:altLabel>
		<skos:broader rdf:resource="http://www.cadastralvocabulary.org/CaLAThe/Document"/>
	</skos:Concept>

	<skos:Concept rdf:about="http://www.cadastralvocabulary.org/CaLAThe/Surface">
		<skos:prefLabel xml:lang="en">Surface</skos:prefLabel>
		<skos:prefLabel xml:lang="da">Overflade</skos:prefLabel>
		<skos:prefLabel xml:lang="tr">Yüzey</skos:prefLabel>
		<skos:prefLabel xml:lang="ms">Permukaan</skos:prefLabel>
		<skos:scopeNote>Geolexica term</skos:scopeNote>
		<skos:definition>2-dimensional geometric primitive, locally representing a continuous image of a region of a plane. Note to entry: The boundary of a surface is the set of oriented, closed curves that delineate the limits of the surface. Surfaces that are isomorphic to a sphere, or to an n-torus (a topological sphere with n "handles") have no boundary. Such surfaces are called cycles. (Geolexica, ISO 19136-1:2020)</skos:definition>
		<skos:changeNote>Established with version 4.</skos:changeNote>
		<skos:exactMatch rdf:resource="https://isotc211.geolexica.org/concepts/437/"/>
		<skos:inScheme rdf:resource="http://www.cadastralvocabulary.org/CaLAThe"/>
		<skos:broader rdf:resource="http://www.cadastralvocabulary.org/CaLAThe/GeometricPrimitive"/>
		<skos:narrower rdf:resource="http://www.cadastralvocabulary.org/CaLAThe/Polygon"/>
	</skos:Concept>

	<skos:Concept rdf:about="http://www.cadastralvocabulary.org/CaLAThe/Survey">
		<skos:prefLabel xml:lang="en">Survey</skos:prefLabel>
		<skos:prefLabel xml:lang="da">Opmåling, Landmåling</skos:prefLabel>
		<skos:prefLabel xml:lang="tr">Ölçme</skos:prefLabel>
		<skos:prefLabel xml:lang="ms">Ukur</skos:prefLabel>
		<skos:scopeNote>OGC LandInfra / InfraGML term</skos:scopeNote>
		<skos:definition>(Observation procedure) Method, algorithm or instrument, or system of these, which may be used in making an observation (Source: ISO 19156:2011, 4.12)</skos:definition>
		<skos:changeNote>Established with version 4</skos:changeNote>
		<skos:exactMatch rdf:resource="https://www.eionet.europa.eu/gemet/en/concept/8240"/>
		<skos:inScheme rdf:resource="http://www.cadastralvocabulary.org/CaLAThe"/>
		<skos:narrower rdf:resource="http://www.cadastralvocabulary.org/CaLAThe/SurveyingInstrument"/>
		<skos:narrower rdf:resource="http://www.cadastralvocabulary.org/CaLAThe/SurveyResult"/>
	</skos:Concept>

	<skos:Concept rdf:about="http://www.cadastralvocabulary.org/CaLAThe/SurveyMark">
		<skos:prefLabel xml:lang="en">Survey mark</skos:prefLabel>
		<skos:prefLabel xml:lang="da">Afmærket punkt</skos:prefLabel>
		<skos:prefLabel xml:lang="tr">Ölçü noktası</skos:prefLabel>
		<skos:prefLabel xml:lang="ms">Tanda ukur</skos:prefLabel>
		<skos:scopeNote>OGC LandInfra / InfraGML term</skos:scopeNote>
		<skos:definition>Physical object which by its form defines a point on the surface of the Earth (Source: OGC LandInfra, 4.1.22).</skos:definition>
		<skos:changeNote>Established with version 3.</skos:changeNote>
		<skos:inScheme rdf:resource="http://www.cadastralvocabulary.org/CaLAThe"/>
		<skos:broader rdf:resource="http://www.cadastralvocabulary.org/CaLAThe/Marker"/>
		<skos:narrower rdf:resource="http://www.cadastralvocabulary.org/CaLAThe/BoundaryMark"/>
		<skos:narrower rdf:resource="http://www.cadastralvocabulary.org/CaLAThe/ControlPointMonument"/>
		<skos:narrower rdf:resource="http://www.cadastralvocabulary.org/CaLAThe/TrigonometricMark"/>
	</skos:Concept>

	<skos:Concept rdf:about="http://www.cadastralvocabulary.org/CaLAThe/SurveyMonumentEstablishment">
		<skos:prefLabel xml:lang="en">Survey monument establishment</skos:prefLabel>
		<skos:prefLabel xml:lang="da">Afmærkning af skel</skos:prefLabel>
		<skos:prefLabel xml:lang="tr">Ölçü noktası tesisi</skos:prefLabel>
		<skos:prefLabel xml:lang="ms">Penubuhan monumen ukur</skos:prefLabel>
		<skos:scopeNote>OGC LandInfra / InfraGML term</skos:scopeNote>
		<skos:definition>An Activity to mark survey points on the Earthâs surface.</skos:definition>
		<skos:changeNote>Established with version 3.</skos:changeNote>
		<skos:inScheme rdf:resource="http://www.cadastralvocabulary.org/CaLAThe"/>
		<skos:broader rdf:resource="http://www.cadastralvocabulary.org/CaLAThe/BoundarySurveyAndMarking"/>
	</skos:Concept>

	<skos:Concept rdf:about="http://www.cadastralvocabulary.org/CaLAThe/SurveyResult">
		<skos:prefLabel xml:lang="en">Survey result</skos:prefLabel>
		<skos:prefLabel xml:lang="da">Opmålingsresultat</skos:prefLabel>
		<skos:prefLabel xml:lang="tr">Ölçü sonucu</skos:prefLabel>
		<skos:prefLabel xml:lang="ms">Keputusan, Hasil pengukuran</skos:prefLabel>
		<skos:scopeNote>OGC LandInfra / InfraGML term</skos:scopeNote>
		<skos:definition>(Observation result) Estimate of the value of a property determined through a known observation procedure (Source: ISO 19156:2011, 4.14).</skos:definition>
		<skos:changeNote>Established with version 4</skos:changeNote>
		<skos:inScheme rdf:resource="http://www.cadastralvocabulary.org/CaLAThe"/>
		<skos:broader rdf:resource="http://www.cadastralvocabulary.org/CaLAThe/Survey"/>
		<skos:narrower rdf:resource="http://www.cadastralvocabulary.org/CaLAThe/Observation"/>
		<skos:narrower rdf:resource="http://www.cadastralvocabulary.org/CaLAThe/PointCloud"/>
		<skos:narrower rdf:resource="http://www.cadastralvocabulary.org/CaLAThe/Image"/>
		<skos:narrower rdf:resource="http://www.cadastralvocabulary.org/CaLAThe/TargetPoint"/>
		<skos:narrower rdf:resource="http://www.cadastralvocabulary.org/CaLAThe/DesignPoint"/>
	</skos:Concept>

	<skos:Concept rdf:about="http://www.cadastralvocabulary.org/CaLAThe/SurveyingInstrument">
		<skos:prefLabel xml:lang="en">Surveying instrument</skos:prefLabel>
		<skos:prefLabel xml:lang="da">Instrument</skos:prefLabel>
		<skos:prefLabel xml:lang="tr">Ölçme aleti</skos:prefLabel>
		<skos:prefLabel xml:lang="ms">Alat pengukuran</skos:prefLabel>
		<skos:changeNote>Established with version 4</skos:changeNote>
		<skos:inScheme rdf:resource="http://www.cadastralvocabulary.org/CaLAThe"/>
		<skos:broader rdf:resource="http://www.cadastralvocabulary.org/CaLAThe/Survey"/>
		<skos:narrower rdf:resource="http://www.cadastralvocabulary.org/CaLAThe/Camera"/>
		<skos:narrower rdf:resource="http://www.cadastralvocabulary.org/CaLAThe/Compass"/>
		<skos:narrower rdf:resource="http://www.cadastralvocabulary.org/CaLAThe/LI_Sensor"/>
		<skos:narrower rdf:resource="http://www.cadastralvocabulary.org/CaLAThe/MeasuringTape"/>
		<skos:narrower rdf:resource="http://www.cadastralvocabulary.org/CaLAThe/EletronicDistanceMeter"/>
		<skos:narrower rdf:resource="http://www.cadastralvocabulary.org/CaLAThe/Theodolite"/>
		<skos:narrower rdf:resource="http://www.cadastralvocabulary.org/CaLAThe/GNSSsensor"/>
		<skos:narrower rdf:resource="http://www.cadastralvocabulary.org/CaLAThe/TerrestrialLaserScanner"/>
		<skos:narrower rdf:resource="http://www.cadastralvocabulary.org/CaLAThe/TotalStation"/>
	</skos:Concept>

	<skos:Concept rdf:about="http://www.cadastralvocabulary.org/CaLAThe/Surveyor">
		<skos:prefLabel xml:lang="en">Surveyor</skos:prefLabel>
		<skos:prefLabel xml:lang="da">Landinspektør med beskikkelse</skos:prefLabel>
		<skos:prefLabel xml:lang="tr">Haritacı</skos:prefLabel>
		<skos:prefLabel xml:lang="ms">Juruukur</skos:prefLabel>
		<skos:definition>A Professional with the academic qualifications and technical expertise to practise the science of measurement; to assemble and assess land and geographic related information; to use that information for the purpose of planning and implementing the efficient administration of the land, the sea and structures thereon; and to instigate the advancement and development of such practices (FIG, https://www.fig.net/about/general/definition/definition.pdf) </skos:definition>
		<skos:changeNote>Established with version 1. Definition is added with version 6.</skos:changeNote>
		<skos:exactMatch rdf:resource="http://aims.fao.org/aos/agrovoc/c_26e30c73"/>
		<skos:inScheme rdf:resource="http://www.cadastralvocabulary.org/CaLAThe"/>
		<skos:broader rdf:resource="http://www.cadastralvocabulary.org/CaLAThe/Professional"/>
		<skos:narrower rdf:resource="http://www.cadastralvocabulary.org/CaLAThe/LicensedSurveyor"/>
		<skos:narrower rdf:resource="http://www.cadastralvocabulary.org/CaLAThe/LI_LandSurveyor"/>
		<skos:narrower rdf:resource="http://www.cadastralvocabulary.org/CaLAThe/LA_CertifiedSurveyor"/>
	</skos:Concept>

	<skos:Concept rdf:about="http://www.cadastralvocabulary.org/CaLAThe/TargetPoint">
		<skos:prefLabel xml:lang="en">Target point</skos:prefLabel>
		<skos:prefLabel xml:lang="da">Sigtepunkt</skos:prefLabel>
		<skos:prefLabel xml:lang="tr">Hedef noktası</skos:prefLabel>
		<skos:prefLabel xml:lang="ms">Titik sasaran</skos:prefLabel>
		<skos:scopeNote>OGC LandInfra / InfraGML term</skos:scopeNote>
		<skos:definition>TargetPoint is the value of a geometry of the feature of interest that has been estimated from the raw observations (OGC LandInfra 7.8.7.2)</skos:definition>
		<skos:changeNote>Established with version 4</skos:changeNote>
		<skos:inScheme rdf:resource="http://www.cadastralvocabulary.org/CaLAThe"/>
		<skos:broader rdf:resource="http://www.cadastralvocabulary.org/CaLAThe/SurveyResult"/>
		<skos:broader rdf:resource="http://www.cadastralvocabulary.org/CaLAThe/TPSobservation"/>
		<skos:broader rdf:resource="http://www.cadastralvocabulary.org/CaLAThe/GNSSobservation"/>
		<skos:narrower rdf:resource="http://www.cadastralvocabulary.org/CaLAThe/Stakeout"/>
	</skos:Concept>

	<skos:Concept rdf:about="http://www.cadastralvocabulary.org/CaLAThe/TerrestrialLaserScanner">
		<skos:prefLabel xml:lang="en">Terrestrial Laser Scanner</skos:prefLabel>
		<skos:prefLabel xml:lang="da">Terrestisk laserscanner</skos:prefLabel>
		<skos:prefLabel xml:lang="tr">Yersel lazer tarayıcı</skos:prefLabel>
		<skos:prefLabel xml:lang="ms">Pengimbas laser terestrial</skos:prefLabel>
		<skos:altLabel>Laser scanner</skos:altLabel>
		<skos:scopeNote>OGC LandInfra / InfraGML term</skos:scopeNote>
		<skos:definition>Terrestrial LaserScanner sensors are used to measure point clouds with the controlled steering of laser beams followed by a distance measurement at every pointing direction. (OGC LandInfra 7.8.5.12)</skos:definition>
		<skos:changeNote>Established with version 4</skos:changeNote>
		<skos:inScheme rdf:resource="http://www.cadastralvocabulary.org/CaLAThe"/>
		<skos:broader rdf:resource="http://www.cadastralvocabulary.org/CaLAThe/SurveyingInstrument"/>
		<skos:narrower rdf:resource="http://www.cadastralvocabulary.org/CaLAThe/PointCloud"/>
	</skos:Concept>

	<skos:Concept rdf:about="http://www.cadastralvocabulary.org/CaLAThe/TextLabelType">
		<skos:prefLabel xml:lang="en">Textlabel type</skos:prefLabel>
		<skos:scopeNote>OGC Land and Infrastructure Conceptual Model Standard (LandInfra) 15-111r1</skos:scopeNote>
		<skos:definition>The BoundingElement is described with text instead of having a geometric representation (LandInfra 7.10.7)</skos:definition>
		<skos:changeNote>Established with version 1. Definition added, and Broader changed to Bounding element with ver 6</skos:changeNote>
		<skos:inScheme rdf:resource="http://www.cadastralvocabulary.org/CaLAThe"/>
		<skos:broader rdf:resource="http://www.cadastralvocabulary.org/CaLAThe/BoundingElement"/>
	</skos:Concept>

	<skos:Concept rdf:about="http://www.cadastralvocabulary.org/CaLAThe/Theodolite">
		<skos:prefLabel xml:lang="en">Theodolite</skos:prefLabel>
		<skos:prefLabel xml:lang="da">Teodolit</skos:prefLabel>
		<skos:prefLabel xml:lang="tr">Teodolit</skos:prefLabel>
		<skos:prefLabel xml:lang="ms">Teodolit</skos:prefLabel>
		<skos:scopeNote>OGC LandInfra / InfraGML term</skos:scopeNote>
		<skos:definition>Instrument for measuring horizontal directions or horizontal directions and vertical angles, whose main components are the horizontal circle and the vertical circle, the telescope and additional devices for reading the graduated circles and for setting up the vertical axis (OGC LandInfra 4.6.18, referring to ISO 9849-1:2000)</skos:definition>
		<skos:changeNote>Established with version 4</skos:changeNote>
		<skos:inScheme rdf:resource="http://www.cadastralvocabulary.org/CaLAThe"/>
		<skos:broader rdf:resource="http://www.cadastralvocabulary.org/CaLAThe/SurveyingInstrument"/>
		<skos:narrower rdf:resource="http://www.cadastralvocabulary.org/CaLAThe/AngelObservation"/>
	</skos:Concept>

	<skos:Concept rdf:about="http://www.cadastralvocabulary.org/CaLAThe/TimeshareRight">
		<skos:prefLabel xml:lang="en">Timeshare right</skos:prefLabel>
		<skos:prefLabel xml:lang="da">Timeshare rettighed</skos:prefLabel>
		<skos:prefLabel xml:lang="tr">Devre mülk hakkı</skos:prefLabel>
		<skos:prefLabel xml:lang="ms">Hak bersama</skos:prefLabel>
		<skos:changeNote>Established with v1.</skos:changeNote>
		<skos:inScheme rdf:resource="http://www.cadastralvocabulary.org/CaLAThe"/>
		<skos:broader rdf:resource="http://www.cadastralvocabulary.org/CaLAThe/CoOwnership"/>
	</skos:Concept>

	<skos:Concept rdf:about="http://www.cadastralvocabulary.org/CaLAThe/Title">
		<skos:prefLabel xml:lang="en">Title</skos:prefLabel>
		<skos:prefLabel xml:lang="da">Adkomst</skos:prefLabel>
		<skos:prefLabel xml:lang="tr">Tapu</skos:prefLabel>
		<skos:prefLabel xml:lang="ms">Hakmilik</skos:prefLabel>
		<skos:scopeNote>EULIS / ELRA term</skos:scopeNote>
		<skos:definition>A Document that is proof of Ownership of Real property.</skos:definition>
		<skos:changeNote>Established with version 3. Definition is added with version 6.</skos:changeNote>
		<skos:inScheme rdf:resource="http://www.cadastralvocabulary.org/CaLAThe"/>
		<skos:broader rdf:resource="http://www.cadastralvocabulary.org/CaLAThe/Owner"/>
	</skos:Concept>

	<skos:Concept rdf:about="http://www.cadastralvocabulary.org/CaLAThe/TitleDeed">
		<skos:prefLabel xml:lang="en">Title deed</skos:prefLabel>
		<skos:prefLabel xml:lang="da">Skøde</skos:prefLabel>
		<skos:prefLabel xml:lang="tr">Tapu senedi</skos:prefLabel>
		<skos:prefLabel xml:lang="ms">Surat lkatan hakmilik</skos:prefLabel>
		<skos:changeNote>Established with version 1. </skos:changeNote>
		<skos:exactMatch rdf:resource="http://aims.fao.org/aos/agrovoc/c_b769471e"/>
		<skos:inScheme rdf:resource="http://www.cadastralvocabulary.org/CaLAThe"/>
		<skos:broader rdf:resource="http://www.cadastralvocabulary.org/CaLAThe/Deed"/>
	</skos:Concept>

	<skos:Concept rdf:about="http://www.cadastralvocabulary.org/CaLAThe/TopographicMap">
		<skos:prefLabel xml:lang="en">Topographic map</skos:prefLabel>
		<skos:prefLabel xml:lang="da">Topografisk kort</skos:prefLabel>
		<skos:prefLabel xml:lang="tr">Topoğrafik harita</skos:prefLabel>
		<skos:prefLabel xml:lang="ms">Peta topografi</skos:prefLabel>
		<skos:definition>A large-scale map, conveying the shape and pattern of a landscape (Cf. Harvey, 1980) </skos:definition>
		<skos:changeNote>Established with version 2.0. Definition added with version 6.</skos:changeNote>
		<skos:inScheme rdf:resource="http://www.cadastralvocabulary.org/CaLAThe"/>
		<skos:broader rdf:resource="http://www.cadastralvocabulary.org/CaLAThe/Map"/>
	</skos:Concept>

	<skos:Concept rdf:about="http://www.cadastralvocabulary.org/CaLAThe/TopographicalFeature">
		<skos:prefLabel xml:lang="en">Topographical feature</skos:prefLabel>
		<skos:prefLabel xml:lang="da">Topografisk objekt</skos:prefLabel>
		<skos:prefLabel xml:lang="tr">Topoğrafik detay</skos:prefLabel>
		<skos:prefLabel xml:lang="ms">Fitur topografi</skos:prefLabel>
		<skos:definition>Land and objects, described from a physical (non-administrative) perspective.</skos:definition>
		<skos:changeNote>Established with version 1. Definition is added in version 5.</skos:changeNote>
		<skos:inScheme rdf:resource="http://www.cadastralvocabulary.org/CaLAThe"/>
		<skos:broader rdf:resource="http://www.cadastralvocabulary.org/CaLAThe/SpatialFeatureType"/>
		<skos:narrower rdf:resource="http://www.cadastralvocabulary.org/CaLAThe/Hydrography"/>
		<skos:narrower rdf:resource="http://www.cadastralvocabulary.org/CaLAThe/Elevation"/>
		<skos:narrower rdf:resource="http://www.cadastralvocabulary.org/CaLAThe/TransportNetwork"/>
		<skos:narrower rdf:resource="http://www.cadastralvocabulary.org/CaLAThe/Construction"/>
	</skos:Concept>

	<skos:Concept rdf:about="http://www.cadastralvocabulary.org/CaLAThe/TopologicalPrimitive">
		<skos:prefLabel xml:lang="en">Topological primitive</skos:prefLabel>
		<skos:prefLabel xml:lang="da">Topologisk objekt</skos:prefLabel>
		<skos:prefLabel xml:lang="tr">Topolojik obje</skos:prefLabel>
		<skos:prefLabel xml:lang="ms">Topologi primitif</skos:prefLabel>
		<skos:scopeNote>ISO/PDTS 19104 term</skos:scopeNote>
		<skos:definition>A topological object that represents a single, non-decomposable element. (Source: ISO 19104:2016).</skos:definition>
		<skos:changeNote>Established with version 1.</skos:changeNote>
		<skos:exactMatch rdf:resource="https://isotc211.geolexica.org/concepts/2254/"/>
		<skos:inScheme rdf:resource="http://www.cadastralvocabulary.org/CaLAThe"/>
		<skos:broader rdf:resource="http://www.cadastralvocabulary.org/CaLAThe/SpatialUnit"/>
		<skos:narrower rdf:resource="http://www.cadastralvocabulary.org/CaLAThe/Node"/>
		<skos:narrower rdf:resource="http://www.cadastralvocabulary.org/CaLAThe/Edge"/>
		<skos:narrower rdf:resource="http://www.cadastralvocabulary.org/CaLAThe/Face"/>
	</skos:Concept>

	<skos:Concept rdf:about="http://www.cadastralvocabulary.org/CaLAThe/TotalStation">
		<skos:prefLabel xml:lang="en">Total station</skos:prefLabel>
		<skos:prefLabel xml:lang="da">Totalstation</skos:prefLabel>
		<skos:prefLabel xml:lang="tr">Totalstation</skos:prefLabel>
		<skos:prefLabel xml:lang="ms">Total station</skos:prefLabel>
		<skos:scopeNote>OGC LandInfra / InfraGML term</skos:scopeNote>
		<skos:changeNote>Established with version 4</skos:changeNote>
		<skos:inScheme rdf:resource="http://www.cadastralvocabulary.org/CaLAThe"/>
		<skos:broader rdf:resource="http://www.cadastralvocabulary.org/CaLAThe/SurveyingInstrument"/>
		<skos:narrower rdf:resource="http://www.cadastralvocabulary.org/CaLAThe/TPSobservation"/>
	</skos:Concept>

	<skos:Concept rdf:about="http://www.cadastralvocabulary.org/CaLAThe/TPSobservation">
		<skos:prefLabel xml:lang="en">TPSobservation</skos:prefLabel>
		<skos:prefLabel xml:lang="da">Vinkel- og afstandsmåling</skos:prefLabel>
		<skos:prefLabel xml:lang="tr">Açı ve mesafe ölçümü</skos:prefLabel>
		<skos:prefLabel xml:lang="ms">TPSobservation</skos:prefLabel>
		<skos:scopeNote>OGC LandInfra / InfraGML term</skos:scopeNote>
		<skos:changeNote>Established with version 4</skos:changeNote>
		<skos:inScheme rdf:resource="http://www.cadastralvocabulary.org/CaLAThe"/>
		<skos:broader rdf:resource="http://www.cadastralvocabulary.org/CaLAThe/TotalStation"/>
		<skos:broader rdf:resource="http://www.cadastralvocabulary.org/CaLAThe/Observation"/>
		<skos:narrower rdf:resource="http://www.cadastralvocabulary.org/CaLAThe/TargetPoint"/>
	</skos:Concept>

	<skos:Concept rdf:about="http://www.cadastralvocabulary.org/CaLAThe/Transfer">
		<skos:prefLabel xml:lang="en">Transfer</skos:prefLabel>
		<skos:prefLabel xml:lang="da">Overdragelse</skos:prefLabel>
		<skos:prefLabel xml:lang="tr">İntikal</skos:prefLabel>
		<skos:prefLabel xml:lang="ms">Pindah milik</skos:prefLabel>
		<skos:definition>The disposal of Real property or Real rights without any payment.</skos:definition>
		<skos:changeNote>Established with version 2.</skos:changeNote>
		<skos:exactMatch rdf:resource="http://eurovoc.europa.eu/4503"/>
		<skos:inScheme rdf:resource="http://www.cadastralvocabulary.org/CaLAThe"/>
		<skos:broader rdf:resource="http://www.cadastralvocabulary.org/CaLAThe/Activity"/>
		<skos:narrower rdf:resource="http://www.cadastralvocabulary.org/CaLAThe/Gift"/>
		<skos:narrower rdf:resource="http://www.cadastralvocabulary.org/CaLAThe/Inheritance"/>
		<skos:narrower rdf:resource="http://www.cadastralvocabulary.org/CaLAThe/Partition"/>
	</skos:Concept>

	<skos:Concept rdf:about="http://www.cadastralvocabulary.org/CaLAThe/TransferOfPartOfProperty">
		<skos:prefLabel xml:lang="en">Transfer of part of property</skos:prefLabel>
		<skos:prefLabel xml:lang="da">Arealoverførsel</skos:prefLabel>
		<skos:prefLabel xml:lang="tr">İfrazen devir</skos:prefLabel>
		<skos:prefLabel xml:lang="ms">Pindah milik sebahagian harta</skos:prefLabel>
		<skos:definition>Exchange of Property rights to a Real property part in the context of Property formation.</skos:definition>
		<skos:changeNote>Established with version 2.0.</skos:changeNote>
		<skos:inScheme rdf:resource="http://www.cadastralvocabulary.org/CaLAThe"/>
		<skos:broader rdf:resource="http://www.cadastralvocabulary.org/CaLAThe/PropertyFormation"/>
		<skos:narrower rdf:resource="http://www.cadastralvocabulary.org/CaLAThe/Reallotment"/>
	</skos:Concept>

	<skos:Concept rdf:about="http://www.cadastralvocabulary.org/CaLAThe/TransportNetwork">
		<skos:prefLabel xml:lang="en">Transport network</skos:prefLabel>
		<skos:prefLabel xml:lang="da">Transportnet</skos:prefLabel>
		<skos:prefLabel xml:lang="tr">Ulaşım ağı</skos:prefLabel>
		<skos:prefLabel xml:lang="ms">Rangkaian pengangkutan</skos:prefLabel>
		<skos:scopeNote>INSPIRE theme</skos:scopeNote>
		<skos:definition>Road, rail, air and water transport networks and related infrastructure. Includes links between different networks. Also includes the trans-European transport network as defined in Decision No 1692/96/EC of the European Parliament and of the Council of 23 July 1996 on Community Guidelines for the development of the trans-European transport network (1) and future revisions of that Decision (Source: INSPIRE theme register).</skos:definition>
		<skos:changeNote>Established with version 1.</skos:changeNote>
		<skos:exactMatch rdf:resource="http://inspire.ec.europa.eu/theme/tn"/>
		<skos:exactMatch rdf:resource="https://isotc211.geolexica.org/concepts/1621/"/>
		<skos:inScheme rdf:resource="http://www.cadastralvocabulary.org/CaLAThe"/>
		<skos:broader rdf:resource="http://www.cadastralvocabulary.org/CaLAThe/TopographicalFeature"/>
	</skos:Concept>

	<skos:Concept rdf:about="http://www.cadastralvocabulary.org/CaLAThe/Tribe">
		<skos:prefLabel xml:lang="en">Tribe</skos:prefLabel>
		<skos:prefLabel xml:lang="da">Stamme</skos:prefLabel>
		<skos:prefLabel xml:lang="tr">Aşiret</skos:prefLabel>
		<skos:prefLabel xml:lang="ms">Suku kaum</skos:prefLabel>
		<skos:definition>A Social group composed of numerous families, clans, or generations having shared ancestry, language and customs.</skos:definition>
		<skos:changeNote>Established with version 1. Definition is added with version 6.</skos:changeNote>
		<skos:exactMatch rdf:resource="http://aims.fao.org/aos/agrovoc/c_331526"/>
		<skos:inScheme rdf:resource="http://www.cadastralvocabulary.org/CaLAThe"/>
		<skos:broader rdf:resource="http://www.cadastralvocabulary.org/CaLAThe/SocialGroup"/>
	</skos:Concept>

	<skos:Concept rdf:about="http://www.cadastralvocabulary.org/CaLAThe/TrigonometricMark">
		<skos:prefLabel xml:lang="en">Trigonometric mark</skos:prefLabel>
		<skos:prefLabel xml:lang="da">Trigonometrisk postament</skos:prefLabel>
		<skos:prefLabel xml:lang="tr">Trigonometrik ölçü noktası</skos:prefLabel>
		<skos:prefLabel xml:lang="ms">Tanda trigonometri</skos:prefLabel>
		<skos:scopeNote>OGC LandInfra / InfraGML term</skos:scopeNote>
		<skos:definition>Marks an observation point of geodetic significance (Source: OGC LandInfra, 7.10.5.1)</skos:definition>
		<skos:changeNote>Established with version 3.</skos:changeNote>
		<skos:inScheme rdf:resource="http://www.cadastralvocabulary.org/CaLAThe"/>
		<skos:broader rdf:resource="http://www.cadastralvocabulary.org/CaLAThe/SurveyMark"/>
	</skos:Concept>

	<skos:Concept rdf:about="http://www.cadastralvocabulary.org/CaLAThe/UserDefinedValue">
		<skos:prefLabel xml:lang="en">User defined value</skos:prefLabel>
		<skos:prefLabel xml:lang="da">Brugerdefineret værdi</skos:prefLabel>
		<skos:prefLabel xml:lang="tr">Özel değer</skos:prefLabel>
		<skos:prefLabel xml:lang="ms">Nilai takrifan pengguna</skos:prefLabel>
		<skos:inScheme rdf:resource="http://www.cadastralvocabulary.org/CaLAThe"/>
		<skos:broader rdf:resource="http://www.cadastralvocabulary.org/CaLAThe/CodeList"/>
	</skos:Concept>

	<skos:Concept rdf:about="http://www.cadastralvocabulary.org/CaLAThe/Usufruct">
		<skos:prefLabel xml:lang="en">Usufruct</skos:prefLabel>
		<skos:prefLabel xml:lang="da">Brugsret</skos:prefLabel>
		<skos:prefLabel xml:lang="tr">Yararlanma (intifa) hakkı</skos:prefLabel>
		<skos:prefLabel xml:lang="ms">Usufruk</skos:prefLabel>
		<skos:scopeNote>EULIS / ELRA term</skos:scopeNote>
		<skos:definition>Temporary right to use and enjoy the benefit and gain of the property of another, without changing the character of the property. (Source: EULIS / ELRA glossary)</skos:definition>
		<skos:exactMatch rdf:resource="http://aims.fao.org/aos/agrovoc/c_28784"/>
		<skos:exactMatch rdf:resource="http://eurovoc.europa.eu/4625"/>
		<skos:inScheme rdf:resource="http://www.cadastralvocabulary.org/CaLAThe"/>
		<skos:broader rdf:resource="http://www.cadastralvocabulary.org/CaLAThe/LimitedRight"/>
	</skos:Concept>

</rdf:RDF>
